refine: arch-split Finalise_R
Signed-off-by: Rafal Kolanski <rafal.kolanski@proofcraft.systems>

proof/refine/ARM/ArchFinalise_R.thy
@@ -1,5 +1,6 @@
 (*
  * Copyright 2014, General Dynamics C4 Systems
+ * Copyright 2023, Proofcraft Pty Ltd
  *
  * SPDX-License-Identifier: GPL-2.0-only
  *)
@@ -9,475 +10,80 @@ imports
   Finalise_R
 begin
 
-context begin interpretation Arch . (*FIXME: arch-split*)
+context Arch begin arch_global_naming
 
-declare doUnbindNotification_def[simp]
+named_theorems Finalise_R_assms
 
 lemma isArchSGISignalCap_NullCap[simp]:
   "\<not>isArchSGISignalCap NullCap"
   by (simp add: isCap_simps)
 
-text \<open>Properties about empty_slot/emptySlot\<close>
+lemma arch_postCapDeletion_ksArchState_lift[Finalise_R_assms]:
+  "\<lbrakk>\<And>s as. P (s\<lparr>ksArchState := as\<rparr>) = P s\<rbrakk> \<Longrightarrow> Arch.postCapDeletion ac \<lbrace>P\<rbrace>"
+  unfolding postCapDeletion_def
+  by wpsimp
 
-lemma case_Null_If:
-  "(case c of NullCap \<Rightarrow> a | _ \<Rightarrow> b) = (if c = NullCap then a else b)"
-  by (case_tac c, simp_all)
+lemmas clearUntypedFreeIndex_typ_ats[wp] = typ_at_lifts[OF clearUntypedFreeIndex_typ_at']
 
-crunch emptySlot
-  for aligned'[wp]: pspace_aligned' (simp: case_Null_If)
-crunch emptySlot
-  for distinct'[wp]: pspace_distinct' (simp: case_Null_If)
+crunch setIRQState
+  for umm[Finalise_R_assms, wp]: "\<lambda>s. P (underlying_memory (ksMachineState s))"
+  (wp: dmo_lift' simp: maskInterrupt_def)
 
-lemma updateCap_cte_wp_at_cases:
-  "\<lbrace>\<lambda>s. (ptr = ptr' \<longrightarrow> cte_wp_at' (P \<circ> cteCap_update (K cap)) ptr' s) \<and> (ptr \<noteq> ptr' \<longrightarrow> cte_wp_at' P ptr' s)\<rbrace>
-     updateCap ptr cap
-   \<lbrace>\<lambda>rv. cte_wp_at' P ptr'\<rbrace>"
-  apply (clarsimp simp: valid_def)
-  apply (drule updateCap_stuff)
-  apply (clarsimp simp: cte_wp_at_ctes_of modify_map_def)
-  done
+(* better crunch names for Arch.postCapDeletion *)
+abbreviation (input)
+  "Arch_postCapDeletion \<equiv> Arch.postCapDeletion"
 
-crunch postCapDeletion, updateTrackedFreeIndex
-  for cte_wp_at'[wp]: "cte_wp_at' P p"
+crunch Arch_postCapDeletion
+  for valid_global_refs[wp]: valid_global_refs'
+  and valid_arch_state'[wp]: valid_arch_state'
+  (rule: ARM_H.postCapDeletion_def)
 
-lemma updateFreeIndex_cte_wp_at:
-  "\<lbrace>\<lambda>s. cte_at' p s \<and> P (cte_wp_at' (if p = p' then P'
-      o (cteCap_update (capFreeIndex_update (K idx))) else P') p' s)\<rbrace>
-    updateFreeIndex p idx
-  \<lbrace>\<lambda>rv s. P (cte_wp_at' P' p' s)\<rbrace>"
-  apply (simp add: updateFreeIndex_def updateTrackedFreeIndex_def
-        split del: if_split)
-  apply (rule hoare_pre)
-   apply (wp updateCap_cte_wp_at' getSlotCap_wp)
-  apply (clarsimp simp: cte_wp_at_ctes_of)
-  apply (cases "p' = p", simp_all)
-  apply (case_tac cte, simp)
-  done
+lemma arch_postCapDeletion_corres[Finalise_R_assms]:
+  "acap_relation cap cap' \<Longrightarrow> corres dc \<top> \<top> (arch_post_cap_deletion cap) (ARM_H.postCapDeletion cap')"
+  by (clarsimp simp: arch_post_cap_deletion_def ARM_H.postCapDeletion_def)
 
-lemma emptySlot_cte_wp_cap_other:
-  "\<lbrace>(\<lambda>s. cte_wp_at' (\<lambda>c. P (cteCap c)) p s) and K (p \<noteq> p')\<rbrace>
-  emptySlot p' opt
-  \<lbrace>\<lambda>rv s. cte_wp_at' (\<lambda>c. P (cteCap c)) p s\<rbrace>"
-  apply (rule hoare_gen_asm)
-  apply (simp add: emptySlot_def clearUntypedFreeIndex_def getSlotCap_def)
-  apply (rule hoare_pre)
-   apply (wp updateMDB_weak_cte_wp_at updateCap_cte_wp_at_cases
-             updateFreeIndex_cte_wp_at getCTE_wp' hoare_vcg_all_lift
-              | simp add:  | wpc
-              | wp (once) hoare_drop_imps)+
-  done
+(* better crunch names for Arch.finaliseCap *)
+abbreviation (input)
+  "Arch_finaliseCap \<equiv> Arch.finaliseCap"
 
-lemmas clearUntypedFreeIndex_typ_ats[wp]
-    = typ_at_lifts[OF clearUntypedFreeIndex_typ_at']
+crunch Arch_finaliseCap, prepareThreadDelete, archThreadSet
+  for typ_at'[Finalise_R_assms, wp]: "\<lambda>s. P (typ_at' T p s)"
+  and aligned'[Finalise_R_assms, wp]: "pspace_aligned'"
+  and distinct'[Finalise_R_assms, wp]: "pspace_distinct'"
+  (wp: crunch_wps getObject_inv loadObject_default_inv
+   simp: crunch_simps unless_def o_def
+   ignore_del: setObject
+   rule: ARM_H.finaliseCap_def)
 
-crunch postCapDeletion
-  for tcb_at'[wp]: "tcb_at' t"
-crunch emptySlot
-  for ct[wp]: "\<lambda>s. P (ksCurThread s)"
-crunch clearUntypedFreeIndex
-  for cur_tcb'[wp]: "cur_tcb'"
-  (wp: cur_tcb_lift)
+crunch prepareThreadDelete, Arch_finaliseCap
+  for it'[Finalise_R_assms, wp]: "\<lambda>s. P (ksIdleThread s)"
+  (wp: hoare_drop_imps mapM_wp
+   simp: crunch_simps updateObject_default_def
+   rule: ARM_H.finaliseCap_def)
 
-crunch emptySlot
-  for ksRQ[wp]: "\<lambda>s. P (ksReadyQueues s)"
-crunch emptySlot
-  for ksRQL1[wp]: "\<lambda>s. P (ksReadyQueuesL1Bitmap s)"
-crunch emptySlot
-  for ksRQL2[wp]: "\<lambda>s. P (ksReadyQueuesL2Bitmap s)"
-crunch postCapDeletion
-  for obj_at'[wp]: "obj_at' P p"
+definition
+  arch_final_matters' :: "arch_capability \<Rightarrow> bool" where
+ "arch_final_matters' acap \<equiv> case acap of
+    PageCap ref rghts sz d mapdata \<Rightarrow> False
+  | ASIDControlCap \<Rightarrow> False
+  | SGISignalCap _ _ \<Rightarrow> False
+  | _ \<Rightarrow> True"
 
-crunch clearUntypedFreeIndex
-  for inQ[wp]: "\<lambda>s. P (obj_at' (inQ d p) t s)"
-crunch clearUntypedFreeIndex
-  for tcbDomain[wp]: "obj_at' (\<lambda>tcb. P (tcbDomain tcb)) t"
-crunch clearUntypedFreeIndex
-  for tcbPriority[wp]: "obj_at' (\<lambda>tcb. P (tcbPriority tcb)) t"
+definition arch_cap_has_cleanup' :: "arch_capability \<Rightarrow> bool" where
+  "arch_cap_has_cleanup' _ \<equiv> False"
 
-crunch emptySlot
-  for nosch[wp]: "\<lambda>s. P (ksSchedulerAction s)"
-crunch emptySlot
-  for ksCurDomain[wp]: "\<lambda>s. P (ksCurDomain s)"
+definition
+  "post_cap_delete_pre' cap sl cs \<equiv> case cap of
+     IRQHandlerCap irq \<Rightarrow> irq \<le> maxIRQ \<and> (\<forall>sl'. sl \<noteq> sl' \<longrightarrow> cs sl' \<noteq> Some cap)
+   | _ \<Rightarrow> False"
 
-lemma emptySlot_sch_act_wf [wp]:
-  "\<lbrace>\<lambda>s. sch_act_wf (ksSchedulerAction s) s\<rbrace>
-  emptySlot sl opt
-  \<lbrace>\<lambda>rv s. sch_act_wf (ksSchedulerAction s) s\<rbrace>"
-  apply (simp add: emptySlot_def case_Null_If)
-  apply (wp sch_act_wf_lift tcb_in_cur_domain'_lift | wpcw | simp)+
-  done
+end (* Arch *)
 
-lemma updateCap_valid_objs' [wp]:
-  "\<lbrace>valid_objs' and valid_cap' cap\<rbrace>
-  updateCap ptr cap \<lbrace>\<lambda>r. valid_objs'\<rbrace>"
-  unfolding updateCap_def
-  by (wp setCTE_valid_objs getCTE_wp) (clarsimp dest!: cte_at_cte_wp_atD)
+arch_requalify_consts
+  arch_final_matters'
+  arch_cap_has_cleanup'
 
-lemma updateFreeIndex_valid_objs' [wp]:
-  "\<lbrace>valid_objs'\<rbrace> clearUntypedFreeIndex ptr \<lbrace>\<lambda>r. valid_objs'\<rbrace>"
-  apply (simp add: clearUntypedFreeIndex_def getSlotCap_def)
-  apply (wp getCTE_wp' | wpc | simp add: updateTrackedFreeIndex_def)+
-  done
-
-crunch emptySlot
-  for valid_objs'[wp]: "valid_objs'"
-
-crunch setInterruptState
-  for state_refs_of'[wp]: "\<lambda>s. P (state_refs_of' s)"
-  (simp: state_refs_of'_pspaceI)
-crunch emptySlot
-  for state_refs_of'[wp]: "\<lambda>s. P (state_refs_of' s)"
-  (wp: crunch_wps)
-
-lemma mdb_chunked2D:
-  "\<lbrakk> mdb_chunked m; m \<turnstile> p \<leadsto> p'; m \<turnstile> p' \<leadsto> p'';
-     m p = Some (CTE cap nd); m p'' = Some (CTE cap'' nd'');
-     sameRegionAs cap cap''; p \<noteq> p''; mdb_chunked_arch_assms cap \<rbrakk>
-     \<Longrightarrow> \<exists>cap' nd'. m p' = Some (CTE cap' nd') \<and> sameRegionAs cap cap'"
-  apply (subgoal_tac "\<exists>cap' nd'. m p' = Some (CTE cap' nd')")
-   apply (clarsimp simp add: mdb_chunked_def)
-   apply (drule spec[where x=p])
-   apply (drule spec[where x=p''])
-   apply clarsimp
-   apply (drule mp, erule trancl_into_trancl2)
-    apply (erule trancl.intros(1))
-   apply (simp add: is_chunk_def)
-   apply (drule spec, drule mp, erule trancl.intros(1))
-   apply (drule mp, rule trancl_into_rtrancl)
-    apply (erule trancl.intros(1))
-   apply clarsimp
-  apply (clarsimp simp: mdb_next_unfold)
-  apply (case_tac z, simp)
-  done
-
-lemma nullPointer_eq_0_simp[simp]: (* FIXME: move to nullPointer_0_simp in Retype_R *)
-  "(0 = nullPointer) = True"
-  by (simp add: nullPointer_def)+
-
-lemma no_0_no_0_lhs_trancl [simp]:
-  "no_0 m \<Longrightarrow> \<not> m \<turnstile> 0 \<leadsto>\<^sup>+ x"
-  by (rule, drule tranclD, clarsimp simp: next_unfold')
-
-lemma no_0_no_0_lhs_rtrancl [simp]:
-  "\<lbrakk> no_0 m; x \<noteq> 0 \<rbrakk> \<Longrightarrow> \<not> m \<turnstile> 0 \<leadsto>\<^sup>* x"
-  by (clarsimp dest!: rtranclD)
-
-end
-locale mdb_empty =
-  mdb_ptr?: mdb_ptr m _ _ slot s_cap s_node
-    for m slot s_cap s_node +
-
-  fixes n
-  defines "n \<equiv>
-           modify_map
-             (modify_map
-               (modify_map
-                 (modify_map m (mdbPrev s_node)
-                   (cteMDBNode_update (mdbNext_update (%_. (mdbNext s_node)))))
-                 (mdbNext s_node)
-                 (cteMDBNode_update
-                   (\<lambda>mdb. mdbFirstBadged_update (%_. (mdbFirstBadged mdb \<or> mdbFirstBadged s_node))
-                           (mdbPrev_update (%_. (mdbPrev s_node)) mdb))))
-               slot (cteCap_update (%_. capability.NullCap)))
-              slot (cteMDBNode_update (const nullMDBNode))"
-begin
-interpretation Arch . (*FIXME: arch-split*)
-
-lemmas m_slot_prev = m_p_prev
-lemmas m_slot_next = m_p_next
-lemmas prev_slot_next = prev_p_next
-lemmas next_slot_prev = next_p_prev
-
-lemma n_revokable:
-  "n p = Some (CTE cap node) \<Longrightarrow>
-  (\<exists>cap' node'. m p = Some (CTE cap' node') \<and>
-              (if p = slot
-               then \<not> mdbRevocable node
-               else mdbRevocable node = mdbRevocable node'))"
-  by (auto simp add: n_def modify_map_if nullMDBNode_def split: if_split_asm)
-
-lemma m_revokable:
-  "m p = Some (CTE cap node) \<Longrightarrow>
-  (\<exists>cap' node'. n p = Some (CTE cap' node') \<and>
-              (if p = slot
-               then \<not> mdbRevocable node'
-               else mdbRevocable node' = mdbRevocable node))"
-  apply (clarsimp simp add: n_def modify_map_if nullMDBNode_def split: if_split_asm)
-  apply (cases "p=slot", simp)
-  apply (cases "p=mdbNext s_node", simp)
-   apply (cases "p=mdbPrev s_node", simp)
-   apply clarsimp
-  apply simp
-  apply (cases "p=mdbPrev s_node", simp)
-  apply simp
-  done
-
-lemma no_0_n:
-  "no_0 n"
-  using no_0 by (simp add: n_def)
-
-lemma n_next:
-  "n p = Some (CTE cap node) \<Longrightarrow>
-  (\<exists>cap' node'. m p = Some (CTE cap' node') \<and>
-              (if p = slot
-               then mdbNext node = 0
-               else if p = mdbPrev s_node
-               then mdbNext node = mdbNext s_node
-               else mdbNext node = mdbNext node'))"
-  apply (subgoal_tac "p \<noteq> 0")
-   prefer 2
-   apply (insert no_0_n)[1]
-   apply clarsimp
-  apply (cases "p = slot")
-   apply (clarsimp simp: n_def modify_map_if initMDBNode_def split: if_split_asm)
-  apply (cases "p = mdbPrev s_node")
-   apply (auto simp: n_def modify_map_if initMDBNode_def split: if_split_asm)
-  done
-
-lemma n_prev:
-  "n p = Some (CTE cap node) \<Longrightarrow>
-  (\<exists>cap' node'. m p = Some (CTE cap' node') \<and>
-              (if p = slot
-               then mdbPrev node = 0
-               else if p = mdbNext s_node
-               then mdbPrev node = mdbPrev s_node
-               else mdbPrev node = mdbPrev node'))"
-  apply (subgoal_tac "p \<noteq> 0")
-   prefer 2
-   apply (insert no_0_n)[1]
-   apply clarsimp
-  apply (cases "p = slot")
-   apply (clarsimp simp: n_def modify_map_if initMDBNode_def split: if_split_asm)
-  apply (cases "p = mdbNext s_node")
-   apply (auto simp: n_def modify_map_if initMDBNode_def split: if_split_asm)
-  done
-
-lemma n_cap:
-  "n p = Some (CTE cap node) \<Longrightarrow>
-  \<exists>cap' node'. m p = Some (CTE cap' node') \<and>
-              (if p = slot
-               then cap = NullCap
-               else cap' = cap)"
-  apply (clarsimp simp: n_def modify_map_if initMDBNode_def split: if_split_asm)
-   apply (cases node)
-   apply auto
-  done
-
-lemma m_cap:
-  "m p = Some (CTE cap node) \<Longrightarrow>
-  \<exists>cap' node'. n p = Some (CTE cap' node') \<and>
-              (if p = slot
-               then cap' = NullCap
-               else cap' = cap)"
-  apply (clarsimp simp: n_def modify_map_cases initMDBNode_def)
-  apply (cases node)
-  apply clarsimp
-  apply (cases "p=slot", simp)
-  apply clarsimp
-  apply (cases "mdbNext s_node = p", simp)
-   apply fastforce
-  apply simp
-  apply (cases "mdbPrev s_node = p", simp)
-  apply fastforce
-  done
-
-lemma n_badged:
-  "n p = Some (CTE cap node) \<Longrightarrow>
-  \<exists>cap' node'. m p = Some (CTE cap' node') \<and>
-              (if p = slot
-               then \<not> mdbFirstBadged node
-               else if p = mdbNext s_node
-               then mdbFirstBadged node = (mdbFirstBadged node' \<or> mdbFirstBadged s_node)
-               else mdbFirstBadged node = mdbFirstBadged node')"
-  apply (subgoal_tac "p \<noteq> 0")
-   prefer 2
-   apply (insert no_0_n)[1]
-   apply clarsimp
-  apply (cases "p = slot")
-   apply (clarsimp simp: n_def modify_map_if initMDBNode_def split: if_split_asm)
-  apply (cases "p = mdbNext s_node")
-   apply (auto simp: n_def modify_map_if nullMDBNode_def split: if_split_asm)
-  done
-
-lemma m_badged:
-  "m p = Some (CTE cap node) \<Longrightarrow>
-  \<exists>cap' node'. n p = Some (CTE cap' node') \<and>
-              (if p = slot
-               then \<not> mdbFirstBadged node'
-               else if p = mdbNext s_node
-               then mdbFirstBadged node' = (mdbFirstBadged node \<or> mdbFirstBadged s_node)
-               else mdbFirstBadged node' = mdbFirstBadged node)"
-  apply (subgoal_tac "p \<noteq> 0")
-   prefer 2
-   apply (insert no_0_n)[1]
-   apply clarsimp
-  apply (cases "p = slot")
-   apply (clarsimp simp: n_def modify_map_if nullMDBNode_def split: if_split_asm)
-  apply (cases "p = mdbNext s_node")
-   apply (clarsimp simp: n_def modify_map_if nullMDBNode_def split: if_split_asm)
-  apply clarsimp
-  apply (cases "p = mdbPrev s_node")
-   apply (auto simp: n_def modify_map_if initMDBNode_def  split: if_split_asm)
-  done
-
-lemmas slot = m_p
-
-lemma m_next:
-  "m p = Some (CTE cap node) \<Longrightarrow>
-  \<exists>cap' node'. n p = Some (CTE cap' node') \<and>
-              (if p = slot
-               then mdbNext node' = 0
-               else if p = mdbPrev s_node
-               then mdbNext node' = mdbNext s_node
-               else mdbNext node' = mdbNext node)"
-  apply (subgoal_tac "p \<noteq> 0")
-   prefer 2
-   apply clarsimp
-  apply (cases "p = slot")
-   apply (clarsimp simp: n_def modify_map_if)
-  apply (cases "p = mdbPrev s_node")
-   apply (simp add: n_def modify_map_if)
-  apply simp
-  apply (simp add: n_def modify_map_if)
-  apply (cases "mdbNext s_node = p")
-   apply fastforce
-  apply fastforce
-  done
-
-lemma m_prev:
-  "m p = Some (CTE cap node) \<Longrightarrow>
-  \<exists>cap' node'. n p = Some (CTE cap' node') \<and>
-              (if p = slot
-               then mdbPrev node' = 0
-               else if p = mdbNext s_node
-               then mdbPrev node' = mdbPrev s_node
-               else mdbPrev node' = mdbPrev node)"
-  apply (subgoal_tac "p \<noteq> 0")
-   prefer 2
-   apply clarsimp
-  apply (cases "p = slot")
-   apply (clarsimp simp: n_def modify_map_if)
-  apply (cases "p = mdbPrev s_node")
-   apply (simp add: n_def modify_map_if)
-  apply simp
-  apply (simp add: n_def modify_map_if)
-  apply (cases "mdbNext s_node = p")
-   apply fastforce
-  apply fastforce
-  done
-
-lemma n_nextD:
-  "n \<turnstile> p \<leadsto> p' \<Longrightarrow>
-  if p = slot then p' = 0
-  else if p = mdbPrev s_node
-  then m \<turnstile> p \<leadsto> slot \<and> p' = mdbNext s_node
-  else m \<turnstile> p \<leadsto> p'"
-  apply (clarsimp simp: mdb_next_unfold split del: if_split cong: if_cong)
-  apply (case_tac z)
-  apply (clarsimp split del: if_split)
-  apply (drule n_next)
-  apply (elim exE conjE)
-  apply (simp split: if_split_asm)
-  apply (frule dlist_prevD [OF m_slot_prev])
-  apply (clarsimp simp: mdb_next_unfold)
-  done
-
-lemma n_next_eq:
-  "n \<turnstile> p \<leadsto> p' =
-  (if p = slot then p' = 0
-  else if p = mdbPrev s_node
-  then m \<turnstile> p \<leadsto> slot \<and> p' = mdbNext s_node
-  else m \<turnstile> p \<leadsto> p')"
-  apply (rule iffI)
-   apply (erule n_nextD)
-  apply (clarsimp simp: mdb_next_unfold split: if_split_asm)
-    apply (simp add: n_def modify_map_if slot)
-   apply hypsubst_thin
-   apply (case_tac z)
-   apply simp
-   apply (drule m_next)
-   apply clarsimp
-  apply (case_tac z)
-  apply simp
-  apply (drule m_next)
-  apply clarsimp
-  done
-
-lemma n_prev_eq:
-  "n \<turnstile> p \<leftarrow> p' =
-  (if p' = slot then p = 0
-  else if p' = mdbNext s_node
-  then m \<turnstile> slot \<leftarrow> p' \<and> p = mdbPrev s_node
-  else m \<turnstile> p \<leftarrow> p')"
-  apply (rule iffI)
-   apply (clarsimp simp: mdb_prev_def split del: if_split cong: if_cong)
-   apply (case_tac z)
-   apply (clarsimp split del: if_split)
-   apply (drule n_prev)
-   apply (elim exE conjE)
-   apply (simp split: if_split_asm)
-   apply (frule dlist_nextD [OF m_slot_next])
-   apply (clarsimp simp: mdb_prev_def)
-  apply (clarsimp simp: mdb_prev_def split: if_split_asm)
-    apply (simp add: n_def modify_map_if slot)
-   apply hypsubst_thin
-   apply (case_tac z)
-   apply clarsimp
-   apply (drule m_prev)
-   apply clarsimp
-  apply (case_tac z)
-  apply simp
-  apply (drule m_prev)
-  apply clarsimp
-  done
-
-lemma valid_dlist_n:
-  "valid_dlist n" using dlist
-  apply (clarsimp simp: valid_dlist_def2 [OF no_0_n])
-  apply (simp add: n_next_eq n_prev_eq m_slot_next m_slot_prev cong: if_cong)
-  apply (rule conjI, clarsimp)
-   apply (rule conjI, clarsimp simp: next_slot_prev prev_slot_next)
-   apply (fastforce dest!: dlist_prev_src_unique)
-  apply clarsimp
-  apply (rule conjI, clarsimp)
-   apply (clarsimp simp: valid_dlist_def2 [OF no_0])
-   apply (case_tac "mdbNext s_node = 0")
-    apply simp
-    apply (subgoal_tac "m \<turnstile> slot \<leadsto> c'")
-     prefer 2
-     apply fastforce
-    apply (clarsimp simp: mdb_next_unfold slot)
-   apply (frule next_slot_prev)
-   apply (drule (1) dlist_prev_src_unique, simp)
-   apply simp
-  apply clarsimp
-  apply (rule conjI, clarsimp)
-   apply (fastforce dest: dlist_next_src_unique)
-  apply clarsimp
-  apply (rule conjI, clarsimp)
-   apply (clarsimp simp: valid_dlist_def2 [OF no_0])
-   apply (clarsimp simp: mdb_prev_def slot)
-  apply (clarsimp simp: valid_dlist_def2 [OF no_0])
-  done
-
-lemma caps_contained_n:
-  "caps_contained' n"
-  using valid
-  apply (clarsimp simp: valid_mdb_ctes_def caps_contained'_def)
-  apply (drule n_cap)+
-  apply (clarsimp split: if_split_asm)
-  apply (erule disjE, clarsimp)
-  apply clarsimp
-  apply fastforce
-  done
-
-lemma chunked:
-  "mdb_chunked m"
-  using valid ..
-
-lemma valid_badges:
-  "valid_badges m"
-  using valid ..
+context Arch_mdb_empty begin
 
 lemma valid_badges_n:
   "valid_badges n"
@@ -485,6 +91,7 @@ proof -
   from valid_badges
   show ?thesis
     supply if_cong[cong]
+    supply to_slot_eq[simp del]
     apply (simp add: valid_badges_def2)
     apply clarsimp
     apply (rule conjI)
@@ -552,14 +159,6 @@ proof -
     done
 qed
 
-lemma to_slot_eq [simp]:
-  "m \<turnstile> p \<leadsto> slot = (p = mdbPrev s_node \<and> p \<noteq> 0)"
-  apply (rule iffI)
-   apply (frule dlist_nextD0, simp)
-   apply (clarsimp simp: mdb_prev_def slot mdb_next_unfold)
-  apply (clarsimp intro!: prev_slot_next)
-  done
-
 lemma n_parent_of:
   "\<lbrakk> n \<turnstile> p parentOf p'; p \<noteq> slot; p' \<noteq> slot \<rbrakk> \<Longrightarrow> m \<turnstile> p parentOf p'"
   supply if_cong[cong]
@@ -590,11 +189,8 @@ lemma m_parent_of:
   apply (frule_tac p=p' in m_badged)
   apply (drule_tac p=p' in m_revokable)
   apply clarsimp
-  apply (simp split: if_split_asm;
-         clarsimp simp: isMDBParentOf_def isArchMDBParentOf_def2 isCap_simps
-                  split: if_split_asm
-                  cong: if_cong)
-  done
+  by (fastforce simp: isMDBParentOf_def isArchMDBParentOf_def2 isCap_simps
+                split: if_split_asm)
 
 lemma m_parent_of_next:
   "\<lbrakk> m \<turnstile> p parentOf mdbNext s_node; m \<turnstile> p parentOf slot; p \<noteq> slot; p\<noteq>mdbNext s_node \<rbrakk>
@@ -614,30 +210,6 @@ lemma m_parent_of_next:
   apply (drule_tac p="slot" in m_revokable)
   by (auto simp: isMDBParentOf_def isArchMDBParentOf_def2 isCap_simps
            split: if_split_asm cong: if_cong)
-
-lemma n_mdbNext:
-  "\<lbrakk> n (mdbNext s_node) = Some (CTE cap node); mdbPrev s_node \<noteq> 0 \<rbrakk> \<Longrightarrow>
-  \<exists>node'. m (mdbNext s_node) = Some (CTE cap node') \<and>
-          mdbNext node = mdbNext node' \<and>
-          mdbPrev node = mdbPrev s_node \<and>
-          mdbRevocable node = mdbRevocable node' \<and>
-          (mdbFirstBadged node = mdbFirstBadged node' \<or> mdbFirstBadged s_node)"
-  apply (clarsimp simp: n_def modify_map_def)
-  apply (case_tac z)
-  apply clarsimp
-  done
-
-lemma n_mdbPrev:
-  "\<lbrakk> n (mdbPrev s_node) = Some (CTE cap node); mdbNext s_node \<noteq> 0 \<rbrakk> \<Longrightarrow>
-    \<exists>node'. m (mdbPrev s_node) = Some (CTE cap node') \<and>
-          mdbNext node = mdbNext s_node \<and>
-          mdbPrev node = mdbPrev node' \<and>
-          mdbRevocable node = mdbRevocable node' \<and>
-          (mdbFirstBadged node = mdbFirstBadged node')"
-  apply (clarsimp simp: n_def modify_map_def)
-  apply (case_tac z)
-  apply clarsimp
-  done
 
 lemma parency_n:
   assumes "n \<turnstile> p \<rightarrow> p'"
@@ -698,13 +270,16 @@ proof induct
      apply (case_tac cap'', simp_all add: isCap_simps)[1]
       apply (clarsimp simp: sameRegionAs_def3 isCap_simps)
      apply (clarsimp simp: sameRegionAs_def3 isCap_simps)
+     apply (rename_tac acap'')
+     apply (case_tac acap''; clarsimp simp: sameRegionAs_def3 isCap_simps)
     (* SGISignalCap *)
-    apply (clarsimp simp: parentOf_def isCap_simps isMDBParentOf_CTE arch_capBadge_def)
+    apply (clarsimp simp: parentOf_def isCap_simps isMDBParentOf_CTE)
     apply (rename_tac next_node)
     apply (rule subtree.trans_parent[OF _ m_slot_next], simp_all)
      apply (rule subtree.direct_parent)
        apply (erule prev_slot_next)
       apply simp
+     prefer 2
      apply (clarsimp simp: parentOf_def slot isMDBParentOf_CTE)
     apply (clarsimp simp: parentOf_def slot isMDBParentOf_CTE isCap_simps)
     apply (cases "mdbFirstBadged s_node", simp)
@@ -796,9 +371,11 @@ next
         apply (case_tac cap'', simp_all add: isCap_simps)[1]
          apply (clarsimp simp: sameRegionAs_def3 isCap_simps)
         apply (clarsimp simp: sameRegionAs_def3 isCap_simps)
+        apply (rename_tac acap'')
+        apply (case_tac acap''; clarsimp simp: sameRegionAs_def3 isCap_simps)
        (* SGISignalCap *)
        apply (rename_tac next_cap next_node)
-       apply (clarsimp simp: isCap_simps arch_capBadge_def)
+       apply (clarsimp simp: isCap_simps)
        apply (case_tac cte, case_tac cte')
        apply (rename_tac cap'' node'')
        apply (clarsimp simp: isMDBParentOf_CTE)
@@ -816,1106 +393,115 @@ next
     done
 qed
 
-lemma parency_m:
-  assumes "m \<turnstile> p \<rightarrow> p'"
-  shows "p \<noteq> slot \<longrightarrow> (if p' \<noteq> slot then n \<turnstile> p \<rightarrow> p' else m \<turnstile> p \<rightarrow> mdbNext s_node \<longrightarrow> n \<turnstile> p \<rightarrow> mdbNext s_node)"
-using assms
-proof induct
-  case (direct_parent c)
-  thus ?case
-    apply clarsimp
-    apply (rule conjI)
-     apply clarsimp
-     apply (rule subtree.direct_parent)
-       apply (simp add: n_next_eq)
-       apply clarsimp
-       apply (subgoal_tac "mdbPrev s_node \<noteq> 0")
-        prefer 2
-        apply (clarsimp simp: mdb_next_unfold)
-       apply (drule prev_slot_next)
-       apply (clarsimp simp: mdb_next_unfold)
-      apply assumption
-     apply (erule m_parent_of, simp, simp)
-      apply clarsimp
-     apply clarsimp
-     apply (drule dlist_next_src_unique)
-       apply fastforce
-      apply clarsimp
-     apply simp
-    apply clarsimp
-    apply (rule subtree.direct_parent)
-      apply (simp add: n_next_eq)
-     apply (drule subtree_parent)
-     apply (clarsimp simp: parentOf_def)
-    apply (drule subtree_parent)
-    apply (erule (1) m_parent_of_next)
-     apply clarsimp
-    apply clarsimp
-    done
-next
-  case (trans_parent c c')
-  thus ?case
-    apply clarsimp
-    apply (rule conjI)
-     apply clarsimp
-     apply (cases "c=slot")
-      apply simp
-      apply (erule impE)
-       apply (erule subtree.trans_parent)
-         apply fastforce
-        apply (clarsimp simp: slot mdb_next_unfold)
-       apply (clarsimp simp: slot mdb_next_unfold)
-      apply (clarsimp simp: slot mdb_next_unfold)
-     apply clarsimp
-     apply (erule subtree.trans_parent)
-       apply (simp add: n_next_eq)
-       apply clarsimp
-       apply (subgoal_tac "mdbPrev s_node \<noteq> 0")
-        prefer 2
-        apply (clarsimp simp: mdb_next_unfold)
-       apply (drule prev_slot_next)
-       apply (clarsimp simp: mdb_next_unfold)
-      apply assumption
-     apply (erule m_parent_of, simp, simp)
-      apply clarsimp
-      apply (drule subtree_mdb_next)
-      apply (drule trancl_trans)
-       apply (erule r_into_trancl)
-      apply simp
-     apply clarsimp
-     apply (drule dlist_next_src_unique)
-       apply fastforce
-      apply clarsimp
-     apply simp
-    apply clarsimp
-    apply (erule subtree.trans_parent)
-      apply (simp add: n_next_eq)
-     apply clarsimp
-    apply (rule m_parent_of_next, erule subtree_parent, assumption, assumption)
-    apply clarsimp
-    done
+end (* Arch_mdb_empty *)
+
+context mdb_empty begin
+
+lemmas gen_arch_assms =
+  Arch_mdb_empty.valid_badges_n
+  Arch_mdb_empty.parency_n
+  Arch_mdb_empty.m_parent_of
+  Arch_mdb_empty.m_parent_of_next
+
+(* extract arch-dependent assumptions of mdb_empty_gen proved in Arch_mdb_empty
+   (faster than interpreting Arch) *)
+lemmas gen_assms = gen_arch_assms[unfolded Arch_mdb_empty_def, OF mdb_empty_axioms]
+
+sublocale mdb_empty_gen
+  by (unfold_locales)
+     (blast intro!: gen_assms)+
+
+(* re-bind names *)
+lemmas vmdb_n = vmdb_n
+lemmas descendants = descendants
+
+end (* mdb_empty *)
+
+interpretation Finalise_R?: Finalise_R arch_final_matters' arch_cap_has_cleanup'
+proof goal_cases
+  interpret Arch  .
+  case 1 show ?case by (intro_locales; (unfold_locales; (fact Finalise_R_assms)?)?)
 qed
 
-lemma parency:
-  "n \<turnstile> p \<rightarrow> p' = (p \<noteq> slot \<and> p' \<noteq> slot \<and> m \<turnstile> p \<rightarrow> p')"
-  by (auto dest!: parency_n parency_m)
+context Arch begin arch_global_naming
 
-lemma descendants:
-  "descendants_of' p n =
-  (if p = slot then {} else descendants_of' p m - {slot})"
-  by (auto simp add: parency descendants_of'_def)
+named_theorems Finalise_R_2_assms
 
-lemma n_tranclD:
-  "n \<turnstile> p \<leadsto>\<^sup>+ p' \<Longrightarrow> m \<turnstile> p \<leadsto>\<^sup>+ p' \<and> p' \<noteq> slot"
-  apply (erule trancl_induct)
-   apply (clarsimp simp add: n_next_eq split: if_split_asm)
-     apply (rule mdb_chain_0D)
-      apply (rule chain)
-     apply (clarsimp simp: slot)
-    apply (blast intro: trancl_trans prev_slot_next)
-   apply fastforce
-  apply (clarsimp simp: n_next_eq split: if_split_asm)
-   apply (erule trancl_trans)
-   apply (blast intro: trancl_trans prev_slot_next)
-  apply (fastforce intro: trancl_trans)
-  done
-
-lemma m_tranclD:
-  "m \<turnstile> p \<leadsto>\<^sup>+ p' \<Longrightarrow>
-  if p = slot then n \<turnstile> mdbNext s_node \<leadsto>\<^sup>* p'
-  else if p' = slot then n \<turnstile> p \<leadsto>\<^sup>+ mdbNext s_node
-  else n \<turnstile> p \<leadsto>\<^sup>+ p'"
-  using no_0_n
-  apply -
-  apply (erule trancl_induct)
-   apply clarsimp
-   apply (rule conjI)
-    apply clarsimp
-    apply (rule r_into_trancl)
-    apply (clarsimp simp: n_next_eq)
-   apply clarsimp
-   apply (rule conjI)
-    apply (insert m_slot_next)[1]
-    apply (clarsimp simp: mdb_next_unfold)
-   apply clarsimp
-   apply (rule r_into_trancl)
-   apply (clarsimp simp: n_next_eq)
-   apply (rule context_conjI)
-    apply (clarsimp simp: mdb_next_unfold)
-   apply (drule prev_slot_next)
-   apply (clarsimp simp: mdb_next_unfold)
-  apply clarsimp
-  apply (rule conjI)
-   apply clarsimp
-   apply (rule conjI)
-    apply clarsimp
-    apply (drule prev_slot_next)
-    apply (drule trancl_trans, erule r_into_trancl)
-    apply simp
-   apply clarsimp
-   apply (erule trancl_trans)
-   apply (rule r_into_trancl)
-   apply (simp add: n_next_eq)
-  apply clarsimp
-  apply (rule conjI)
-   apply clarsimp
-   apply (erule rtrancl_trans)
-   apply (rule r_into_rtrancl)
-   apply (simp add: n_next_eq)
-   apply (rule conjI)
-    apply clarsimp
-    apply (rule context_conjI)
-     apply (clarsimp simp: mdb_next_unfold)
-    apply (drule prev_slot_next)
-    apply (clarsimp simp: mdb_next_unfold)
-   apply clarsimp
-  apply clarsimp
-  apply (simp split: if_split_asm)
-   apply (clarsimp simp: mdb_next_unfold slot)
-  apply (erule trancl_trans)
-  apply (rule r_into_trancl)
-  apply (clarsimp simp add: n_next_eq)
-  apply (rule context_conjI)
-   apply (clarsimp simp: mdb_next_unfold)
-  apply (drule prev_slot_next)
-  apply (clarsimp simp: mdb_next_unfold)
-  done
-
-lemma n_trancl_eq:
-  "n \<turnstile> p \<leadsto>\<^sup>+ p' = (m \<turnstile> p \<leadsto>\<^sup>+ p' \<and> (p = slot \<longrightarrow> p' = 0) \<and> p' \<noteq> slot)"
-  using no_0_n
-  apply -
-  apply (rule iffI)
-   apply (frule n_tranclD)
-   apply clarsimp
-   apply (drule tranclD)
-   apply (clarsimp simp: n_next_eq)
-   apply (simp add: rtrancl_eq_or_trancl)
-  apply clarsimp
-  apply (drule m_tranclD)
-  apply (simp split: if_split_asm)
-  apply (rule r_into_trancl)
-  apply (simp add: n_next_eq)
-  done
-
-lemma n_rtrancl_eq:
-  "n \<turnstile> p \<leadsto>\<^sup>* p' =
-  (m \<turnstile> p \<leadsto>\<^sup>* p' \<and>
-   (p = slot \<longrightarrow> p' = 0 \<or> p' = slot) \<and>
-   (p' = slot \<longrightarrow> p = slot))"
-  by (auto simp: rtrancl_eq_or_trancl n_trancl_eq)
-
-lemma mdb_chain_0_n:
-  "mdb_chain_0 n"
-  using chain
-  apply (clarsimp simp: mdb_chain_0_def)
-  apply (drule bspec)
-   apply (fastforce simp: n_def modify_map_if split: if_split_asm)
-  apply (simp add: n_trancl_eq)
-  done
-
-lemma mdb_chunked_n:
-  "mdb_chunked n"
-  using chunked
-  apply (clarsimp simp: mdb_chunked_def)
-  apply (drule n_cap)+
-  apply (clarsimp split: if_split_asm)
-  apply (case_tac "p=slot", clarsimp)
-  apply clarsimp
-  apply (erule_tac x=p in allE)
-  apply (erule_tac x=p' in allE)
-  apply (clarsimp simp: is_chunk_def)
-  apply (simp add: n_trancl_eq n_rtrancl_eq)
-  apply (rule conjI)
-   apply clarsimp
-   apply (erule_tac x=p'' in allE)
-   apply clarsimp
-   apply (drule_tac p=p'' in m_cap)
-   apply clarsimp
-  apply clarsimp
-  apply (erule_tac x=p'' in allE)
-  apply clarsimp
-  apply (drule_tac p=p'' in m_cap)
-  apply clarsimp
-  done
-
-lemma untyped_mdb_n:
-  "untyped_mdb' n"
-  using untyped_mdb
-  apply (simp add: untyped_mdb'_def descendants_of'_def parency)
-  apply clarsimp
-  apply (drule n_cap)+
-  apply (clarsimp split: if_split_asm)
-  apply (case_tac "p=slot", simp)
-  apply clarsimp
-  done
-
-lemma untyped_inc_n:
-  "untyped_inc' n"
-  using untyped_inc
-  apply (simp add: untyped_inc'_def descendants_of'_def parency)
-  apply clarsimp
-  apply (drule n_cap)+
-  apply (clarsimp split: if_split_asm)
-  apply (case_tac "p=slot", simp)
-  apply clarsimp
-  apply (erule_tac x=p in allE)
-  apply (erule_tac x=p' in allE)
-  apply simp
-  done
-
-lemmas vn_prev [dest!] = valid_nullcaps_prev [OF _ slot no_0 dlist nullcaps]
-lemmas vn_next [dest!] = valid_nullcaps_next [OF _ slot no_0 dlist nullcaps]
-
-lemma nullcaps_n: "valid_nullcaps n"
-proof -
-  from valid have "valid_nullcaps m" ..
-  thus ?thesis
-    apply (clarsimp simp: valid_nullcaps_def nullMDBNode_def nullPointer_def)
-    apply (frule n_cap)
-    apply (frule n_next)
-    apply (frule n_badged)
-    apply (frule n_revokable)
-    apply (drule n_prev)
-    apply (case_tac n)
-    apply (insert slot)
-    apply (fastforce split: if_split_asm)
-    done
-qed
-
-lemma ut_rev_n: "ut_revocable' n"
-  apply(insert valid)
-  apply(clarsimp simp: ut_revocable'_def)
-  apply(frule n_cap)
-  apply(drule n_revokable)
-  apply(clarsimp simp: isCap_simps split: if_split_asm)
-  apply(simp add: valid_mdb_ctes_def ut_revocable'_def)
-  done
-
-lemma class_links_n: "class_links n"
-  using valid slot
-  apply (clarsimp simp: valid_mdb_ctes_def class_links_def)
-  apply (case_tac cte, case_tac cte')
-  apply (drule n_nextD)
-  apply (clarsimp simp: split: if_split_asm)
-    apply (simp add: no_0_n)
-   apply (drule n_cap)+
-   apply clarsimp
-   apply (frule spec[where x=slot],
-          drule spec[where x="mdbNext s_node"],
-          simp, simp add: m_slot_next)
-   apply (drule spec[where x="mdbPrev s_node"],
-          drule spec[where x=slot], simp)
-  apply (drule n_cap)+
-  apply clarsimp
-  apply (fastforce split: if_split_asm)
-  done
-
-lemma distinct_zombies_m: "distinct_zombies m"
-  using valid by (simp add: valid_mdb_ctes_def)
-
-lemma distinct_zombies_n[simp]:
-  "distinct_zombies n"
-  using distinct_zombies_m
-  apply (simp add: n_def distinct_zombies_nonCTE_modify_map)
-  apply (subst modify_map_apply[where p=slot])
-   apply (simp add: modify_map_def slot)
-  apply simp
-  apply (rule distinct_zombies_sameMasterE)
-    apply (simp add: distinct_zombies_nonCTE_modify_map)
-   apply (simp add: modify_map_def slot)
-  apply simp
-  done
-
-lemma irq_control_n [simp]: "irq_control n"
-  using slot
-  apply (clarsimp simp: irq_control_def)
-  apply (frule n_revokable)
-  apply (drule n_cap)
-  apply (clarsimp split: if_split_asm)
-  apply (frule irq_revocable, rule irq_control)
-  apply clarsimp
-  apply (drule n_cap)
-  apply (clarsimp simp: if_split_asm)
-  apply (erule (1) irq_controlD, rule irq_control)
-  done
-
-lemma reply_masters_rvk_fb_m: "reply_masters_rvk_fb m"
-  using valid by auto
-
-lemma reply_masters_rvk_fb_n [simp]: "reply_masters_rvk_fb n"
-  using reply_masters_rvk_fb_m
-  apply (simp add: reply_masters_rvk_fb_def n_def
-                   ball_ran_modify_map_eq
-                   modify_map_comp[symmetric])
-  apply (subst ball_ran_modify_map_eq)
-   apply (frule bspec, rule ranI, rule slot)
-   apply (simp add: nullMDBNode_def isCap_simps modify_map_def
-                    slot)
-  apply (subst ball_ran_modify_map_eq)
-   apply (clarsimp simp add: modify_map_def)
-   apply fastforce
-  apply (simp add: ball_ran_modify_map_eq)
-  done
-
-lemma vmdb_n: "valid_mdb_ctes n"
-  by (simp add: valid_mdb_ctes_def valid_dlist_n
-                no_0_n mdb_chain_0_n valid_badges_n
-                caps_contained_n mdb_chunked_n
-                untyped_mdb_n untyped_inc_n
-                nullcaps_n ut_rev_n class_links_n)
-
-end
-
-context begin interpretation Arch .
-crunch postCapDeletion, clearUntypedFreeIndex
-  for ctes_of[wp]: "\<lambda>s. P (ctes_of s)"
-
-lemma emptySlot_mdb [wp]:
-  "\<lbrace>valid_mdb'\<rbrace>
-  emptySlot sl opt
-  \<lbrace>\<lambda>_. valid_mdb'\<rbrace>"
-  unfolding emptySlot_def
-  apply (simp only: case_Null_If valid_mdb'_def)
-  apply (wp updateCap_ctes_of_wp getCTE_wp'
-            opt_return_pres_lift | simp add: cte_wp_at_ctes_of)+
-  apply (clarsimp)
-  apply (case_tac cte)
-  apply (rename_tac cap node)
-  apply (simp)
-  apply (subgoal_tac "mdb_empty (ctes_of s) sl cap node")
-   prefer 2
-   apply (rule mdb_empty.intro)
-   apply (rule mdb_ptr.intro)
-    apply (rule vmdb.intro)
-    apply (simp add: valid_mdb_ctes_def)
-   apply (rule mdb_ptr_axioms.intro)
-   apply (simp add: cte_wp_at_ctes_of)
-  apply (rule conjI, clarsimp simp: valid_mdb_ctes_def)
-  apply (erule mdb_empty.vmdb_n[unfolded const_def])
-  done
-end
-
-lemma if_live_then_nonz_cap'_def2:
-  "if_live_then_nonz_cap' = (\<lambda>s. \<forall>ptr. ko_wp_at' live' ptr s
-                               \<longrightarrow> (\<exists>p zr. (option_map zobj_refs' o cteCaps_of s) p = Some zr \<and> ptr \<in> zr))"
-  by (fastforce intro!: ext
-                 simp: if_live_then_nonz_cap'_def ex_nonz_cap_to'_def
-                       cte_wp_at_ctes_of cteCaps_of_def)
-
-lemma updateMDB_ko_wp_at_live[wp]:
-  "\<lbrace>\<lambda>s. P (ko_wp_at' live' p' s)\<rbrace>
-      updateMDB p m
-   \<lbrace>\<lambda>rv s. P (ko_wp_at' live' p' s)\<rbrace>"
-  unfolding updateMDB_def Let_def
-  apply (rule hoare_pre, wp)
-  apply simp
-  done
-
-lemma updateCap_ko_wp_at_live[wp]:
-  "\<lbrace>\<lambda>s. P (ko_wp_at' live' p' s)\<rbrace>
-      updateCap p cap
-   \<lbrace>\<lambda>rv s. P (ko_wp_at' live' p' s)\<rbrace>"
-  unfolding updateCap_def
-  by wp
-
-primrec
-  threadCapRefs :: "capability \<Rightarrow> word32 set"
-where
-  "threadCapRefs (ThreadCap r)                  = {r}"
-| "threadCapRefs (ReplyCap t m x)               = {}"
-| "threadCapRefs NullCap                        = {}"
-| "threadCapRefs (UntypedCap d r n i)           = {}"
-| "threadCapRefs (EndpointCap r badge x y z t)  = {}"
-| "threadCapRefs (NotificationCap r badge x y)  = {}"
-| "threadCapRefs (CNodeCap r b g gsz)           = {}"
-| "threadCapRefs (Zombie r b n)                 = {}"
-| "threadCapRefs (ArchObjectCap ac)             = {}"
-| "threadCapRefs (IRQHandlerCap irq)            = {}"
-| "threadCapRefs (IRQControlCap)                = {}"
-| "threadCapRefs (DomainCap)                    = {}"
-
-definition
-  "isFinal cap p m \<equiv>
-  \<not>isUntypedCap cap \<and>
-  (\<forall>p' c. m p' = Some c \<longrightarrow>
-          p \<noteq> p' \<longrightarrow> \<not>isUntypedCap c \<longrightarrow>
-          \<not> sameObjectAs cap c)"
-
-lemma not_FinalE:
-  "\<lbrakk> \<not> isFinal cap sl cps; isUntypedCap cap \<Longrightarrow> P;
-     \<And>p c. \<lbrakk> cps p = Some c; p \<noteq> sl; \<not> isUntypedCap c; sameObjectAs cap c \<rbrakk> \<Longrightarrow> P
-    \<rbrakk> \<Longrightarrow> P"
-  by (fastforce simp: isFinal_def)
-
-definition
- "removeable' sl \<equiv> \<lambda>s cap.
-    (\<exists>p. p \<noteq> sl \<and> cte_wp_at' (\<lambda>cte. capMasterCap (cteCap cte) = capMasterCap cap) p s)
-    \<or> ((\<forall>p \<in> cte_refs' cap (irq_node' s). p \<noteq> sl \<longrightarrow> cte_wp_at' (\<lambda>cte. cteCap cte = NullCap) p s)
-         \<and> (\<forall>p \<in> zobj_refs' cap. ko_wp_at' (Not \<circ> live') p s))"
-
-lemma not_Final_removeable:
-  "\<not> isFinal cap sl (cteCaps_of s)
-    \<Longrightarrow> removeable' sl s cap"
+lemma not_Final_removeable[Finalise_R_2_assms]:
+  "\<not> isFinal cap sl (cteCaps_of s) \<Longrightarrow> removeable' sl s cap"
   apply (erule not_FinalE)
    apply (clarsimp simp: removeable'_def gen_isCap_simps)
   apply (clarsimp simp: cteCaps_of_def ARM.sameObjectAs_def2 removeable'_def
-                        cte_wp_at_ctes_of) (* FIXME arch-split *)
+                        cte_wp_at_ctes_of)
   apply fastforce
   done
 
-context begin interpretation Arch .
-crunch postCapDeletion
-  for ko_wp_at'[wp]: "\<lambda>s. P (ko_wp_at' P' p s)"
-crunch postCapDeletion
-  for cteCaps_of[wp]: "\<lambda>s. P (cteCaps_of s)"
-  (simp: cteCaps_of_def o_def)
-end
-
-crunch clearUntypedFreeIndex
-  for ko_at_live[wp]: "\<lambda>s. P (ko_wp_at' live' ptr s)"
-
-lemma clearUntypedFreeIndex_cteCaps_of[wp]:
-  "\<lbrace>\<lambda>s. P (cteCaps_of s)\<rbrace>
-       clearUntypedFreeIndex sl \<lbrace>\<lambda>y s. P (cteCaps_of s)\<rbrace>"
-  by (simp add: cteCaps_of_def, wp)
-
-lemma emptySlot_iflive'[wp]:
-  "\<lbrace>\<lambda>s. if_live_then_nonz_cap' s \<and> cte_wp_at' (\<lambda>cte. removeable' sl s (cteCap cte)) sl s\<rbrace>
-     emptySlot sl opt
-   \<lbrace>\<lambda>rv. if_live_then_nonz_cap'\<rbrace>"
-  apply (simp add: emptySlot_def case_Null_If if_live_then_nonz_cap'_def2
-              del: comp_apply)
+lemma deletedIRQHandler_valid_global_refs[Finalise_R_2_assms, wp]:
+  "\<lbrace>valid_global_refs'\<rbrace> deletedIRQHandler irq \<lbrace>\<lambda>rv. valid_global_refs'\<rbrace>"
+  apply (clarsimp simp: valid_global_refs'_def global_refs'_def)
   apply (rule hoare_pre)
-   apply (wp hoare_vcg_all_lift hoare_vcg_disj_lift
-             getCTE_wp opt_return_pres_lift
-             clearUntypedFreeIndex_ctes_of
-             clearUntypedFreeIndex_cteCaps_of
-             hoare_vcg_ex_lift
-             | wp (once) hoare_vcg_imp_lift
-             | simp add: cte_wp_at_ctes_of del: comp_apply)+
-  apply (clarsimp simp: modify_map_same
-    imp_conjR[symmetric])
-  apply (drule spec, drule(1) mp)
-  apply (clarsimp simp: cte_wp_at_ctes_of modify_map_def split: if_split_asm)
-  apply (case_tac "p \<noteq> sl")
-   apply blast
-  apply (simp add: removeable'_def cteCaps_of_def)
-  apply (erule disjE)
-   apply (clarsimp simp: cte_wp_at_ctes_of modify_map_def
-                  dest!: capMaster_same_refs)
-   apply fastforce
-  apply clarsimp
-  apply (drule(1) bspec)
-  apply (clarsimp simp: ko_wp_at'_def)
-  done
-
-lemma setIRQState_irq_node'[wp]:
-  "\<lbrace>\<lambda>s. P (irq_node' s)\<rbrace> setIRQState state irq \<lbrace>\<lambda>_ s. P (irq_node' s)\<rbrace>"
-  apply (simp add: setIRQState_def setInterruptState_def getInterruptState_def)
-  apply wp
-  apply simp
-  done
-
-context begin interpretation Arch .
-crunch emptySlot
-  for irq_node'[wp]: "\<lambda>s. P (irq_node' s)"
-end
-
-lemma emptySlot_ifunsafe'[wp]:
-  "\<lbrace>\<lambda>s. if_unsafe_then_cap' s \<and> cte_wp_at' (\<lambda>cte. removeable' sl s (cteCap cte)) sl s\<rbrace>
-     emptySlot sl opt
-   \<lbrace>\<lambda>rv. if_unsafe_then_cap'\<rbrace>"
-  apply (simp add: ifunsafe'_def3)
-  apply (rule hoare_pre, rule hoare_use_eq_irq_node'[OF emptySlot_irq_node'])
-   apply (simp add: emptySlot_def case_Null_If)
-   apply (wp opt_return_pres_lift | simp add: o_def)+
-   apply (wp getCTE_cteCap_wp clearUntypedFreeIndex_cteCaps_of)+
-  apply (clarsimp simp: tree_cte_cteCap_eq[unfolded o_def]
-                        modify_map_same
-                        modify_map_comp[symmetric]
-                 split: option.split_asm if_split_asm
-                 dest!: modify_map_K_D)
-  apply (clarsimp simp: modify_map_def)
-  apply (drule_tac x=cref in spec, clarsimp)
-  apply (case_tac "cref' \<noteq> sl")
-   apply (rule_tac x=cref' in exI)
-   apply (clarsimp simp: modify_map_def)
-  apply (simp add: removeable'_def)
-  apply (erule disjE)
-   apply (clarsimp simp: modify_map_def)
-   apply (subst(asm) tree_cte_cteCap_eq[unfolded o_def])
-   apply (clarsimp split: option.split_asm dest!: capMaster_same_refs)
-   apply fastforce
-  apply clarsimp
-  apply (drule(1) bspec)
-  apply (clarsimp simp: cte_wp_at_ctes_of cteCaps_of_def)
-  done
-
-lemma ctes_of_valid'[elim]:
-  "\<lbrakk>ctes_of s p = Some cte; valid_objs' s\<rbrakk> \<Longrightarrow> s \<turnstile>' cteCap cte"
-  by (cases cte, simp) (rule ctes_of_valid_cap')
-
-crunch setInterruptState
-  for valid_idle'[wp]: "valid_idle'"
-  (simp: valid_idle'_def)
-
-context begin interpretation Arch .
-crunch emptySlot
-  for valid_idle'[wp]: "valid_idle'"
-
-crunch emptySlot
-  for ksArch[wp]: "\<lambda>s. P (ksArchState s)"
-crunch emptySlot
-  for ksIdle[wp]: "\<lambda>s. P (ksIdleThread s)"
-crunch emptySlot
-  for gsMaxObjectSize[wp]: "\<lambda>s. P (gsMaxObjectSize s)"
-end
-
-lemma emptySlot_cteCaps_of:
-  "\<lbrace>\<lambda>s. P ((cteCaps_of s)(p \<mapsto> NullCap))\<rbrace>
-     emptySlot p opt
-   \<lbrace>\<lambda>rv s. P (cteCaps_of s)\<rbrace>"
-  apply (simp add: emptySlot_def case_Null_If)
-  apply (wp opt_return_pres_lift getCTE_cteCap_wp
-            clearUntypedFreeIndex_cteCaps_of)
-  apply (clarsimp simp: cteCaps_of_def cte_wp_at_ctes_of)
-  apply (auto elim!: rsubst[where P=P]
-               simp: modify_map_def fun_upd_def[symmetric] o_def
-                     fun_upd_idem cteCaps_of_def
-              split: option.splits)
-  done
-
-lemma emptySlot_valid_global_refs[wp]:
-  "\<lbrace>valid_global_refs' and cte_at' sl\<rbrace> emptySlot sl opt \<lbrace>\<lambda>rv. valid_global_refs'\<rbrace>"
-  apply (simp add: valid_global_refs'_def ARM.global_refs'_def)
-  apply (rule hoare_pre)
-   apply (rule hoare_use_eq_irq_node' [OF emptySlot_irq_node'])
-   apply (rule hoare_use_eq [where f=ksArchState, OF emptySlot_ksArch])
-   apply (rule hoare_use_eq [where f=ksIdleThread, OF emptySlot_ksIdle])
-   apply (rule hoare_use_eq [where f=gsMaxObjectSize], wp)
+   apply (rule hoare_use_eq_irq_node' [OF deletedIRQHandler_irq_node'])
+   apply (rule hoare_use_eq [where f=ksIdleThread, OF deletedIRQHandler_ksIdle])
+   apply (rule hoare_use_eq [where f=ksArchState, OF deletedIRQHandler_ksArch])
+   apply (rule hoare_use_eq[where f="gsMaxObjectSize"], wp)
    apply (simp add: valid_refs'_cteCaps valid_cap_sizes_cteCaps)
-   apply (rule emptySlot_cteCaps_of)
+   apply (rule deletedIRQHandler_cteCaps_of)
   apply (clarsimp simp: cte_wp_at_ctes_of)
-  apply (frule(1) cte_at_valid_cap_sizes_0)
   apply (clarsimp simp: valid_refs'_cteCaps valid_cap_sizes_cteCaps ball_ran_eq)
   done
 
-lemmas doMachineOp_irq_handlers[wp]
-    = valid_irq_handlers_lift'' [OF doMachineOp_ctes doMachineOp_ksInterruptState]
-
-lemma deletedIRQHandler_irq_handlers'[wp]:
-  "\<lbrace>\<lambda>s. valid_irq_handlers' s \<and> (IRQHandlerCap irq \<notin> ran (cteCaps_of s))\<rbrace>
-       deletedIRQHandler irq
-   \<lbrace>\<lambda>rv. valid_irq_handlers'\<rbrace>"
-  apply (simp add: deletedIRQHandler_def setIRQState_def setInterruptState_def getInterruptState_def)
-  apply wp
-  apply (clarsimp simp: valid_irq_handlers'_def irq_issued'_def ran_def cteCaps_of_def)
-  done
-
-context begin interpretation Arch .
-
-lemma postCapDeletion_irq_handlers'[wp]:
-  "\<lbrace>\<lambda>s. valid_irq_handlers' s \<and> (cap \<noteq> NullCap \<longrightarrow> cap \<notin> ran (cteCaps_of s))\<rbrace>
-       postCapDeletion cap
-   \<lbrace>\<lambda>rv. valid_irq_handlers'\<rbrace>"
-  by (wpsimp simp: Retype_H.postCapDeletion_def ARM_H.postCapDeletion_def)
-
-end
-
-crunch clearUntypedFreeIndex
-  for ksInterruptState[wp]: "\<lambda>s. P (ksInterruptState s)"
-
-lemma emptySlot_valid_irq_handlers'[wp]:
-  "\<lbrace>\<lambda>s. valid_irq_handlers' s
-          \<and> (\<forall>sl'. info \<noteq> NullCap \<longrightarrow> sl' \<noteq> sl \<longrightarrow> cteCaps_of s sl' \<noteq> Some info)\<rbrace>
-     emptySlot sl info
-   \<lbrace>\<lambda>rv. valid_irq_handlers'\<rbrace>"
-  apply (simp add: emptySlot_def case_Null_If)
-  apply (wp | wpc)+
-        apply (unfold valid_irq_handlers'_def irq_issued'_def)
-        apply (wp getCTE_cteCap_wp clearUntypedFreeIndex_cteCaps_of
-          | wps clearUntypedFreeIndex_ksInterruptState)+
-  apply (clarsimp simp: cteCaps_of_def cte_wp_at_ctes_of ran_def modify_map_def
-                 split: option.split)
-  apply auto
-  done
-
-context begin interpretation Arch .
-crunch emptySlot
-  for irq_states'[wp]: valid_irq_states'
-
-crunch emptySlot
-  for no_0_obj'[wp]: no_0_obj'
- (wp: crunch_wps)
-
-crunch emptySlot
-  for pde_mappings'[wp]: "valid_pde_mappings'"
-
-lemma deletedIRQHandler_irqs_masked'[wp]:
-  "\<lbrace>irqs_masked'\<rbrace> deletedIRQHandler irq \<lbrace>\<lambda>_. irqs_masked'\<rbrace>"
-  apply (simp add: deletedIRQHandler_def setIRQState_def getInterruptState_def setInterruptState_def)
-  apply (wp dmo_maskInterrupt)
-  apply (simp add: irqs_masked'_def)
-  done
-
-crunch emptySlot
-  for irqs_masked'[wp]: "irqs_masked'"
-
-lemma setIRQState_umm:
- "\<lbrace>\<lambda>s. P (underlying_memory (ksMachineState s))\<rbrace>
-   setIRQState irqState irq
-  \<lbrace>\<lambda>_ s. P (underlying_memory (ksMachineState s))\<rbrace>"
-  by (simp add: setIRQState_def maskInterrupt_def
-                setInterruptState_def getInterruptState_def
-      | wp dmo_lift')+
-
-crunch emptySlot
-  for umm[wp]: "\<lambda>s. P (underlying_memory (ksMachineState s))"
-  (wp: setIRQState_umm)
-
-lemma emptySlot_vms'[wp]:
-  "\<lbrace>valid_machine_state'\<rbrace> emptySlot slot irq \<lbrace>\<lambda>_. valid_machine_state'\<rbrace>"
-  by (simp add: valid_machine_state'_def pointerInUserData_def pointerInDeviceData_def)
-     (wp hoare_vcg_all_lift hoare_vcg_disj_lift)
-
-crunch emptySlot
-  for pspace_domain_valid[wp]: "pspace_domain_valid"
-
-crunch emptySlot
-  for ksDomSchedule[wp]: "\<lambda>s. P (ksDomSchedule s)"
-  and ksDomScheduleIdx[wp]: "\<lambda>s. P (ksDomScheduleIdx s)"
-
-lemma deletedIRQHandler_ct_not_inQ[wp]:
-  "\<lbrace>ct_not_inQ\<rbrace> deletedIRQHandler irq \<lbrace>\<lambda>_. ct_not_inQ\<rbrace>"
-  apply (rule ct_not_inQ_lift [OF deletedIRQHandler_nosch])
-  apply (rule hoare_weaken_pre)
-   apply (wps deletedIRQHandler_ct)
-   apply (simp add: deletedIRQHandler_def setIRQState_def)
-   apply (wp)
-  apply (simp add: comp_def)
-  done
-
-crunch emptySlot
-  for ct_not_inQ[wp]: "ct_not_inQ"
-
-crunch emptySlot
-  for tcbDomain[wp]: "obj_at' (\<lambda>tcb. P (tcbDomain tcb)) t"
-
-lemma emptySlot_ct_idle_or_in_cur_domain'[wp]:
-  "\<lbrace>ct_idle_or_in_cur_domain'\<rbrace> emptySlot sl opt \<lbrace>\<lambda>_. ct_idle_or_in_cur_domain'\<rbrace>"
-apply (wp ct_idle_or_in_cur_domain'_lift2 tcb_in_cur_domain'_lift | simp)+
-done
-
-crunch postCapDeletion
-  for gsUntypedZeroRanges[wp]: "\<lambda>s. P (gsUntypedZeroRanges s)"
-  (wp: crunch_wps simp: crunch_simps)
-
-lemma untypedZeroRange_modify_map_isUntypedCap:
-  "m sl = Some v \<Longrightarrow> \<not> isUntypedCap v \<Longrightarrow> \<not> isUntypedCap (f v)
-    \<Longrightarrow> (untypedZeroRange \<circ>\<^sub>m modify_map m sl f) = (untypedZeroRange \<circ>\<^sub>m m)"
-  by (simp add: modify_map_def map_comp_def fun_eq_iff untypedZeroRange_def)
-
-lemma emptySlot_untyped_ranges[wp]:
-  "\<lbrace>untyped_ranges_zero' and valid_objs' and valid_mdb'\<rbrace>
-     emptySlot sl opt \<lbrace>\<lambda>rv. untyped_ranges_zero'\<rbrace>"
-  apply (simp add: emptySlot_def case_Null_If)
+lemma clearUntypedFreeIndex_valid_global_refs[Finalise_R_2_assms, wp]:
+  "\<lbrace>valid_global_refs'\<rbrace> clearUntypedFreeIndex irq \<lbrace>\<lambda>rv. valid_global_refs'\<rbrace>"
+  apply (clarsimp simp: valid_global_refs'_def global_refs'_def)
   apply (rule hoare_pre)
-   apply (rule bind_wp)
-    apply (rule untyped_ranges_zero_lift)
-     apply (wp getCTE_cteCap_wp clearUntypedFreeIndex_cteCaps_of
-       | wpc | simp add: clearUntypedFreeIndex_def updateTrackedFreeIndex_def
-                         getSlotCap_def
-                  split: option.split)+
-  apply (clarsimp simp: modify_map_comp[symmetric] modify_map_same)
-  apply (case_tac "\<not> isUntypedCap (the (cteCaps_of s sl))")
-   apply (case_tac "the (cteCaps_of s sl)",
-     simp_all add: untyped_ranges_zero_inv_def
-                   untypedZeroRange_modify_map_isUntypedCap isCap_simps)[1]
-  apply (clarsimp simp: isCap_simps untypedZeroRange_def modify_map_def)
-  apply (strengthen untyped_ranges_zero_fun_upd[mk_strg I E])
-  apply simp
-  apply (simp add: untypedZeroRange_def isCap_simps)
-  done
-
-crunch emptySlot
-  for valid_bitmaps[wp]: valid_bitmaps
-  and tcbQueued_opt_pred[wp]: "\<lambda>s. P (tcbQueued |< tcbs_of' s)"
-  and valid_sched_pointers[wp]: valid_sched_pointers
-  and sched_projs[wp]: "\<lambda>s. P (tcbSchedNexts_of s) (tcbSchedPrevs_of s)"
-  and valid_arch_state'[wp]: valid_arch_state'
-  and ksDomScheduleStart[wp]: "\<lambda>s. P (ksDomScheduleStart s)"
-  (wp: valid_bitmaps_lift)
-
-lemma emptySlot_invs'[wp]:
-  "\<lbrace>\<lambda>s. invs' s \<and> cte_wp_at' (\<lambda>cte. removeable' sl s (cteCap cte)) sl s
-            \<and> (\<forall>sl'. info \<noteq> NullCap \<longrightarrow> sl' \<noteq> sl \<longrightarrow> cteCaps_of s sl' \<noteq> Some info)\<rbrace>
-     emptySlot sl info
-   \<lbrace>\<lambda>rv. invs'\<rbrace>"
-  apply (simp add: invs'_def valid_state'_def valid_pspace'_def)
-  apply (wp valid_irq_node_lift cur_tcb_lift valid_dom_schedule'_lift)
+   apply (rule hoare_use_eq_irq_node' [OF clearUntypedFreeIndex_irq_node'])
+   apply (rule hoare_use_eq [where f=ksIdleThread, OF clearUntypedFreeIndex_ksIdle])
+   apply (rule hoare_use_eq [where f=ksArchState, OF clearUntypedFreeIndex_ksArch])
+   apply (rule hoare_use_eq[where f="gsMaxObjectSize"], wp)
+   apply (simp add: valid_refs'_cteCaps valid_cap_sizes_cteCaps)
+   apply (rule clearUntypedFreeIndex_cteCaps_of)
   apply (clarsimp simp: cte_wp_at_ctes_of)
+  apply (clarsimp simp: valid_refs'_cteCaps valid_cap_sizes_cteCaps ball_ran_eq)
   done
-
-lemma deletedIRQHandler_corres:
-  "corres dc \<top> \<top>
-    (deleted_irq_handler irq)
-    (deletedIRQHandler irq)"
-  apply (simp add: deleted_irq_handler_def deletedIRQHandler_def)
-  apply (rule setIRQState_corres)
-  apply (simp add: irq_state_relation_def)
-  done
-
-lemma arch_postCapDeletion_corres:
-  "acap_relation cap cap' \<Longrightarrow> corres dc \<top> \<top> (arch_post_cap_deletion cap) (ARM_H.postCapDeletion cap')"
-  by (corresKsimp simp: arch_post_cap_deletion_def ARM_H.postCapDeletion_def)
-
-lemma postCapDeletion_corres:
-  "cap_relation cap cap' \<Longrightarrow> corres dc \<top> \<top> (post_cap_deletion cap) (postCapDeletion cap')"
-  apply (cases cap; clarsimp simp: post_cap_deletion_def Retype_H.postCapDeletion_def)
-   apply (corresKsimp corres: deletedIRQHandler_corres)
-  by (corresKsimp corres: arch_postCapDeletion_corres)
-
-lemma set_cap_trans_state:
-  "((),s') \<in> fst (set_cap c p s) \<Longrightarrow> ((),trans_state f s') \<in> fst (set_cap c p (trans_state f s))"
-  apply (cases p)
-  apply (clarsimp simp add: set_cap_def in_monad set_object_def get_object_def)
-  apply (case_tac y)
-  apply (auto simp add: in_monad set_object_def split: if_split_asm)
-  done
-
-lemma clearUntypedFreeIndex_noop_corres:
-  "corres dc \<top> (cte_at' (cte_map slot))
-    (return ()) (clearUntypedFreeIndex (cte_map slot))"
-  apply (simp add: clearUntypedFreeIndex_def)
-  apply (rule corres_guard_imp)
-    apply (rule corres_bind_return2)
-    apply (rule corres_symb_exec_r_conj[where P'="cte_at' (cte_map slot)"])
-       apply (rule corres_trivial, simp)
-      apply (wp getCTE_wp' | wpc
-        | simp add: updateTrackedFreeIndex_def getSlotCap_def)+
-     apply (clarsimp simp: state_relation_def)
-    apply (rule no_fail_pre)
-     apply (wp no_fail_getSlotCap getCTE_wp'
-       | wpc | simp add: updateTrackedFreeIndex_def getSlotCap_def)+
-  done
-
-lemma clearUntypedFreeIndex_valid_pspace'[wp]:
-  "\<lbrace>valid_pspace'\<rbrace> clearUntypedFreeIndex slot \<lbrace>\<lambda>rv. valid_pspace'\<rbrace>"
-  apply (simp add: valid_pspace'_def)
-  apply (rule hoare_pre)
-   apply (wp | simp add: valid_mdb'_def)+
-  done
-
-lemma emptySlot_corres:
-  "cap_relation info info' \<Longrightarrow> corres dc (einvs and cte_at slot) (invs' and cte_at' (cte_map slot))
-             (empty_slot slot info) (emptySlot (cte_map slot) info')"
-  unfolding emptySlot_def empty_slot_def
-  apply (simp add: case_Null_If)
-  apply (rule corres_guard_imp)
-    apply (rule corres_split_noop_rhs[OF clearUntypedFreeIndex_noop_corres])
-     apply (rule_tac R="\<lambda>cap. einvs and cte_wp_at ((=) cap) slot" and
-                     R'="\<lambda>cte. valid_pspace' and cte_wp_at' ((=) cte) (cte_map slot)" in
-                     corres_split[OF get_cap_corres])
-       defer
-       apply (wp get_cap_wp getCTE_wp')+
-     apply (simp add: cte_wp_at_ctes_of)
-     apply (wp hoare_vcg_imp_lift clearUntypedFreeIndex_valid_pspace')
-    apply fastforce
-   apply (fastforce simp: cte_wp_at_ctes_of)
-  apply simp
-  apply (rule conjI, clarsimp)
-   defer
-  apply clarsimp
-  apply (rule conjI, clarsimp)
-  apply clarsimp
-  apply (simp only: bind_assoc[symmetric])
-  apply (rule corres_underlying_split[where r'=dc, OF _ postCapDeletion_corres])
-    defer
-    apply wpsimp+
-  apply (rule corres_no_failI)
-   apply (rule no_fail_pre, wp hoare_weak_lift_imp)
-   apply (clarsimp simp: cte_wp_at_ctes_of valid_pspace'_def)
-   apply (clarsimp simp: valid_mdb'_def valid_mdb_ctes_def)
-   apply (rule conjI, clarsimp)
-    apply (erule (2) valid_dlistEp)
-    apply simp
-   apply clarsimp
-   apply (erule (2) valid_dlistEn)
-   apply simp
-  apply (clarsimp simp: in_monad bind_assoc exec_gets)
-  apply (subgoal_tac "mdb_empty_abs a")
-   prefer 2
-   apply (rule mdb_empty_abs.intro)
-   apply (rule vmdb_abs.intro)
-   apply fastforce
-  apply (frule mdb_empty_abs'.intro)
-  apply (simp add: mdb_empty_abs'.empty_slot_ext_det_def2 update_cdt_list_def set_cdt_list_def exec_gets set_cdt_def bind_assoc exec_get exec_put set_original_def modify_def del: fun_upd_apply | subst bind_def, simp, simp add: mdb_empty_abs'.empty_slot_ext_det_def2)+
-  apply (simp add: put_def)
-  apply (simp add: exec_gets exec_get exec_put del: fun_upd_apply | subst bind_def)+
-  apply (clarsimp simp: state_relation_def)
-  apply (drule updateMDB_the_lot, fastforce simp: pspace_relation_def, fastforce, fastforce)
-   apply (clarsimp simp: invs'_def valid_state'_def valid_pspace'_def
-                         valid_mdb'_def valid_mdb_ctes_def)
-  apply (elim conjE)
-  apply (drule (4) updateMDB_the_lot, elim conjE)
-  apply clarsimp
-  apply (drule_tac s'=s''a and c=cap.NullCap in set_cap_not_quite_corres)
-                      subgoal by simp
-                     subgoal by simp
-                    subgoal by simp
-                   subgoal by simp
-                  subgoal by fastforce
-                 subgoal by fastforce
-                subgoal by fastforce
-               subgoal by fastforce
-              subgoal by fastforce
-             apply fastforce
-            subgoal by fastforce
-           subgoal by fastforce
-          subgoal by fastforce
-         apply (erule cte_wp_at_weakenE, rule TrueI)
-        apply assumption
-       subgoal by simp
-      subgoal by simp
-     subgoal by simp
-    subgoal by simp
-   apply (rule refl)
-  apply clarsimp
-  apply (drule updateCap_stuff, elim conjE, erule (1) impE)
-  apply clarsimp
-  apply (drule updateMDB_the_lot, force simp: pspace_relation_def, assumption+, simp)
-  apply (rule bexI)
-   prefer 2
-   apply (simp only: trans_state_update[symmetric])
-   apply (rule set_cap_trans_state)
-   apply (rule set_cap_revokable_update)
-   apply (erule set_cap_cdt_update)
-  apply clarsimp
-  apply (thin_tac "ctes_of t = s" for t s)+
-  apply (thin_tac "ksMachineState t = p" for t p)+
-  apply (thin_tac "ksCurThread t = p" for t p)+
-  apply (thin_tac "ksReadyQueues t = p" for t p)+
-  apply (thin_tac "ksSchedulerAction t = p" for t p)+
-  apply (clarsimp simp: cte_wp_at_ctes_of)
-  apply (case_tac rv')
-  apply (rename_tac s_cap s_node)
-  apply (subgoal_tac "cte_at slot a")
-   prefer 2
-   apply (fastforce elim: cte_wp_at_weakenE)
-  apply (subgoal_tac "mdb_empty (ctes_of b) (cte_map slot) s_cap s_node")
-   prefer 2
-   apply (rule mdb_empty.intro)
-   apply (rule mdb_ptr.intro)
-    apply (rule vmdb.intro)
-    subgoal by (simp add: invs'_def valid_state'_def valid_pspace'_def valid_mdb'_def)
-   apply (rule mdb_ptr_axioms.intro)
-   subgoal by simp
-  apply (clarsimp simp: ghost_relation_typ_at set_cap_a_type_inv)
-  apply (simp add: pspace_relation_def)
-  apply (rule conjI)
-   apply (clarsimp simp: data_at_def ghost_relation_typ_at set_cap_a_type_inv)
-  apply (rule conjI)
-   prefer 2
-   apply (rule conjI)
-    apply (clarsimp simp: cdt_list_relation_def)
-    apply(frule invs_valid_pspace, frule invs_mdb)
-    apply(subgoal_tac "no_mloop (cdt a) \<and> finite_depth (cdt a)")
-     prefer 2
-     subgoal by(simp add: finite_depth valid_mdb_def)
-    apply(subgoal_tac "valid_mdb_ctes (ctes_of b)")
-     prefer 2
-     subgoal by(simp add: mdb_empty_def mdb_ptr_def vmdb_def)
-    apply(clarsimp simp: valid_pspace_def)
-
-    apply(case_tac "cdt a slot")
-     apply(simp add: next_slot_eq[OF mdb_empty_abs'.next_slot_no_parent])
-     apply(case_tac "next_slot (aa, bb) (cdt_list a) (cdt a)")
-      subgoal by (simp)
-     apply(clarsimp)
-     apply(frule(1) mdb_empty.n_next)
-     apply(clarsimp)
-     apply(erule_tac x=aa in allE, erule_tac x=bb in allE)
-     apply(simp split: if_split_asm)
-      apply(drule cte_map_inj_eq)
-           apply(drule cte_at_next_slot)
-             apply(assumption)+
-      apply(simp)
-     apply(subgoal_tac "(ab, bc) = slot")
-      prefer 2
-      apply(drule_tac cte="CTE s_cap s_node" in valid_mdbD2')
-        subgoal by (clarsimp simp: valid_mdb_ctes_def no_0_def)
-       subgoal by (clarsimp simp: invs'_def valid_state'_def valid_pspace'_def)
-      apply(clarsimp)
-      apply(rule cte_map_inj_eq)
-           apply(assumption)
-          apply(drule(3) cte_at_next_slot', assumption)
-         apply(assumption)+
-     apply(simp)
-     apply(drule_tac p="(aa, bb)" in no_parent_not_next_slot)
-        apply(assumption)+
-     apply(clarsimp)
-
-    apply(simp add: next_slot_eq[OF mdb_empty_abs'.next_slot] split del: if_split)
-    apply(case_tac "next_slot (aa, bb) (cdt_list a) (cdt a)")
-     subgoal by (simp)
-    apply(case_tac "(aa, bb) = slot", simp)
-    apply(case_tac "next_slot (aa, bb) (cdt_list a) (cdt a) = Some slot")
-     apply(simp)
-     apply(case_tac "next_slot ac (cdt_list a) (cdt a)", simp)
-     apply(simp)
-     apply(frule(1) mdb_empty.n_next)
-     apply(clarsimp)
-     apply(erule_tac x=aa in allE', erule_tac x=bb in allE)
-     apply(erule_tac x=ac in allE, erule_tac x=bd in allE)
-     apply(clarsimp split: if_split_asm)
-      apply(drule(1) no_self_loop_next)
-      apply(simp)
-     apply(drule_tac cte="CTE cap' node'" in valid_mdbD1')
-       apply(fastforce simp: valid_mdb_ctes_def no_0_def)
-      subgoal by (simp add: valid_mdb'_def)
-     apply(clarsimp)
-    apply(simp)
-    apply(frule(1) mdb_empty.n_next)
-    apply(erule_tac x=aa in allE, erule_tac x=bb in allE)
-    apply(clarsimp split: if_split_asm)
-     apply(drule(1) no_self_loop_prev)
-     apply(clarsimp)
-     apply(drule_tac cte="CTE s_cap s_node" in valid_mdbD2')
-       apply(clarsimp simp: valid_mdb_ctes_def no_0_def)
-      apply clarify
-     apply(clarsimp)
-     apply(drule cte_map_inj_eq)
-          apply(drule(3) cte_at_next_slot')
-          apply(assumption)+
-     apply(simp)
-    apply(erule disjE)
-     apply(drule cte_map_inj_eq)
-          apply(drule(3) cte_at_next_slot)
-          apply(assumption)+
-     apply(simp)
-    subgoal by (simp)
-   apply (simp add: revokable_relation_def)
-   apply (clarsimp simp: in_set_cap_cte_at)
-   apply (rule conjI)
-    apply clarsimp
-    apply (drule(1) mdb_empty.n_revokable)
-    subgoal by clarsimp
-   apply clarsimp
-   apply (drule (1) mdb_empty.n_revokable)
-   apply (subgoal_tac "null_filter (caps_of_state a) (aa,bb) \<noteq> None")
-    prefer 2
-    apply (drule set_cap_caps_of_state_monad)
-    subgoal by (force simp: null_filter_def)
-   apply clarsimp
-   apply (subgoal_tac "cte_at (aa, bb) a")
-    prefer 2
-    apply (drule null_filter_caps_of_stateD, erule cte_wp_cte_at)
-   apply (drule (2) cte_map_inj_ps, fastforce)
-   subgoal by simp
-  apply (clarsimp simp add: cdt_relation_def)
-  apply (subst mdb_empty_abs.descendants, assumption)
-  apply (subst mdb_empty.descendants, assumption)
-  apply clarsimp
-  apply (frule_tac p="(aa, bb)" in in_set_cap_cte_at)
-  apply clarsimp
-  apply (frule (2) cte_map_inj_ps, fastforce)
-  apply simp
-  apply (case_tac "slot \<in> descendants_of (aa,bb) (cdt a)")
-   apply (subst inj_on_image_set_diff)
-      apply (rule inj_on_descendants_cte_map)
-         apply fastforce
-        apply fastforce
-       apply fastforce
-      apply fastforce
-     apply fastforce
-    subgoal by simp
-   subgoal by simp
-  apply simp
-  apply (subgoal_tac "cte_map slot \<notin> descendants_of' (cte_map (aa,bb)) (ctes_of b)")
-   subgoal by simp
-  apply (erule_tac x=aa in allE, erule allE, erule (1) impE)
-  apply (drule_tac s="cte_map ` u" for u in sym)
-  apply clarsimp
-  apply (drule cte_map_inj_eq, assumption)
-      apply (erule descendants_of_cte_at, fastforce)
-     apply fastforce
-    apply fastforce
-   apply fastforce
-  apply simp
-  done
-
-
-
-text \<open>Some facts about is_final_cap/isFinalCapability\<close>
-
-lemma isFinalCapability_inv:
-  "\<lbrace>P\<rbrace> isFinalCapability cap \<lbrace>\<lambda>_. P\<rbrace>"
-  apply (simp add: isFinalCapability_def Let_def
-              split del: if_split cong: if_cong)
-  apply (rule hoare_pre, wp)
-   apply (rule hoare_post_imp[where Q'="\<lambda>s. P"], simp)
-   apply wp
-  apply simp
-  done
-
-definition
-  final_matters' :: "capability \<Rightarrow> bool"
-where
- "final_matters' cap \<equiv> case cap of
-    EndpointCap ref bdg s r g gr \<Rightarrow> True
-  | NotificationCap ref bdg s r \<Rightarrow> True
-  | ThreadCap ref \<Rightarrow> True
-  | CNodeCap ref bits gd gs \<Rightarrow> True
-  | Zombie ptr zb n \<Rightarrow> True
-  | IRQHandlerCap irq \<Rightarrow> True
-  | ArchObjectCap acap \<Rightarrow> (case acap of
-    PageCap d ref rghts sz mapdata \<Rightarrow> False
-  | ASIDControlCap \<Rightarrow> False
-  | SGISignalCap _ _ \<Rightarrow> False
-  | _ \<Rightarrow> True)
-  | _ \<Rightarrow> False"
 
 lemma final_matters_Master:
   "final_matters' (capMasterCap cap) = final_matters' cap"
   by (simp add: capMasterCap_def arch_capMasterCap_def split: capability.split arch_capability.split,
-      simp add: final_matters'_def)
+      simp add: final_matters'_def arch_final_matters'_def)
 
 lemma final_matters_sameRegion_sameObject:
   "final_matters' cap \<Longrightarrow> sameRegionAs cap cap' = sameObjectAs cap cap'"
   apply (rule iffI)
    apply (erule sameRegionAsE)
       apply (simp add: sameObjectAs_def3)
-      apply (clarsimp simp: isCap_simps sameObjectAs_sameRegionAs final_matters'_def
-        split:capability.splits arch_capability.splits)+
+      apply (clarsimp simp: isCap_simps sameObjectAs_sameRegionAs
+                            final_matters'_def arch_final_matters'_def
+                      split: capability.splits arch_capability.splits)+
   done
 
 lemma final_matters_sameRegion_sameObject2:
   "\<lbrakk> final_matters' cap'; \<not> isUntypedCap cap; \<not> isIRQHandlerCap cap' \<rbrakk>
-     \<Longrightarrow> sameRegionAs cap cap' = sameObjectAs cap cap'"
+   \<Longrightarrow> sameRegionAs cap cap' = sameObjectAs cap cap'"
   apply (rule iffI)
    apply (erule sameRegionAsE)
        apply (simp add: sameObjectAs_def3)
-       apply (fastforce simp: isCap_simps final_matters'_def)
+       apply (fastforce simp: isCap_simps final_matters'_def arch_final_matters'_def)
       apply simp
-     apply (clarsimp simp: final_matters'_def isCap_simps)
-    apply (clarsimp simp: final_matters'_def isCap_simps)
-   apply (clarsimp simp: final_matters'_def isCap_simps)
+     apply (clarsimp simp: final_matters'_def arch_final_matters'_def isCap_simps)+
   apply (erule sameObjectAs_sameRegionAs)
   done
 
 lemma final_matters_mdb_chunked_arch_assms:
   "final_matters' cap \<Longrightarrow> mdb_chunked_arch_assms cap"
-  by (clarsimp simp: mdb_chunked_arch_assms_def isCap_simps final_matters'_def)
+  by (clarsimp simp: mdb_chunked_arch_assms_def isCap_simps
+                     final_matters'_def arch_final_matters'_def)
 
-lemma notFinal_prev_or_next:
+lemma notFinal_prev_or_next[Finalise_R_2_assms]:
   "\<lbrakk> \<not> isFinal cap x (cteCaps_of s); mdb_chunked (ctes_of s);
-      valid_dlist (ctes_of s); no_0 (ctes_of s);
-      ctes_of s x = Some (CTE cap node); final_matters' cap \<rbrakk>
-     \<Longrightarrow> (\<exists>cap' node'. ctes_of s (mdbPrev node) = Some (CTE cap' node')
-              \<and> sameObjectAs cap cap')
-      \<or> (\<exists>cap' node'. ctes_of s (mdbNext node) = Some (CTE cap' node')
-              \<and> sameObjectAs cap cap')"
+     valid_dlist (ctes_of s); no_0 (ctes_of s);
+     ctes_of s x = Some (CTE cap node); final_matters' cap \<rbrakk>
+   \<Longrightarrow> (\<exists>cap' node'. ctes_of s (mdbPrev node) = Some (CTE cap' node') \<and> sameObjectAs cap cap')
+      \<or> (\<exists>cap' node'. ctes_of s (mdbNext node) = Some (CTE cap' node') \<and> sameObjectAs cap cap')"
   apply (erule not_FinalE)
    apply (clarsimp simp: isCap_simps final_matters'_def)
   apply (frule final_matters_mdb_chunked_arch_assms)
@@ -1957,91 +543,20 @@ lemma notFinal_prev_or_next:
   apply (clarsimp simp: sameObjectAs_def3 simp del: isArchFrameCap_capMasterCap)
   done
 
-lemma isFinal:
-  "\<lbrace>\<lambda>s. valid_mdb' s \<and> cte_wp_at' ((=) cte) x s
-          \<and> final_matters' (cteCap cte)
-          \<and> Q (isFinal (cteCap cte) x (cteCaps_of s)) s\<rbrace>
-    isFinalCapability cte
-   \<lbrace>Q\<rbrace>"
-  unfolding isFinalCapability_def
-  apply (cases cte)
-  apply (rename_tac cap node)
-  apply (unfold Let_def)
-  apply (simp only: if_False)
-  apply (wp getCTE_wp')
-  apply (cases "mdbPrev (cteMDBNode cte) = nullPointer")
-   apply simp
-   apply (clarsimp simp: valid_mdb_ctes_def valid_mdb'_def
-                         cte_wp_at_ctes_of)
-   apply (rule conjI, clarsimp simp: nullPointer_def)
-    apply (erule rsubst[where P="\<lambda>x. Q x s" for s], simp)
-    apply (rule classical)
-    apply (drule(5) notFinal_prev_or_next)
-    apply clarsimp
-   apply (clarsimp simp: nullPointer_def)
-   apply (erule rsubst[where P="\<lambda>x. Q x s" for s])
-   apply (rule sym, rule iffI)
-    apply (rule classical)
-    apply (drule(5) notFinal_prev_or_next)
-    apply clarsimp
-   apply clarsimp
-   apply (clarsimp simp: cte_wp_at_ctes_of cteCaps_of_def)
-   apply (case_tac cte)
-   apply clarsimp
-   apply (clarsimp simp add: isFinal_def)
-   apply (erule_tac x="mdbNext node" in allE)
-   apply simp
-   apply (erule impE)
-    apply (clarsimp simp: valid_mdb'_def valid_mdb_ctes_def)
-    apply (drule (1) mdb_chain_0_no_loops)
-    apply simp
-   apply (clarsimp simp: sameObjectAs_def3 isCap_simps)
-  apply simp
-  apply (clarsimp simp: cte_wp_at_ctes_of
-                        valid_mdb_ctes_def valid_mdb'_def)
-  apply (case_tac cte)
-  apply clarsimp
-  apply (rule conjI)
-   apply clarsimp
-   apply (erule rsubst[where P="\<lambda>x. Q x s" for s])
-   apply clarsimp
-   apply (clarsimp simp: isFinal_def cteCaps_of_def)
-   apply (erule_tac x="mdbPrev node" in allE)
-   apply simp
-   apply (erule impE)
-    apply clarsimp
-    apply (drule (1) mdb_chain_0_no_loops)
-    apply (subgoal_tac "ctes_of s (mdbNext node) = Some (CTE cap node)")
-     apply clarsimp
-    apply (erule (1) valid_dlistEp)
-     apply clarsimp
-    apply (case_tac cte')
-    apply clarsimp
-   apply (fastforce simp add: sameObjectAs_def3 isCap_simps)
-  apply clarsimp
-  apply (rule conjI)
-   apply clarsimp
-   apply (erule rsubst[where P="\<lambda>x. Q x s" for s], simp)
-   apply (rule classical, drule(5) notFinal_prev_or_next)
-   apply (clarsimp simp: sameObjectAs_sym nullPointer_def)
-  apply (clarsimp simp: nullPointer_def)
-  apply (erule rsubst[where P="\<lambda>x. Q x s" for s])
-  apply (rule sym, rule iffI)
-   apply (rule classical, drule(5) notFinal_prev_or_next)
-   apply (clarsimp simp: sameObjectAs_sym)
-   apply auto[1]
-  apply (clarsimp simp: isFinal_def cteCaps_of_def)
-  apply (case_tac cte)
-  apply (erule_tac x="mdbNext node" in allE)
-  apply simp
-  apply (erule impE)
-   apply clarsimp
-   apply (drule (1) mdb_chain_0_no_loops)
-   apply simp
-  apply clarsimp
-  apply (clarsimp simp: isCap_simps sameObjectAs_def3)
-  done
-end
+lemma sameObjectAs_not_Untyped[Finalise_R_2_assms]:
+  "\<lbrakk> global.sameObjectAs cap cap'; \<not> isUntypedCap cap \<rbrakk>
+   \<Longrightarrow> \<not> isUntypedCap cap'"
+  by (clarsimp simp: gen_isCap_simps sameObjectAs_def3)
+
+lemma sameObjectAs_not_Untyped'[Finalise_R_2_assms]:
+  "\<lbrakk> global.sameObjectAs cap cap'; \<not> isUntypedCap cap' \<rbrakk>
+   \<Longrightarrow> global.sameObjectAs cap' cap"
+  by (clarsimp simp: isCap_simps sameObjectAs_def3)
+
+end (* Arch *)
+
+(* only two arch-specific lemmas in vmdb;
+   save processing time by not creating an extra Arch_vmdb locale, directly requalify instead *)
 
 lemma (in vmdb) isFinal_no_subtree:
   "\<lbrakk> m \<turnstile> sl \<rightarrow> p; isFinal cap sl (option_map cteCap o m);
@@ -2051,20 +566,9 @@ lemma (in vmdb) isFinal_no_subtree:
    apply (clarsimp simp: isFinal_def parentOf_def mdb_next_unfold cteCaps_of_def)
    apply (erule_tac x="mdbNext n" in allE)
    apply simp
-   (* FIXME arch-split *)
-   apply (clarsimp simp: ARM.isMDBParentOf_CTE final_matters_sameRegion_sameObject)
-   apply (clarsimp simp: gen_isCap_simps ARM.sameObjectAs_def3) (* FIXME arch-split *)
+   apply (clarsimp simp: ARM.isMDBParentOf_CTE ARM.final_matters_sameRegion_sameObject)
+   apply (clarsimp simp: gen_isCap_simps ARM.sameObjectAs_def3)
   apply clarsimp
-  done
-
-lemma isFinal_no_descendants:
-  "\<lbrakk> isFinal cap sl (cteCaps_of s); ctes_of s sl = Some (CTE cap n);
-      valid_mdb' s; final_matters' cap \<rbrakk>
-  \<Longrightarrow> descendants_of' sl (ctes_of s) = {}"
-  apply (clarsimp simp add: descendants_of'_def cteCaps_of_def)
-  apply (erule(3) vmdb.isFinal_no_subtree[rotated])
-  apply unfold_locales[1]
-  apply (simp add: valid_mdb'_def)
   done
 
 lemma (in vmdb) isFinal_untypedParent:
@@ -2089,67 +593,535 @@ lemma (in vmdb) isFinal_untypedParent:
   apply clarsimp
   apply (drule isMDBParent_sameRegion)
   apply simp
-  apply (frule final_matters_mdb_chunked_arch_assms)
+  apply (frule ARM.final_matters_mdb_chunked_arch_assms)
   apply (rule classical, simp)
-  apply (simp add: final_matters_sameRegion_sameObject2
+  apply (simp add: ARM.final_matters_sameRegion_sameObject2
                    sameObjectAs_sym)
   done
 
-context begin interpretation Arch . (*FIXME: arch-split*)
+context Arch begin arch_global_naming
 
-lemma no_fail_isFinalCapability [wp]:
-  "no_fail (valid_mdb' and cte_wp_at' ((=) cte) p) (isFinalCapability cte)"
-  apply (simp add: isFinalCapability_def)
-  apply (clarsimp simp: Let_def split del: if_split)
-  apply (rule no_fail_pre, wp getCTE_wp')
-  apply (clarsimp simp: valid_mdb'_def valid_mdb_ctes_def cte_wp_at_ctes_of nullPointer_def)
-  apply (rule conjI)
-   apply clarsimp
-   apply (erule (2) valid_dlistEp)
-   apply simp
-  apply clarsimp
-  apply (rule conjI)
-   apply (erule (2) valid_dlistEn)
-   apply simp
-  apply clarsimp
-  apply (rule valid_dlistEn, assumption+)
-  apply (erule (2) valid_dlistEp)
-  apply simp
+lemma isFinal_no_descendants:
+  "\<lbrakk> isFinal cap sl (cteCaps_of s); ctes_of s sl = Some (CTE cap n);
+      valid_mdb' s; final_matters' cap \<rbrakk>
+  \<Longrightarrow> descendants_of' sl (ctes_of s) = {}"
+  apply (clarsimp simp add: descendants_of'_def cteCaps_of_def)
+  apply (erule(3) vmdb.isFinal_no_subtree[rotated])
+  apply unfold_locales[1]
+  apply (simp add: valid_mdb'_def)
   done
 
-lemma corres_gets_lift:
-  assumes inv: "\<And>P. \<lbrace>P\<rbrace> g \<lbrace>\<lambda>_. P\<rbrace>"
-  assumes res: "\<lbrace>Q'\<rbrace> g \<lbrace>\<lambda>r s. r = g' s\<rbrace>"
-  assumes Q: "\<And>s. Q s \<Longrightarrow> Q' s"
-  assumes nf: "no_fail Q g"
-  shows "corres r P Q f (gets g') \<Longrightarrow> corres r P Q f g"
-  apply (clarsimp simp add: corres_underlying_def simpler_gets_def)
-  apply (drule (1) bspec)
+lemmas cancelAllIPC_typs[wp] = typ_at_lifts[OF cancelAllIPC_typ_at']
+lemmas cancelAllSignals_typs[wp] = typ_at_lifts[OF cancelAllSignals_typ_at']
+lemmas suspend_typs[wp] = typ_at_lifts[OF suspend_typ_at']
+
+lemmas finaliseCap_typ_ats[wp] = typ_at_lifts[OF finaliseCap_typ_at']
+
+crunch flushSpace
+  for invs'[wp]: "invs'"
+  (ignore: doMachineOp)
+
+lemma invalidateASIDEntry_invs'[wp]:
+  "invalidateASIDEntry asid \<lbrace>invs'\<rbrace>"
+  apply (simp add: invalidateASIDEntry_def invalidateASID_def
+                   invalidateHWASIDEntry_def bind_assoc)
+  apply (wp loadHWASID_wp | simp)+
+  apply (clarsimp simp: fun_upd_def[symmetric])
   apply (rule conjI)
-   apply clarsimp
-   apply (rule bexI)
-    prefer 2
-    apply assumption
-   apply simp
-   apply (frule in_inv_by_hoareD [OF inv])
-   apply simp
-   apply (drule use_valid, rule res)
-    apply (erule Q)
-   apply simp
-  apply (insert nf)
-  apply (clarsimp simp: no_fail_def)
+   apply (clarsimp simp: invs'_def valid_state'_def)
+   apply (rule conjI)
+    apply (simp add: valid_global_refs'_def
+                     global_refs'_def)
+   apply (simp add: valid_arch_state'_def ran_def
+                    valid_asid_table'_def is_inv_None_upd
+                    valid_machine_state'_def
+                    comp_upd_simp fun_upd_def[symmetric]
+                    inj_on_fun_upd_elsewhere
+                    valid_asid_map'_def
+                    ct_idle_or_in_cur_domain'_def tcb_in_cur_domain'_def
+             cong: option.case_cong)
+   subgoal by (auto elim!: subset_inj_on)
+  apply (clarsimp simp: invs'_def valid_state'_def)
+  apply (rule conjI)
+   apply (simp add: valid_global_refs'_def global_refs'_def)
+  apply (rule conjI)
+   apply (simp add: valid_arch_state'_def ran_def
+                    valid_asid_table'_def comp_upd_simp
+              cong: option.case_cong)
+  apply (simp add: valid_machine_state'_def ct_idle_or_in_cur_domain'_def tcb_in_cur_domain'_def)
   done
 
-lemma obj_refs_Master:
-  "\<lbrakk> cap_relation cap cap'; P cap \<rbrakk>
-      \<Longrightarrow> obj_refs cap =
-           (if capClass (capMasterCap cap') = PhysicalClass
-                  \<and> \<not> isUntypedCap (capMasterCap cap')
-            then {capUntypedPtr (capMasterCap cap')} else {})"
-  by (clarsimp simp: isCap_simps
-              split: cap_relation_split_asm arch_cap.split_asm)
+lemma invs_asid_update_strg':
+  "invs' s \<and> tab = armKSASIDTable (ksArchState s) \<longrightarrow>
+   invs' (s\<lparr>ksArchState := armKSASIDTable_update
+            (\<lambda>_. tab (asid := None)) (ksArchState s)\<rparr>)"
+  apply (simp add: invs'_def)
+  apply (simp add: valid_state'_def)
+  apply (simp add: valid_global_refs'_def global_refs'_def valid_arch_state'_def
+                   valid_asid_table'_def valid_machine_state'_def ct_idle_or_in_cur_domain'_def
+                   tcb_in_cur_domain'_def
+             cong: option.case_cong)
+  apply (auto simp add: ran_def split: if_split_asm)
+  done
 
-lemma isFinalCapability_corres':
+crunch invalidateTLBByASID
+  for asidTable[wp]: "\<lambda>s. P (armKSASIDTable (ksArchState s))"
+
+crunch copyGlobalMappings
+  for pred_tcb_at'[wp]: "pred_tcb_at' proj P t"
+  (wp: crunch_wps ignore: storePDE)
+
+lemma deleteASIDPool_invs[wp]:
+  "\<lbrace>invs'\<rbrace> deleteASIDPool asid pool \<lbrace>\<lambda>rv. invs'\<rbrace>"
+  apply (simp add: deleteASIDPool_def)
+  apply wp
+      apply (simp del: fun_upd_apply)
+      apply (strengthen invs_asid_update_strg')
+      apply (wpsimp wp: mapM_wp' getObject_inv loadObject_default_inv)+
+  done
+
+lemma deleteASID_invs'[wp]:
+  "deleteASID asid pd \<lbrace>invs'\<rbrace>"
+  apply (simp add: deleteASID_def cong: option.case_cong)
+  apply (rule hoare_pre)
+   apply (wp | wpc)+
+    apply (rule_tac Q'="\<lambda>rv. valid_obj' (injectKO rv) and invs'"
+              in hoare_post_imp)
+     apply (rename_tac rv s)
+     apply (clarsimp split: if_split_asm del: subsetI)
+     apply (simp add: fun_upd_def[symmetric] valid_obj'_def)
+     apply (case_tac rv, simp)
+     apply (subst inv_f_f, rule inj_onI, simp)+
+     apply (rule conjI)
+      apply clarsimp
+      apply (drule subsetD, blast)
+      apply clarsimp
+     apply (auto dest!: ran_del_subset)[1]
+    apply (wp getObject_valid_obj getObject_inv loadObject_default_inv
+             | simp add: objBits_simps pageBits_def)+
+  apply clarsimp
+  done
+
+lemmas archThreadSet_typ_ats[wp] = typ_at_lifts[OF archThreadSet_typ_at']
+
+lemma archThreadSet_valid_objs'[wp]:
+  "\<lbrace>valid_objs' and (\<lambda>s. \<forall>tcb. ko_at' tcb t s \<longrightarrow> valid_arch_tcb' (f (tcbArch tcb)) s)\<rbrace>
+   archThreadSet f t \<lbrace>\<lambda>_. valid_objs'\<rbrace>"
+  unfolding archThreadSet_def
+  apply (wp setObject_tcb_valid_objs getObject_tcb_wp)
+  apply clarsimp
+  apply normalise_obj_at'
+  apply (drule (1) tcb_ko_at_valid_objs_valid_tcb')
+  apply (clarsimp simp: valid_obj'_def valid_tcb'_def tcb_cte_cases_def cteSizeBits_def)
+  done
+
+crunch archThreadSet
+  for no_0_obj'[wp]: no_0_obj'
+
+lemma archThreadSet_ctes_of[wp]:
+  "archThreadSet f t \<lbrace>\<lambda>s. P (ctes_of s)\<rbrace>"
+  unfolding archThreadSet_def
+  apply (wpsimp wp: getObject_tcb_wp)
+  apply normalise_obj_at'
+  apply (auto simp: tcb_cte_cases_def cteSizeBits_def)
+  done
+
+crunch archThreadSet
+  for ksCurDomain[wp]: "\<lambda>s. P (ksCurDomain s)"
+  (wp: setObject_cd_inv)
+
+lemma archThreadSet_obj_at':
+  "(\<And>tcb. P tcb \<Longrightarrow> P (tcb \<lparr> tcbArch:= f (tcbArch tcb)\<rparr>)) \<Longrightarrow> archThreadSet f t \<lbrace>obj_at' P t'\<rbrace>"
+  unfolding archThreadSet_def
+  apply (wpsimp wp: getObject_tcb_wp setObject_tcb_strongest)
+  apply normalise_obj_at'
+  apply auto
+  done
+
+lemma archThreadSet_tcbDomain[wp]:
+  "archThreadSet f t \<lbrace>obj_at' (\<lambda>tcb. x = tcbDomain tcb) t'\<rbrace>"
+  by (wpsimp wp: archThreadSet_obj_at')
+
+lemma archThreadSet_inQ[wp]:
+  "archThreadSet f t' \<lbrace>\<lambda>s. P (obj_at' (inQ d p) t s)\<rbrace>"
+  unfolding obj_at'_real_def archThreadSet_def
+  apply (wpsimp wp: setObject_ko_wp_at getObject_tcb_wp
+              simp: objBits_simps' archObjSize_def pageBits_def
+         | simp)+
+  apply (auto simp: obj_at'_def ko_wp_at'_def)
+  done
+
+crunch archThreadSet
+  for ct[wp]: "\<lambda>s. P (ksCurThread s)"
+  and sched[wp]: "\<lambda>s. P (ksSchedulerAction s)"
+  and L1[wp]: "\<lambda>s. P (ksReadyQueuesL1Bitmap s)"
+  and L2[wp]: "\<lambda>s. P (ksReadyQueuesL2Bitmap s)"
+  and ksArch[wp]: "\<lambda>s. P (ksArchState s)"
+  and ksDomSchedule[wp]: "\<lambda>s. P (ksDomSchedule s)"
+  and pspace_canonical'[wp]: pspace_canonical'
+  and gsMaxObjectSize[wp]: "\<lambda>s. P (gsMaxObjectSize s)"
+  and ksInterruptState[wp]: "\<lambda>s. P (ksInterruptState s)"
+  (wp: setObject_ct_inv setObject_sa_unchanged setObject_ksDomSchedule_inv)
+
+crunch archThreadSet
+  for ksDomScheduleIdx[wp]: "\<lambda>s. P (ksDomScheduleIdx s)"
+  and ksDomScheduleStart[wp]: "\<lambda>s. P (ksDomScheduleStart s)"
+  (simp: setObject_def wp: updateObject_default_inv)
+
+crunch archThreadSet
+  for ksMachineState[wp]: "\<lambda>s. P (ksMachineState s)"
+  (wp: setObject_ksMachine updateObject_default_inv)
+
+lemma archThreadSet_state_refs_of'[wp]:
+  "archThreadSet f t \<lbrace>\<lambda>s. P (state_refs_of' s)\<rbrace>"
+  unfolding archThreadSet_def
+  apply (wpsimp wp: setObject_tcb_state_refs_of' getObject_tcb_wp)
+  apply normalise_obj_at'
+  apply (erule rsubst[where P=P])
+  apply (rule ext)
+  apply (auto simp: state_refs_of'_def obj_at'_def)
+  done
+
+lemma archThreadSet_state_hyp_refs_of'[wp]:
+  "\<lbrace>\<lambda>s. \<forall>tcb. ko_at' tcb t s \<longrightarrow> P ((state_hyp_refs_of' s)(t := tcb_hyp_refs' (f (tcbArch tcb))))\<rbrace>
+  archThreadSet f t \<lbrace>\<lambda>_ s. P (state_hyp_refs_of' s)\<rbrace>"
+  unfolding archThreadSet_def
+  apply (wpsimp wp: setObject_state_hyp_refs_of' getObject_tcb_wp simp: objBits_simps')
+  apply normalise_obj_at'
+  apply (erule rsubst[where P=P])
+  apply auto
+  done
+
+crunch archThreadSet
+  for ko_at'_pde[wp]: "\<lambda>s. P (ko_at' (pde::pde) p' s)"
+  and valid_pde_mappings'[wp]: valid_pde_mappings'
+
+lemma archThreadSet_ifunsafe'[wp]:
+  "archThreadSet f t \<lbrace>if_unsafe_then_cap'\<rbrace>"
+  unfolding archThreadSet_def
+  apply (wpsimp wp: setObject_tcb_ifunsafe' getObject_tcb_wp)
+  apply normalise_obj_at'
+  apply (auto simp: tcb_cte_cases_def if_live_then_nonz_cap'_def cteSizeBits_def)
+  done
+
+lemma archThreadSet_valid_idle'[wp]:
+  "archThreadSet f t \<lbrace>valid_idle'\<rbrace>"
+  unfolding archThreadSet_def
+  apply (wpsimp wp: setObject_tcb_idle' getObject_tcb_wp)
+  apply (clarsimp simp: valid_idle'_def pred_tcb_at'_def obj_at'_def idle_tcb'_def)
+  done
+
+lemma archThreadSet_ct_not_inQ[wp]:
+  "archThreadSet f t \<lbrace>ct_not_inQ\<rbrace>"
+  unfolding ct_not_inQ_def
+  apply (rule hoare_lift_Pf[where f=ksCurThread]; wp?)
+  apply (wpsimp wp: hoare_vcg_imp_lift simp: o_def)
+  done
+
+lemma archThreadSet_obj_at'_pte[wp]:
+  "archThreadSet f t \<lbrace>obj_at' (P::pte \<Rightarrow> bool) p\<rbrace>"
+  unfolding archThreadSet_def
+  by (wpsimp wp: obj_at_setObject2 simp: updateObject_default_def in_monad)
+
+crunch archThreadSet
+  for pspace_domain_valid[wp]: pspace_domain_valid
+
+crunch archThreadSet
+  for gsUntypedZeroRanges[wp]: "\<lambda>s. P (gsUntypedZeroRanges s)"
+
+lemma archThreadSet_untyped_ranges_zero'[wp]:
+  "archThreadSet f t \<lbrace>untyped_ranges_zero'\<rbrace>"
+  by (rule hoare_lift_Pf[where f=cteCaps_of]; wp cteCaps_of_ctes_of_lift)
+
+lemma archThreadSet_tcb_at'[wp]:
+  "\<lbrace>\<top>\<rbrace> archThreadSet f t \<lbrace>\<lambda>_. tcb_at' t\<rbrace>"
+  unfolding archThreadSet_def
+  by (wpsimp wp: getObject_tcb_wp simp: obj_at'_def)
+
+lemma archThreadSet_tcbSchedPrevs_of[wp]:
+  "archThreadSet f t \<lbrace>\<lambda>s. P (tcbSchedPrevs_of s)\<rbrace>"
+  unfolding archThreadSet_def
+  apply (wp getObject_tcb_wp)
+  apply normalise_obj_at'
+  apply (erule rsubst[where P=P])
+  apply (rule ext)
+  apply (clarsimp simp: opt_map_def obj_at'_def split: option.splits)
+  done
+
+lemma archThreadSet_tcbSchedNexts_of[wp]:
+  "archThreadSet f t \<lbrace>\<lambda>s. P (tcbSchedNexts_of s)\<rbrace>"
+  unfolding archThreadSet_def
+  apply (wp getObject_tcb_wp)
+  apply normalise_obj_at'
+  apply (erule rsubst[where P=P])
+  apply (rule ext)
+  apply (clarsimp simp: opt_map_def obj_at'_def split: option.splits)
+  done
+
+lemma archThreadSet_tcbQueued[wp]:
+  "archThreadSet f t \<lbrace>\<lambda>s. P (tcbQueued |< tcbs_of' s)\<rbrace>"
+  unfolding archThreadSet_def
+  apply (wp getObject_tcb_wp)
+  apply normalise_obj_at'
+  apply (erule rsubst[where P=P])
+  apply (rule ext)
+  apply (clarsimp simp: opt_pred_def opt_map_def obj_at'_def split: option.splits)
+  done
+
+lemma archThreadSet_valid_sched_pointers[wp]:
+  "archThreadSet f t \<lbrace>valid_sched_pointers\<rbrace>"
+  by (wp_pre, wps, wp, assumption)
+
+lemma arch_finaliseCap_invs[Finalise_R_2_assms, wp]:
+  "\<lbrace>invs' and valid_cap' (ArchObjectCap cap)\<rbrace> Arch.finaliseCap cap fin \<lbrace>\<lambda>rv. invs'\<rbrace>"
+  unfolding ARM_H.finaliseCap_def Let_def by wpsimp
+
+crunch setVMRoot, deleteASIDPool, invalidateTLBByASID, invalidateASIDEntry
+  for ctes_of[wp]: "\<lambda>s. P (ctes_of s)"
+  (wp: crunch_wps getObject_inv loadObject_default_inv getASID_wp simp: crunch_simps)
+
+lemma deleteASID_ctes_of[wp]:
+  "deleteASID a ptr \<lbrace>\<lambda>s. P (ctes_of s)\<rbrace>"
+  unfolding deleteASID_def by (wpsimp wp: getASID_wp hoare_drop_imps hoare_vcg_all_lift)
+
+lemma arch_finaliseCap_removeable[wp]:
+  "\<lbrace>\<lambda>s. s \<turnstile>' ArchObjectCap cap \<and> invs' s
+       \<and> (final_matters' (ArchObjectCap cap)
+               \<longrightarrow> (final = isFinal (ArchObjectCap cap) slot (cteCaps_of s))) \<rbrace>
+     Arch.finaliseCap cap final
+   \<lbrace>\<lambda>rv s. isNullCap (fst rv) \<and> removeable' slot s (ArchObjectCap cap) \<and> isNullCap (snd rv)\<rbrace>"
+  apply (simp add: ARM_H.finaliseCap_def
+                   removeable'_def)
+  apply (safe ; wpsimp)
+  done
+
+crunch archThreadSet
+  for isFinal: "\<lambda>s. isFinal cap slot (cteCaps_of s)"
+  (wp: cteCaps_of_ctes_of_lift)
+
+crunch prepareThreadDelete
+  for isFinal: "\<lambda>s. isFinal cap slot (cteCaps_of s)"
+
+lemma archThreadSet_bound_tcb_at'[wp]:
+  "archThreadSet f t \<lbrace>bound_tcb_at' P t'\<rbrace>"
+  unfolding archThreadSet_def
+  apply (wpsimp wp: setObject_tcb_strongest getObject_tcb_wp simp: pred_tcb_at'_def)
+  by (auto simp: obj_at'_def objBits_simps)
+
+crunch prepareThreadDelete
+  for bound_tcb_at'[wp]: "bound_tcb_at' P t"
+  (wp: sts_bound_tcb_at' crunch_wps hoare_vcg_all_lift hoare_vcg_if_lift3
+   ignore: archThreadSet)
+
+crunch Arch.finaliseCap, prepareThreadDelete
+  for irq_node'[Finalise_R_2_assms, wp]: "\<lambda>s. P (irq_node' s)"
+  (wp: crunch_wps getObject_inv loadObject_default_inv
+       updateObject_default_inv setObject_ksInterrupt
+   simp: crunch_simps o_def)
+
+lemmas Arch_finaliseCap_irq_node'[Finalise_R_2_assms] = ArchRetypeDecls_H_ARM_H_finaliseCap_irq_node'
+
+crunch prepareThreadDelete
+  for cte_wp_at'[Finalise_R_2_assms, wp]: "cte_wp_at' P p"
+  and valid_cap'[Finalise_R_2_assms, wp]: "valid_cap' cap"
+
+crunch prepareThreadDelete
+  for invs[Finalise_R_2_assms, wp]: "invs'"
+  (ignore: doMachineOp simp: crunch_simps)
+
+lemma archThreadSet_tcbSchedPrevNext[wp]:
+  "archThreadSet f t' \<lbrace>obj_at' (\<lambda>tcb. P (tcbSchedNext tcb) (tcbSchedPrev tcb)) t\<rbrace>"
+  unfolding archThreadSet_def
+  apply (wpsimp wp: setObject_tcb_strongest getObject_tcb_wp)
+  apply normalise_obj_at'
+  apply auto
+  done
+
+context notes if_cong[cong] begin
+
+crunch asUser
+  for tcbSchedPrevNext[wp]: "obj_at' (\<lambda>tcb. P (tcbSchedNext tcb) (tcbSchedPrev tcb)) t"
+  (wp: threadGet_wp)
+
+end
+
+crunch prepareThreadDelete
+  for tcbSchedPrevNext[wp]: "obj_at' (\<lambda>tcb. P (tcbSchedNext tcb) (tcbSchedPrev tcb)) t"
+  (wp: threadGet_wp archThreadGet_wp crunch_wps simp: crunch_simps)
+
+crunch deleteASIDPool
+  for cte_wp_at'[wp]: "cte_wp_at' P p"
+  (simp: crunch_simps assertE_def
+   wp: crunch_wps getObject_inv loadObject_default_inv)
+
+lemma deleteASID_cte_wp_at'[wp]:
+  "\<lbrace>cte_wp_at' P p\<rbrace> deleteASID param_a param_b \<lbrace>\<lambda>_. cte_wp_at' P p\<rbrace>"
+  apply (simp add: deleteASID_def
+              cong: option.case_cong)
+  apply (wp setObject_cte_wp_at'[where Q="\<top>"] getObject_inv
+            loadObject_default_inv setVMRoot_cte_wp_at'
+          | clarsimp simp: updateObject_default_def in_monad cong: if_cong
+          | rule equals0I
+          | wpc)+
+  done
+
+lemma arch_finaliseCap_cte_wp_at[Finalise_R_2_assms, wp]:
+  "\<lbrace>cte_wp_at' P p\<rbrace> Arch.finaliseCap cap fin \<lbrace>\<lambda>rv. cte_wp_at' P p\<rbrace>"
+  unfolding ARM_H.finaliseCap_def
+  by (wpsimp wp: unmapPage_cte_wp_at'|rule conjI)+
+
+lemma finaliseCap_valid_cap[Finalise_R_2_assms, wp]:
+  "\<lbrace>\<top>\<rbrace> Arch.finaliseCap cap final \<lbrace>\<lambda>rv. valid_cap' (fst rv)\<rbrace>"
+  by (wpsimp simp: ARM_H.finaliseCap_def split_del: if_split)
+
+lemma finaliseCap_cases[wp]:
+  "\<lbrace>\<top>\<rbrace>
+   finaliseCap cap final flag
+   \<lbrace>\<lambda>rv s. fst rv = NullCap \<and> (snd rv \<noteq> NullCap \<longrightarrow> final \<and> cap_has_cleanup' cap \<and> snd rv = cap)
+           \<or> isZombie (fst rv) \<and> final \<and> \<not> flag \<and> snd rv = NullCap
+             \<and> capUntypedPtr (fst rv) = capUntypedPtr cap
+             \<and> (isThreadCap cap \<or> isCNodeCap cap \<or> isZombie cap)\<rbrace>"
+  apply (simp add: finaliseCap_def ARM_H.finaliseCap_def Let_def
+                   getThreadCSpaceRoot
+             cong: if_cong split del: if_split)
+  apply (rule hoare_pre)
+   apply ((wp | simp add: gen_isCap_simps split del: if_split
+              | wpc
+              | simp only: valid_NullCap fst_conv snd_conv)+)[1]
+  apply (simp only: simp_thms fst_conv snd_conv option.simps if_cancel
+                    o_def)
+  apply (intro allI impI conjI TrueI)
+  apply (auto simp add: gen_isCap_simps cap_has_cleanup'_def)
+  done
+
+lemmas [Finalise_R_2_assms] =
+  cancelAllIPC_cte_wp_at' cancelAllSignals_cte_wp_at' unbindMaybeNotification_cte_wp_at'
+  prepareThreadDelete_cte_wp_at' unbindNotification_cte_wp_at'
+  Arch_postCapDeletion_valid_global_refs Arch_postCapDeletion_valid_arch_state'
+  mdb_empty.vmdb_n mdb_empty.descendants not_Final_removeable
+
+end (* Arch *)
+
+interpretation Finalise_R_2?: Finalise_R_2 arch_final_matters' arch_cap_has_cleanup'
+proof goal_cases
+  interpret Arch  .
+  case 1 show ?case by (intro_locales; (unfold_locales; (fact Finalise_R_2_assms)?)?)
+qed
+
+(* this is the only arch-specific lemma in delete_one_conc_pre so far;
+   save processing time by not creating an extra Arch_delete_one_conc_pre locale
+   by directly requalifying instead *)
+lemma (in delete_one_conc_pre) finaliseCap_replaceable:
+  "\<lbrace>\<lambda>s. invs' s \<and> cte_wp_at' (\<lambda>cte. cteCap cte = cap) slot s
+       \<and> (final_matters' cap \<longrightarrow> (final = isFinal cap slot (cteCaps_of s)))
+       \<and> weak_sch_act_wf (ksSchedulerAction s) s\<rbrace>
+     finaliseCap cap final flag
+   \<lbrace>\<lambda>rv s. (isNullCap (fst rv) \<and> removeable' slot s cap
+                \<and> (snd rv \<noteq> NullCap \<longrightarrow> snd rv = cap \<and> cap_has_cleanup' cap
+                                      \<and> isFinal cap slot (cteCaps_of s)))
+        \<or>
+          (isZombie (fst rv) \<and> snd rv = NullCap
+            \<and> isFinal cap slot (cteCaps_of s)
+            \<and> capClass cap = capClass (fst rv)
+            \<and> capUntypedPtr (fst rv) = capUntypedPtr cap
+            \<and> capBits (fst rv) = capBits cap
+            \<and> capRange (fst rv) = capRange cap
+            \<and> (isThreadCap cap \<or> isCNodeCap cap \<or> isZombie cap)
+            \<and> (\<forall>p \<in> threadCapRefs cap. st_tcb_at' ((=) Inactive) p s
+                     \<and> obj_at' (Not \<circ> tcbQueued) p s
+                     \<and> bound_tcb_at' ((=) None) p s
+                     \<and> obj_at' (\<lambda>tcb. tcbSchedNext tcb = None \<and> tcbSchedPrev tcb = None) p s))\<rbrace>"
+  supply [wp] = ARM.prepareThreadDelete_bound_tcb_at'
+                ARM.prepareThreadDelete_tcbSchedPrevNext
+  apply (simp add: finaliseCap_def Let_def getThreadCSpaceRoot
+             cong: if_cong split del: if_split)
+  apply (rule hoare_pre)
+   apply (wp prepares_delete_helper'' [OF cancelAllIPC_unlive]
+             prepares_delete_helper'' [OF cancelAllSignals_unlive]
+             suspend_isFinal ARM.prepareThreadDelete_unqueued
+             ARM.prepareThreadDelete_inactive ARM.prepareThreadDelete_isFinal
+             suspend_makes_inactive
+             deletingIRQHandler_removeable'
+             deletingIRQHandler_final[where slot=slot ]
+             unbindMaybeNotification_obj_at'_bound
+             getNotification_wp
+             suspend_bound_tcb_at'
+             unbindNotification_bound_tcb_at'
+             suspend_tcbSchedNext_tcbSchedPrev_None
+           | simp add: isZombie_Null isThreadCap_threadCapRefs_tcbptr
+                       isArchObjectCap_Cap_capCap
+           | (rule hoare_strengthen_post[OF ARM.arch_finaliseCap_removeable[where slot=slot]],
+              clarsimp simp: gen_isCap_simps)
+           | wpc)+
+  apply clarsimp
+  apply (frule cte_wp_at_valid_objs_valid_cap', clarsimp+)
+  apply (case_tac "cteCap cte",
+         simp_all add: gen_isCap_simps capRange_def cap_has_cleanup'_def
+                       final_matters'_def gen_objBits_simps
+                       not_Final_removeable finaliseCap_def,
+         simp_all add: removeable'_def)
+     (* thread *)
+     apply (frule capAligned_capUntypedPtr [OF valid_capAligned], simp)
+     apply (clarsimp simp: valid_cap'_def)
+     apply (drule valid_globals_cte_wpD'[rotated], clarsimp)
+     apply (clarsimp simp: invs'_def valid_state'_def valid_pspace'_def)
+    apply (clarsimp simp: obj_at'_def | rule conjI)+
+  done
+
+context Arch begin arch_global_naming
+
+named_theorems Finalise_R_3_assms
+
+lemma finaliseCap_cte_refs:
+  "\<lbrace>\<lambda>s. s \<turnstile>' cap\<rbrace>
+     finaliseCap cap final flag
+   \<lbrace>\<lambda>rv s. fst rv \<noteq> NullCap \<longrightarrow> cte_refs' (fst rv) = cte_refs' cap\<rbrace>"
+  apply (simp add: global.finaliseCap_def Let_def getThreadCSpaceRoot finaliseCap_def
+             cong: if_cong split del: if_split)
+  apply (rule hoare_pre)
+   apply (wp | wpc | simp only: o_def)+
+  apply (frule valid_capAligned)
+  apply (cases cap, simp_all add: gen_isCap_simps)
+   apply (clarsimp simp: tcb_cte_cases_def word_count_from_top gen_objBits_simps)
+  apply clarsimp
+  apply (rule ext, simp)
+  apply (rule image_cong [OF _ refl])
+  apply (fastforce simp: mask_def capAligned_def gen_objBits_simps shiftL_nat)
+  done
+
+lemma emptySlot_invs'[wp]:
+  "\<lbrace>\<lambda>s. invs' s \<and> cte_wp_at' (\<lambda>cte. removeable' sl s (cteCap cte)) sl s
+            \<and> (\<forall>sl'. info \<noteq> NullCap \<longrightarrow> sl' \<noteq> sl \<longrightarrow> cteCaps_of s sl' \<noteq> Some info)\<rbrace>
+     emptySlot sl info
+   \<lbrace>\<lambda>rv. invs'\<rbrace>"
+  apply (simp add: invs'_def valid_state'_def valid_pspace'_def)
+  apply (wp valid_irq_node_lift cur_tcb_lift valid_dom_schedule'_lift)
+  apply (clarsimp simp: cte_wp_at_ctes_of)
+  done
+
+lemma cteDeleteOne_invs[Finalise_R_3_assms, wp]:
+  "cteDeleteOne ptr \<lbrace>invs'\<rbrace>"
+  apply (simp add: cteDeleteOne_def unless_def
+                   split_def finaliseCapTrue_standin_simple_def)
+  apply wp
+    apply (rule hoare_strengthen_post)
+     apply (rule hoare_vcg_conj_lift[OF finaliseCap_True_invs])
+     apply (rule hoare_vcg_conj_lift[OF finaliseCap_replaceable[where slot=ptr]])
+     apply (rule hoare_vcg_conj_lift[OF finaliseCap_cte_refs])
+     apply (rule finaliseCap_equal_cap[where sl=ptr])
+    apply (clarsimp simp: cte_wp_at_ctes_of)
+    apply (erule disjE, solves simp)
+    apply (clarsimp dest!: isCapDs simp: capRemovable_def)
+    apply (clarsimp simp: removeable'_def fun_eq_iff[where f="cte_refs' cap" for cap]
+                     del: disjCI)
+    subgoal by (auto dest!: isCapDs simp: pred_tcb_at'_def obj_at'_def
+                                          live'_def hyp_live'_def ko_wp_at'_def)
+   apply (wp isFinalCapability_inv getCTE_wp' hoare_weak_lift_imp
+          | wp (once) isFinal[where x=ptr])+
+  apply (fastforce simp: cte_wp_at_ctes_of)
+  done
+
+lemma isFinalCapability_corres'[Finalise_R_3_assms]:
   "final_matters' (cteCap cte) \<Longrightarrow>
    corres (=) (invs and cte_wp_at ((=) cap) ptr)
                (invs' and cte_wp_at' ((=) cte) (cte_map ptr))
@@ -2191,7 +1163,7 @@ lemma isFinalCapability_corres':
    apply (erule_tac x=aa in allE)
    apply (erule_tac x=ba in allE)
    apply (clarsimp simp: cte_wp_at_caps_of_state)
-   apply (clarsimp simp: sameObjectAs_def3 obj_refs_Master cap_irqs_relation_Master
+   apply (clarsimp simp: sameObjectAs_def3 obj_refs_relation_Master cap_irqs_relation_Master
                          arch_gen_refs_relation_Master gen_obj_refs_Int
                    cong: if_cong
                   split: capability.split_asm)
@@ -2199,7 +1171,7 @@ lemma isFinalCapability_corres':
   apply (rule_tac x="fst ptr" in exI)
   apply (rule_tac x="snd ptr" in exI)
   apply (rule conjI)
-   apply (clarsimp simp: cte_wp_at_def final_matters'_def
+   apply (clarsimp simp: cte_wp_at_def final_matters'_def arch_final_matters'_def
                          gen_obj_refs_Int
                   split: cap_relation_split_asm arch_cap.split_asm)
   apply clarsimp
@@ -2225,1176 +1197,45 @@ lemma isFinalCapability_corres':
    apply (rule classical)
    apply (frule(1) zombies_finalD2[OF _ _ _ invs_zombies],
           simp?, clarsimp, assumption+)
-   subgoal by (clarsimp simp: sameObjectAs_def3 isCap_simps valid_cap_def
-                         obj_at_def is_obj_defs a_type_def final_matters'_def
-                  split: cap.split_asm arch_cap.split_asm
-                         option.split_asm if_split_asm,
-          simp_all add: is_cap_defs)
+   subgoal by (clarsimp simp: sameObjectAs_def3 isCap_simps valid_cap_def valid_arch_cap_def
+                              valid_arch_cap_ref_def obj_at_def is_obj_defs a_type_def
+                              final_matters'_def arch_final_matters'_def
+                        split: cap.split_asm arch_cap.split_asm option.split_asm if_split_asm,
+               simp_all add: is_cap_defs)
   apply (rule classical)
   by (clarsimp simp: cap_irqs_def cap_irq_opt_def sameObjectAs_def3 isCap_simps arch_gen_obj_refs_def
                  split: cap.split_asm)
 
-lemma isFinalCapability_corres:
-  "corres (\<lambda>rv rv'. final_matters' (cteCap cte) \<longrightarrow> rv = rv')
-          (invs and cte_wp_at ((=) cap) ptr)
-          (invs' and cte_wp_at' ((=) cte) (cte_map ptr))
-       (is_final_cap cap) (isFinalCapability cte)"
-  apply (cases "final_matters' (cteCap cte)")
-   apply simp
-   apply (erule isFinalCapability_corres')
-  apply (subst bind_return[symmetric],
-         rule corres_symb_exec_r)
-     apply (rule corres_no_failI)
-      apply wp
-     apply (clarsimp simp: in_monad is_final_cap_def simpler_gets_def)
-    apply (wp isFinalCapability_inv)+
-  apply fastforce
-  done
-
-text \<open>Facts about finalise_cap/finaliseCap and
-        cap_delete_one/cteDelete in no particular order\<close>
-
-
-definition
-  finaliseCapTrue_standin_simple_def:
-  "finaliseCapTrue_standin cap fin \<equiv> finaliseCap cap fin True"
-
-context
-begin
-
-declare if_cong [cong]
-
-lemmas finaliseCapTrue_standin_def
-    = finaliseCapTrue_standin_simple_def
-        [unfolded finaliseCap_def, simplified]
-
-lemmas cteDeleteOne_def'
-    = eq_reflection [OF cteDeleteOne_def]
-lemmas cteDeleteOne_def
-    = cteDeleteOne_def'[folded finaliseCapTrue_standin_simple_def]
-
-crunch cteDeleteOne, suspend, prepareThreadDelete
-  for typ_at'[wp]: "\<lambda>s. P (typ_at' T p s)"
-  (wp: crunch_wps getObject_inv loadObject_default_inv
-   simp: crunch_simps unless_def o_def)
-
-end
-
-lemmas cancelAllIPC_typs[wp] = typ_at_lifts [OF cancelAllIPC_typ_at']
-lemmas cancelAllSignals_typs[wp] = typ_at_lifts [OF cancelAllSignals_typ_at']
-lemmas suspend_typs[wp] = typ_at_lifts [OF suspend_typ_at']
-
-definition
-  arch_cap_has_cleanup' :: "arch_capability \<Rightarrow> bool"
-where
-  "arch_cap_has_cleanup' acap \<equiv> False"
-
-definition
-  cap_has_cleanup' :: "capability \<Rightarrow> bool"
-where
-  "cap_has_cleanup' cap \<equiv> case cap of
-     IRQHandlerCap _ \<Rightarrow> True
-   | ArchObjectCap acap \<Rightarrow> arch_cap_has_cleanup' acap
-   | _ \<Rightarrow> False"
-
-lemmas cap_has_cleanup'_simps[simp] = cap_has_cleanup'_def[split_simps capability.split]
-
-lemma finaliseCap_cases[wp]:
-  "\<lbrace>\<top>\<rbrace>
-     finaliseCap cap final flag
-   \<lbrace>\<lambda>rv s. fst rv = NullCap \<and> (snd rv \<noteq> NullCap \<longrightarrow> final \<and> cap_has_cleanup' cap \<and> snd rv = cap)
-     \<or>
-       isZombie (fst rv) \<and> final \<and> \<not> flag \<and> snd rv = NullCap
-        \<and> capUntypedPtr (fst rv) = capUntypedPtr cap
-        \<and> (isThreadCap cap \<or> isCNodeCap cap \<or> isZombie cap)\<rbrace>"
-  apply (simp add: finaliseCap_def ARM_H.finaliseCap_def Let_def
-                   getThreadCSpaceRoot
-             cong: if_cong split del: if_split)
-  apply (rule hoare_pre)
-   apply ((wp | simp add: isCap_simps split del: if_split
-              | wpc
-              | simp only: valid_NullCap fst_conv snd_conv)+)[1]
-  apply (simp only: simp_thms fst_conv snd_conv option.simps if_cancel
-                    o_def)
-  apply (intro allI impI conjI TrueI)
-  apply (auto simp add: isCap_simps cap_has_cleanup'_def)
-  done
-
-crunch finaliseCap
-  for aligned'[wp]: "pspace_aligned'"
-  (simp: crunch_simps assertE_def unless_def o_def
-     wp: getObject_inv loadObject_default_inv crunch_wps)
-
-crunch finaliseCap
-  for distinct'[wp]: "pspace_distinct'"
-  (simp: crunch_simps assertE_def unless_def o_def
-     wp: getObject_inv loadObject_default_inv crunch_wps)
-
-crunch finaliseCap
-  for typ_at'[wp]: "\<lambda>s. P (typ_at' T p s)"
-  (simp: crunch_simps assertE_def
-     wp: getObject_inv loadObject_default_inv crunch_wps)
-lemmas finaliseCap_typ_ats[wp] = typ_at_lifts[OF finaliseCap_typ_at']
-
-crunch finaliseCap
-  for it'[wp]: "\<lambda>s. P (ksIdleThread s)"
-  (wp: mapM_x_wp_inv mapM_wp' hoare_drop_imps getObject_inv loadObject_default_inv
-   simp: crunch_simps o_def)
-
-lemma ntfn_q_refs_of'_mult:
-  "ntfn_q_refs_of' ntfn = (case ntfn of Structures_H.WaitingNtfn q \<Rightarrow> set q | _ \<Rightarrow> {}) \<times> {NTFNSignal}"
-  by (cases ntfn, simp_all)
-
-lemma tcb_st_not_Bound:
-  "(p, NTFNBound) \<notin> tcb_st_refs_of' ts"
-  "(p, TCBBound) \<notin> tcb_st_refs_of' ts"
-  by (auto simp: tcb_st_refs_of'_def split: Structures_H.thread_state.split)
-
-crunch setBoundNotification
-  for valid_bitmaps[wp]: valid_bitmaps
-  and tcbSchedNexts_of[wp]: "\<lambda>s. P (tcbSchedNexts_of s)"
-  and tcbSchedPrevs_of[wp]: "\<lambda>s. P (tcbSchedPrevs_of s)"
-  and tcbQueued[wp]: "\<lambda>s. P (tcbQueued |< tcbs_of' s)"
-  and valid_sched_pointers[wp]: valid_sched_pointers
-  (wp: valid_bitmaps_lift)
-
-lemma unbindNotification_invs[wp]:
-  "\<lbrace>invs'\<rbrace> unbindNotification tcb \<lbrace>\<lambda>rv. invs'\<rbrace>"
-  apply (simp add: unbindNotification_def invs'_def valid_state'_def)
-  apply (rule bind_wp[OF _ gbn_sp'])
-  apply (case_tac ntfnPtr, clarsimp, wp, clarsimp)
-  apply clarsimp
-  apply (rule bind_wp[OF _ get_ntfn_sp'])
-  apply (rule hoare_pre)
-  apply (wp sbn'_valid_pspace'_inv sbn_sch_act' valid_irq_node_lift valid_dom_schedule'_lift
-            irqs_masked_lift setBoundNotification_ct_not_inQ sym_heap_sched_pointers_lift
-            untyped_ranges_zero_lift | clarsimp simp: cteCaps_of_def o_def)+
-  apply (rule conjI)
-   apply (clarsimp elim!: obj_atE'
-                    simp: projectKOs
-                   dest!: pred_tcb_at')
-  apply (clarsimp simp: pred_tcb_at' conj_comms)
-  apply (frule bound_tcb_ex_cap'', clarsimp+)
-  apply (frule(1) sym_refs_bound_tcb_atD')
-  apply (frule(1) sym_refs_obj_atD')
-  apply (clarsimp simp: refs_of_rev')
-  apply normalise_obj_at'
-  apply (subst delta_sym_refs, assumption)
-    apply (auto split: if_split_asm)[1]
-   apply (auto simp: tcb_st_not_Bound ntfn_q_refs_of'_mult split: if_split_asm)[1]
-  apply (frule obj_at_valid_objs', clarsimp+)
-  apply (simp add: valid_ntfn'_def valid_obj'_def projectKOs live'_def
-            split: ntfn.splits)
-  apply (erule if_live_then_nonz_capE')
-  apply (clarsimp simp: obj_at'_def ko_wp_at'_def projectKOs live'_def)
-  done
-
-lemma ntfn_bound_tcb_at':
-  "\<lbrakk>sym_refs (state_refs_of' s); valid_objs' s; ko_at' ntfn ntfnptr s;
-    ntfnBoundTCB ntfn = Some tcbptr; P (Some ntfnptr)\<rbrakk>
-  \<Longrightarrow> bound_tcb_at' P tcbptr s"
-  apply (drule_tac x=ntfnptr in sym_refsD[rotated])
-   apply (clarsimp simp: obj_at'_def projectKOs)
-   apply (fastforce simp: state_refs_of'_def)
-  apply (auto simp: pred_tcb_at'_def obj_at'_def valid_obj'_def valid_ntfn'_def
-                    state_refs_of'_def refs_of_rev' projectKOs
-          simp del: refs_of_simps
-             elim!: valid_objsE
-             split: option.splits if_split_asm)
-  done
-
-
-lemma unbindMaybeNotification_invs[wp]:
-  "\<lbrace>invs'\<rbrace> unbindMaybeNotification ntfnptr \<lbrace>\<lambda>rv. invs'\<rbrace>"
-  apply (simp add: unbindMaybeNotification_def invs'_def valid_state'_def)
-  apply (rule bind_wp[OF _ get_ntfn_sp'])
-  apply (rule hoare_pre)
-   apply (wp sbn'_valid_pspace'_inv sbn_sch_act' sym_heap_sched_pointers_lift valid_irq_node_lift
-             irqs_masked_lift valid_dom_schedule'_lift setBoundNotification_ct_not_inQ
-             untyped_ranges_zero_lift
-             | wpc | clarsimp simp: cteCaps_of_def o_def)+
-  apply safe[1]
-           defer 3
-           defer 7
-           apply (fold_subgoals (prefix))[8]
-           subgoal premises prems using prems by (auto simp: pred_tcb_at' valid_pspace'_def projectKOs valid_obj'_def valid_ntfn'_def
-                             ko_wp_at'_def live'_def
-                      elim!: obj_atE' valid_objsE' if_live_then_nonz_capE'
-                      split: option.splits ntfn.splits)
-   apply (rule delta_sym_refs, assumption)
-    apply (fold_subgoals (prefix))[2]
-    subgoal premises prems using prems by (fastforce simp: symreftype_inverse' ntfn_q_refs_of'_def
-                    split: ntfn.splits if_split_asm
-                     dest!: ko_at_state_refs_ofD')+
-  apply (rule delta_sym_refs, assumption)
-   apply (clarsimp split: if_split_asm)
-   apply (frule ko_at_state_refs_ofD', simp)
-  apply (clarsimp split: if_split_asm)
-   apply (frule_tac P="(=) (Some ntfnptr)" in ntfn_bound_tcb_at', simp_all add: valid_pspace'_def)[1]
-   subgoal by (fastforce simp: ntfn_q_refs_of'_def state_refs_of'_def tcb_ntfn_is_bound'_def
-                          tcb_st_refs_of'_def
-                   dest!: bound_tcb_at_state_refs_ofD'
-                   split: ntfn.splits thread_state.splits)
-  apply (frule ko_at_state_refs_ofD', simp)
-  done
-
-(* Ugh, required to be able to split out the abstract invs *)
-lemma finaliseCap_True_invs[wp]:
-  "\<lbrace>invs'\<rbrace> finaliseCap cap final True \<lbrace>\<lambda>rv. invs'\<rbrace>"
-  apply (simp add: finaliseCap_def Let_def)
-  apply safe
-    apply (wp irqs_masked_lift| simp | wpc)+
-  done
-
-crunch flushSpace
-  for invs'[wp]: "invs'"
-  (ignore: doMachineOp)
-
-lemma invs_asid_update_strg':
-  "invs' s \<and> tab = armKSASIDTable (ksArchState s) \<longrightarrow>
-   invs' (s\<lparr>ksArchState := armKSASIDTable_update
-            (\<lambda>_. tab (asid := None)) (ksArchState s)\<rparr>)"
-  apply (simp add: invs'_def)
-  apply (simp add: valid_state'_def)
-  apply (simp add: valid_global_refs'_def global_refs'_def valid_arch_state'_def valid_asid_table'_def valid_machine_state'_def ct_idle_or_in_cur_domain'_def tcb_in_cur_domain'_def)
-  apply (auto simp add: ran_def split: if_split_asm)
-  done
-
-lemma invalidateASIDEntry_invs' [wp]:
-  "\<lbrace>invs'\<rbrace> invalidateASIDEntry asid \<lbrace>\<lambda>r. invs'\<rbrace>"
-  apply (simp add: invalidateASIDEntry_def invalidateASID_def
-                   invalidateHWASIDEntry_def bind_assoc)
-  apply (wp loadHWASID_wp | simp)+
-  apply (clarsimp simp: fun_upd_def[symmetric])
-  apply (rule conjI)
-   apply (clarsimp simp: invs'_def valid_state'_def)
-   apply (rule conjI)
-    apply (simp add: valid_global_refs'_def
-                     global_refs'_def)
-   apply (simp add: valid_arch_state'_def ran_def
-                    valid_asid_table'_def is_inv_None_upd
-                    valid_machine_state'_def
-                    comp_upd_simp fun_upd_def[symmetric]
-                    inj_on_fun_upd_elsewhere
-                    valid_asid_map'_def
-                    ct_idle_or_in_cur_domain'_def tcb_in_cur_domain'_def)
-   subgoal by (auto elim!: subset_inj_on)
-  apply (clarsimp simp: invs'_def valid_state'_def)
-  apply (rule conjI)
-   apply (simp add: valid_global_refs'_def
-                    global_refs'_def)
-  apply (rule conjI)
-   apply (simp add: valid_arch_state'_def ran_def
-                    valid_asid_table'_def None_upd_eq
-                    fun_upd_def[symmetric] comp_upd_simp)
-  apply (simp add: valid_machine_state'_def ct_idle_or_in_cur_domain'_def tcb_in_cur_domain'_def)
-  done
-
-lemma deleteASIDPool_invs[wp]:
-  "\<lbrace>invs'\<rbrace> deleteASIDPool asid pool \<lbrace>\<lambda>rv. invs'\<rbrace>"
-  apply (simp add: deleteASIDPool_def)
-  apply wp
-    apply (simp del: fun_upd_apply)
-    apply (strengthen invs_asid_update_strg')
-  apply (wp mapM_wp' getObject_inv loadObject_default_inv
-              | simp)+
-  done
-
-lemmas flushSpace_typ_ats' [wp] = typ_at_lifts [OF flushSpace_typ_at']
-
-lemma deleteASID_invs'[wp]:
-  "\<lbrace>invs'\<rbrace> deleteASID asid pd \<lbrace>\<lambda>rv. invs'\<rbrace>"
-  apply (simp add: deleteASID_def cong: option.case_cong)
-  apply (rule hoare_pre)
-   apply (wp | wpc)+
-    apply (rule_tac Q'="\<lambda>rv. valid_obj' (injectKO rv) and invs'"
-              in hoare_post_imp)
-     apply (rename_tac rv s)
-     apply (clarsimp split: if_split_asm del: subsetI)
-     apply (simp add: fun_upd_def[symmetric] valid_obj'_def)
-     apply (case_tac rv, simp)
-     apply (subst inv_f_f, rule inj_onI, simp)+
-     apply (rule conjI)
-      apply clarsimp
-      apply (drule subsetD, blast)
-      apply clarsimp
-     apply (auto dest!: ran_del_subset)[1]
-    apply (wp getObject_valid_obj getObject_inv loadObject_default_inv
-             | simp add: objBits_simps archObjSize_def pageBits_def)+
-  apply clarsimp
-  done
-
-lemma arch_finaliseCap_invs[wp]:
-  "\<lbrace>invs' and valid_cap' (ArchObjectCap cap)\<rbrace>
-     Arch.finaliseCap cap fin
-   \<lbrace>\<lambda>rv. invs'\<rbrace>"
-  unfolding ARM_H.finaliseCap_def
-  apply clarsimp
-  apply (safe ; wpsimp)
-  done
-
-lemma arch_finaliseCap_removeable[wp]:
-  "\<lbrace>\<lambda>s. s \<turnstile>' ArchObjectCap cap \<and> invs' s
-       \<and> (final \<and> final_matters' (ArchObjectCap cap)
-            \<longrightarrow> isFinal (ArchObjectCap cap) slot (cteCaps_of s))\<rbrace>
-     Arch.finaliseCap cap final
-   \<lbrace>\<lambda>rv s. isNullCap (fst rv) \<and> removeable' slot s (ArchObjectCap cap) \<and> isNullCap (snd rv)\<rbrace>"
-  apply (simp add: ARM_H.finaliseCap_def
-                   removeable'_def)
-  apply (safe ; wpsimp)
-  done
-
-lemma isZombie_Null:
-  "\<not> isZombie NullCap"
-  by (simp add: isCap_simps)
-
-lemma prepares_delete_helper'':
-  assumes x: "\<lbrace>P\<rbrace> f \<lbrace>\<lambda>rv. ko_wp_at' (Not \<circ> live') p\<rbrace>"
-  shows      "\<lbrace>P and K ((\<forall>x. cte_refs' cap x = {})
-                          \<and> zobj_refs' cap = {p}
-                          \<and> threadCapRefs cap = {})\<rbrace>
-                 f \<lbrace>\<lambda>rv s. removeable' sl s cap\<rbrace>"
-  apply (rule hoare_gen_asm)
-  apply (rule hoare_strengthen_post [OF x])
-  apply (clarsimp simp: removeable'_def)
-  done
-
-lemmas ctes_of_cteCaps_of_lift = cteCaps_of_ctes_of_lift
-
-crunch finaliseCapTrue_standin, unbindNotification
-  for ctes_of[wp]: "\<lambda>s. P (ctes_of s)"
-  (wp: crunch_wps getObject_inv loadObject_default_inv simp: crunch_simps)
-
-lemma cteDeleteOne_cteCaps_of:
-  "\<lbrace>\<lambda>s. (cte_wp_at' (\<lambda>cte. \<exists>final. finaliseCap (cteCap cte) final True \<noteq> fail) p s \<longrightarrow>
-          P ((cteCaps_of s)(p \<mapsto> NullCap)))\<rbrace>
-     cteDeleteOne p
-   \<lbrace>\<lambda>rv s. P (cteCaps_of s)\<rbrace>"
-  apply (simp add: cteDeleteOne_def unless_def split_def)
-  apply (rule bind_wp [OF _ getCTE_sp])
-  apply (case_tac "\<forall>final. finaliseCap (cteCap cte) final True = fail")
-   apply (simp add: finaliseCapTrue_standin_simple_def)
-   apply wp
-   apply (clarsimp simp: cte_wp_at_ctes_of cteCaps_of_def
-                         finaliseCap_def isCap_simps)
-   apply (drule_tac x=s in fun_cong)
-   apply (simp add: return_def fail_def)
-  apply (wp emptySlot_cteCaps_of)
-    apply (simp add: cteCaps_of_def)
-    apply (wp (once) hoare_drop_imps)
-    apply (wp isFinalCapability_inv getCTE_wp')+
-  apply (clarsimp simp: cteCaps_of_def cte_wp_at_ctes_of)
-  apply (auto simp: fun_upd_idem fun_upd_def[symmetric] o_def)
-  done
-
-lemma cteDeleteOne_isFinal:
-  "\<lbrace>\<lambda>s. isFinal cap slot (cteCaps_of s)\<rbrace>
-     cteDeleteOne p
-   \<lbrace>\<lambda>rv s. isFinal cap slot (cteCaps_of s)\<rbrace>"
-  apply (wp cteDeleteOne_cteCaps_of)
-  apply (clarsimp simp: isFinal_def sameObjectAs_def2)
-  done
-
-lemmas setEndpoint_cteCaps_of[wp] = ctes_of_cteCaps_of_lift [OF set_ep_ctes_of]
-lemmas setNotification_cteCaps_of[wp] = ctes_of_cteCaps_of_lift [OF set_ntfn_ctes_of]
-lemmas threadSet_cteCaps_of = ctes_of_cteCaps_of_lift [OF threadSet_ctes_of]
-
-crunch suspend, prepareThreadDelete
-  for isFinal: "\<lambda>s. isFinal cap slot (cteCaps_of s)"
-  (ignore: threadSet
-       wp: threadSet_cteCaps_of crunch_wps
-     simp: crunch_simps unless_def o_def)
-
-lemma isThreadCap_threadCapRefs_tcbptr:
-  "isThreadCap cap \<Longrightarrow> threadCapRefs cap = {capTCBPtr cap}"
-  by (clarsimp simp: isCap_simps)
-
-lemma isArchObjectCap_Cap_capCap:
-  "isArchObjectCap cap \<Longrightarrow> ArchObjectCap (capCap cap) = cap"
-  by (clarsimp simp: isCap_simps)
-
-lemma cteDeleteOne_deletes[wp]:
-  "\<lbrace>\<top>\<rbrace> cteDeleteOne p \<lbrace>\<lambda>rv s. cte_wp_at' (\<lambda>c. cteCap c = NullCap) p s\<rbrace>"
-  apply (subst tree_cte_cteCap_eq[unfolded o_def])
-  apply (wp cteDeleteOne_cteCaps_of)
-  apply clarsimp
-  done
-
-crunch finaliseCap
-  for irq_node'[wp]: "\<lambda>s. P (irq_node' s)"
-  (wp: mapM_x_wp crunch_wps getObject_inv loadObject_default_inv
-       updateObject_default_inv setObject_ksInterrupt
-   simp: crunch_simps unless_def o_def)
-
-lemma deletingIRQHandler_removeable':
-  "\<lbrace>invs' and (\<lambda>s. isFinal (IRQHandlerCap irq) slot (cteCaps_of s))
-          and K (cap = IRQHandlerCap irq)\<rbrace>
-     deletingIRQHandler irq
-   \<lbrace>\<lambda>rv s. removeable' slot s cap\<rbrace>"
-  apply (rule hoare_gen_asm)
-  apply (simp add: deletingIRQHandler_def getIRQSlot_def locateSlot_conv
-                   getInterruptState_def getSlotCap_def)
-  apply (simp add: removeable'_def tree_cte_cteCap_eq[unfolded o_def])
-  apply (subst tree_cte_cteCap_eq[unfolded o_def])+
-  apply (wp hoare_use_eq_irq_node' [OF cteDeleteOne_irq_node' cteDeleteOne_cteCaps_of]
-            getCTE_wp')
-  apply (clarsimp simp: cte_level_bits_def ucast_nat_def shiftl_t2n mult_ac cteSizeBits_def
-                  split: option.split_asm)
-  done
-
-lemma finaliseCap_cte_refs:
-  "\<lbrace>\<lambda>s. s \<turnstile>' cap\<rbrace>
-     finaliseCap cap final flag
-   \<lbrace>\<lambda>rv s. fst rv \<noteq> NullCap \<longrightarrow> cte_refs' (fst rv) = cte_refs' cap\<rbrace>"
-  apply (simp  add: finaliseCap_def Let_def getThreadCSpaceRoot
-                    ARM_H.finaliseCap_def
-             cong: if_cong split del: if_split)
-  apply (rule hoare_pre)
-   apply (wp | wpc | simp only: o_def)+
-  apply (frule valid_capAligned)
-  apply (cases cap, simp_all add: isCap_simps)
-   apply (clarsimp simp: tcb_cte_cases_def word_count_from_top objBits_defs)
-  apply clarsimp
-  apply (rule ext, simp)
-  apply (rule image_cong [OF _ refl])
-  apply (fastforce simp: capAligned_def objBits_simps shiftL_nat mask_def)
-  done
-
-lemma deletingIRQHandler_final:
-  "\<lbrace>\<lambda>s. isFinal cap slot (cteCaps_of s)
-             \<and> (\<forall>final. finaliseCap cap final True = fail)\<rbrace>
-     deletingIRQHandler irq
-   \<lbrace>\<lambda>rv s. isFinal cap slot (cteCaps_of s)\<rbrace>"
-  apply (simp add: deletingIRQHandler_def isFinal_def getIRQSlot_def
-                   getInterruptState_def locateSlot_conv getSlotCap_def)
-  apply (wp cteDeleteOne_cteCaps_of getCTE_wp')
-  apply (auto simp: sameObjectAs_def3)
-  done
-
-declare suspend_unqueued [wp]
-
-lemma unbindNotification_valid_objs'_helper:
-  "valid_tcb' tcb s \<longrightarrow> valid_tcb' (tcbBoundNotification_update (\<lambda>_. None) tcb) s "
-  by (clarsimp simp: valid_bound_ntfn'_def valid_tcb'_def tcb_cte_cases_def tcb_cte_cases_neqs
-                  split: option.splits ntfn.splits)
-
-lemma unbindNotification_valid_objs'_helper':
-  "valid_ntfn' tcb s \<longrightarrow> valid_ntfn' (ntfnBoundTCB_update (\<lambda>_. None) tcb) s "
-  by (clarsimp simp: valid_bound_tcb'_def valid_ntfn'_def
-                  split: option.splits ntfn.splits)
-
-lemmas setNotification_valid_tcb' = typ_at'_valid_tcb'_lift [OF setNotification_typ_at']
-
-lemma unbindNotification_valid_objs'[wp]:
-  "\<lbrace>valid_objs'\<rbrace>
-     unbindNotification t
-   \<lbrace>\<lambda>rv. valid_objs'\<rbrace>"
-  apply (simp add: unbindNotification_def)
-  apply (rule hoare_pre)
-  apply (wp threadSet_valid_objs' gbn_wp' set_ntfn_valid_objs' hoare_vcg_all_lift
-            setNotification_valid_tcb' getNotification_wp
-        | wpc | clarsimp simp: setBoundNotification_def unbindNotification_valid_objs'_helper)+
-  apply (clarsimp elim!: obj_atE' simp: projectKOs)
-  apply (rule valid_objsE', assumption+)
-  apply (clarsimp simp: valid_obj'_def unbindNotification_valid_objs'_helper')
-  done
-
-lemma unbindMaybeNotification_valid_objs'[wp]:
-  "\<lbrace>valid_objs'\<rbrace>
-     unbindMaybeNotification t
-   \<lbrace>\<lambda>rv. valid_objs'\<rbrace>"
-  apply (simp add: unbindMaybeNotification_def)
-  apply (rule bind_wp[OF _ get_ntfn_sp'])
-  apply (rule hoare_pre)
-  apply (wp threadSet_valid_objs' gbn_wp' set_ntfn_valid_objs' hoare_vcg_all_lift
-            setNotification_valid_tcb' getNotification_wp
-        | wpc | clarsimp simp: setBoundNotification_def unbindNotification_valid_objs'_helper)+
-  apply (clarsimp elim!: obj_atE' simp: projectKOs)
-  apply (rule valid_objsE', assumption+)
-  apply (clarsimp simp: valid_obj'_def unbindNotification_valid_objs'_helper')
-  done
-
-lemma unbindMaybeNotification_sch_act_wf[wp]:
-  "\<lbrace>\<lambda>s. sch_act_wf (ksSchedulerAction s) s\<rbrace> unbindMaybeNotification t
-  \<lbrace>\<lambda>rv s. sch_act_wf (ksSchedulerAction s) s\<rbrace>"
-  apply (simp add: unbindMaybeNotification_def)
-  apply (rule hoare_pre)
-  apply (wp sbn_sch_act' | wpc | simp)+
-  done
-
-lemma valid_cong:
-  "\<lbrakk> \<And>s. P s = P' s; \<And>s. P' s \<Longrightarrow> f s = f' s;
-        \<And>rv s' s. \<lbrakk> (rv, s') \<in> fst (f' s); P' s \<rbrakk> \<Longrightarrow> Q rv s' = Q' rv s' \<rbrakk>
-    \<Longrightarrow> \<lbrace>P\<rbrace> f \<lbrace>Q\<rbrace> = \<lbrace>P'\<rbrace> f' \<lbrace>Q'\<rbrace>"
-  by (clarsimp simp add: valid_def, blast)
-
-lemma unbindMaybeNotification_obj_at'_bound:
-  "\<lbrace>\<top>\<rbrace>
-     unbindMaybeNotification r
-   \<lbrace>\<lambda>_ s. obj_at' (\<lambda>ntfn. ntfnBoundTCB ntfn = None) r s\<rbrace>"
-  apply (simp add: unbindMaybeNotification_def)
-  apply (rule bind_wp[OF _ get_ntfn_sp'])
-  apply (rule hoare_pre)
-   apply (wp obj_at_setObject2
-        | wpc
-        | simp add: setBoundNotification_def threadSet_def updateObject_default_def in_monad projectKOs)+
-  apply (simp add: setNotification_def obj_at'_real_def cong: valid_cong)
-   apply (wp setObject_ko_wp_at, (simp add: objBits_simps')+)
-  apply (clarsimp simp: obj_at'_def ko_wp_at'_def projectKOs)
-  done
-
-context
-notes option.case_cong_weak[cong]
-begin
-crunch unbindNotification, unbindMaybeNotification
-  for isFinal[wp]: "\<lambda>s. isFinal cap slot (cteCaps_of s)"
-  (wp: sts_bound_tcb_at' threadSet_cteCaps_of crunch_wps getObject_inv loadObject_default_inv
-   ignore: threadSet)
-end
-
-crunch cancelSignal, cancelAllIPC
-  for bound_tcb_at'[wp]: "bound_tcb_at' P t"
-  (wp: sts_bound_tcb_at' threadSet_cteCaps_of crunch_wps getObject_inv
-       loadObject_default_inv)
-
-lemma finaliseCapTrue_standin_bound_tcb_at':
-  "\<lbrace>\<lambda>s. bound_tcb_at' P t s \<and> (\<exists>tt b r. cap = ReplyCap tt b r) \<rbrace>
-     finaliseCapTrue_standin cap final
-   \<lbrace>\<lambda>_. bound_tcb_at' P t\<rbrace>"
-  apply (case_tac cap, simp_all add:finaliseCapTrue_standin_def)
-  apply (clarsimp simp: isNotificationCap_def)
-  apply (wp, clarsimp)
-  done
-
-lemma capDeleteOne_bound_tcb_at':
-  "\<lbrace>bound_tcb_at' P tptr and cte_wp_at' (isReplyCap \<circ> cteCap) callerCap\<rbrace>
-      cteDeleteOne callerCap \<lbrace>\<lambda>rv. bound_tcb_at' P tptr\<rbrace>"
-  apply (simp add: cteDeleteOne_def unless_def)
-  apply (rule hoare_pre)
-   apply (wp finaliseCapTrue_standin_bound_tcb_at' hoare_vcg_all_lift
-            hoare_vcg_if_lift2 getCTE_cteCap_wp
-        | wpc | simp | wp (once) hoare_drop_imp)+
-  apply (clarsimp simp:  cteCaps_of_def projectKOs isReplyCap_def cte_wp_at_ctes_of
-                 split: option.splits)
-  apply (case_tac "cteCap cte", simp_all)
-  done
-
-lemma cancelIPC_bound_tcb_at'[wp]:
-  "\<lbrace>bound_tcb_at' P tptr\<rbrace> cancelIPC t \<lbrace>\<lambda>rv. bound_tcb_at' P tptr\<rbrace>"
-  apply (simp add: cancelIPC_def Let_def)
-  apply (rule bind_wp[OF _ gts_sp'])
-  apply (case_tac "state", simp_all)
-         defer 2
-         apply (rule hoare_pre)
-          apply ((wp sts_bound_tcb_at' getEndpoint_wp | wpc | simp)+)[8]
-  apply (simp add: getThreadReplySlot_def locateSlot_conv liftM_def)
-  apply (rule hoare_pre)
-   apply (wp capDeleteOne_bound_tcb_at' getCTE_ctes_of)
-   apply (rule_tac Q'="\<lambda>_. bound_tcb_at' P tptr" in hoare_post_imp)
-   apply (clarsimp simp: capHasProperty_def cte_wp_at_ctes_of)
-   apply (wp threadSet_pred_tcb_no_state | simp)+
-  done
-
-crunch suspend, prepareThreadDelete
-  for bound_tcb_at'[wp]: "bound_tcb_at' P t"
-  (wp: sts_bound_tcb_at' cancelIPC_bound_tcb_at')
-
-lemma unbindNotification_bound_tcb_at':
-  "\<lbrace>\<lambda>_. True\<rbrace> unbindNotification t \<lbrace>\<lambda>rv. bound_tcb_at' ((=) None) t\<rbrace>"
-  apply (simp add: unbindNotification_def)
-  apply (wp setBoundNotification_bound_tcb gbn_wp' | wpc | simp)+
-  done
-
-crunch unbindNotification, unbindMaybeNotification
-  for weak_sch_act_wf[wp]: "\<lambda>s. weak_sch_act_wf (ksSchedulerAction s) s"
-
-lemma unbindNotification_tcb_at'[wp]:
-  "\<lbrace>tcb_at' t'\<rbrace> unbindNotification t \<lbrace>\<lambda>rv. tcb_at' t'\<rbrace>"
-  apply (simp add: unbindNotification_def)
-  apply (wp gbn_wp' | wpc | simp)+
-  done
-
-lemma unbindMaybeNotification_tcb_at'[wp]:
-  "\<lbrace>tcb_at' t'\<rbrace> unbindMaybeNotification t \<lbrace>\<lambda>rv. tcb_at' t'\<rbrace>"
-  apply (simp add: unbindMaybeNotification_def)
-  apply (wp gbn_wp' | wpc | simp)+
-  done
-
-crunch prepareThreadDelete
-  for cte_wp_at'[wp]: "cte_wp_at' P p"
-crunch prepareThreadDelete
-  for valid_cap'[wp]: "valid_cap' cap"
-crunch prepareThreadDelete
-  for invs[wp]: "invs'"
-
-crunch prepareThreadDelete
-  for sched_projs_obj_at'[wp]:
-    "\<lambda>s. obj_at' (\<lambda>tcb. tcbSchedNext tcb = None \<and> tcbSchedPrev tcb = None) t s"
-
-end
-
-lemma tcbQueueRemove_tcbSchedNext_tcbSchedPrev_None_obj_at':
-  "\<lbrace>\<lambda>s. \<exists>ts. list_queue_relation ts q (tcbSchedNexts_of s) (tcbSchedPrevs_of s)\<rbrace>
-   tcbQueueRemove q t
-   \<lbrace>\<lambda>_ s. obj_at' (\<lambda>tcb. tcbSchedNext tcb = None \<and> tcbSchedPrev tcb = None) t s\<rbrace>"
-  apply (clarsimp simp: tcbQueueRemove_def)
-  apply (wpsimp wp: threadSet_wp getTCB_wp)
-  by (fastforce dest!: heap_ls_last_None
-                 simp: list_queue_relation_def prev_queue_head_def queue_end_valid_def
-                       obj_at'_def projectKOs opt_map_def ps_clear_def gen_objBits_simps
-                split: if_splits)
-
-lemma tcbSchedDequeue_tcbSchedNext_tcbSchedPrev_None_obj_at':
-  "\<lbrace>valid_sched_pointers\<rbrace>
-   tcbSchedDequeue t
-   \<lbrace>\<lambda>_ s. obj_at' (\<lambda>tcb. tcbSchedNext tcb = None \<and> tcbSchedPrev tcb = None) t s\<rbrace>"
-  unfolding tcbSchedDequeue_def
-  by (wpsimp wp: tcbQueueRemove_tcbSchedNext_tcbSchedPrev_None_obj_at' threadGet_wp)
-     (fastforce simp: ready_queue_relation_def ksReadyQueues_asrt_def obj_at'_def
-                      valid_sched_pointers_def opt_pred_def opt_map_def projectKOs
-               split: option.splits)
-
-crunch updateRestartPC, cancelIPC
-  for valid_sched_pointers[wp]: valid_sched_pointers
-  (simp: crunch_simps wp: crunch_wps)
-
-lemma setThreadState_tcbSchedNext_tcbSchedPrev_None_obj_at'[wp]:
-  "setThreadState ref ts \<lbrace>\<lambda>s. obj_at' (\<lambda>tcb. tcbSchedNext tcb = None \<and> tcbSchedPrev tcb = None) t s\<rbrace>"
-  unfolding setThreadState_def
-  apply (wpsimp wp: threadSet_wp getTCB_wp)
-  apply (fastforce simp: obj_at'_def gen_objBits_simps)
-  done
-
-lemma suspend_tcbSchedNext_tcbSchedPrev_None:
-  "\<lbrace>invs'\<rbrace> suspend t \<lbrace>\<lambda>_ s. obj_at' (\<lambda>tcb. tcbSchedNext tcb = None \<and> tcbSchedPrev tcb = None) t s\<rbrace>"
-  unfolding suspend_def
-  by (wpsimp wp: hoare_drop_imps tcbSchedDequeue_tcbSchedNext_tcbSchedPrev_None_obj_at')
-
-lemma (in delete_one_conc_pre) finaliseCap_replaceable:
-  "\<lbrace>\<lambda>s. invs' s \<and> cte_wp_at' (\<lambda>cte. cteCap cte = cap) slot s
-       \<and> (final_matters' cap \<longrightarrow> (final = isFinal cap slot (cteCaps_of s)))
-       \<and> weak_sch_act_wf (ksSchedulerAction s) s\<rbrace>
-     finaliseCap cap final flag
-   \<lbrace>\<lambda>rv s. (isNullCap (fst rv) \<and> removeable' slot s cap
-                \<and> (snd rv \<noteq> NullCap \<longrightarrow> snd rv = cap \<and> cap_has_cleanup' cap
-                                      \<and> isFinal cap slot (cteCaps_of s)))
-        \<or>
-          (isZombie (fst rv) \<and> snd rv = NullCap
-            \<and> isFinal cap slot (cteCaps_of s)
-            \<and> capClass cap = capClass (fst rv)
-            \<and> capUntypedPtr (fst rv) = capUntypedPtr cap
-            \<and> capBits (fst rv) = capBits cap
-            \<and> capRange (fst rv) = capRange cap
-            \<and> (isThreadCap cap \<or> isCNodeCap cap \<or> isZombie cap)
-            \<and> (\<forall>p \<in> threadCapRefs cap. st_tcb_at' ((=) Inactive) p s
-                     \<and> obj_at' (Not \<circ> tcbQueued) p s
-                     \<and> bound_tcb_at' ((=) None) p s
-                     \<and> obj_at' (\<lambda>tcb. tcbSchedNext tcb = None \<and> tcbSchedPrev tcb = None) p s))\<rbrace>"
-  apply (simp add: finaliseCap_def Let_def getThreadCSpaceRoot
-             cong: if_cong split del: if_split)
-  apply (rule hoare_pre)
-   apply (wp prepares_delete_helper'' [OF cancelAllIPC_unlive]
-             prepares_delete_helper'' [OF cancelAllSignals_unlive]
-             suspend_isFinal ARM.prepareThreadDelete_unqueued (* FIXME arch-split: interface *)
-             ARM.prepareThreadDelete_inactive prepareThreadDelete_isFinal
-             suspend_makes_inactive
-             deletingIRQHandler_removeable'
-             deletingIRQHandler_final[where slot=slot ]
-             unbindMaybeNotification_obj_at'_bound
-             getNotification_wp
-             suspend_bound_tcb_at'
-             unbindNotification_bound_tcb_at'
-             suspend_tcbSchedNext_tcbSchedPrev_None
-           | simp add: isZombie_Null isThreadCap_threadCapRefs_tcbptr
-                       isArchObjectCap_Cap_capCap
-           | (rule hoare_strengthen_post [OF arch_finaliseCap_removeable[where slot=slot]],
-              clarsimp simp: gen_isCap_simps)
-           | wpc)+
-
-  apply clarsimp
-  apply (frule cte_wp_at_valid_objs_valid_cap', clarsimp+)
-  apply (case_tac "cteCap cte",
-         simp_all add: gen_isCap_simps capRange_def cap_has_cleanup'_def
-                       final_matters'_def gen_objBits_simps
-                       not_Final_removeable finaliseCap_def,
-         simp_all add: removeable'_def)
-     (* thread *)
-     apply (frule capAligned_capUntypedPtr [OF valid_capAligned], simp)
-     apply (clarsimp simp: valid_cap'_def)
-     apply (drule valid_globals_cte_wpD'[rotated], clarsimp)
-     apply (clarsimp simp: invs'_def valid_state'_def valid_pspace'_def)
-    apply (clarsimp simp: obj_at'_def | rule conjI)+
-  done
-
-lemma cteDeleteOne_cte_wp_at_preserved:
-  assumes x: "\<And>cap final. P cap \<Longrightarrow> finaliseCap cap final True = fail"
-  shows "\<lbrace>\<lambda>s. cte_wp_at' (\<lambda>cte. P (cteCap cte)) p s\<rbrace>
-           cteDeleteOne ptr
-         \<lbrace>\<lambda>rv s. cte_wp_at' (\<lambda>cte. P (cteCap cte)) p s\<rbrace>"
-  apply (simp add: tree_cte_cteCap_eq[unfolded o_def])
-  apply (rule hoare_pre, wp cteDeleteOne_cteCaps_of)
-  apply (clarsimp simp: cteCaps_of_def cte_wp_at_ctes_of x)
-  done
-
-crunch cancelSignal
-  for ctes_of[wp]: "\<lambda>s. P (ctes_of s)"
-  (simp: crunch_simps wp: crunch_wps)
-
-lemma cancelIPC_cteCaps_of:
-  "\<lbrace>\<lambda>s. (\<forall>p. cte_wp_at' (\<lambda>cte. \<exists>final. finaliseCap (cteCap cte) final True \<noteq> fail) p s \<longrightarrow>
-          P ((cteCaps_of s)(p \<mapsto> NullCap))) \<and>
-     P (cteCaps_of s)\<rbrace>
-     cancelIPC t
-   \<lbrace>\<lambda>rv s. P (cteCaps_of s)\<rbrace>"
-  apply (simp add: cancelIPC_def Let_def capHasProperty_def
-                   getThreadReplySlot_def locateSlot_conv)
-  apply (rule hoare_pre)
-   apply (wp cteDeleteOne_cteCaps_of getCTE_wp' | wpcw
-        | simp add: cte_wp_at_ctes_of
-        | wp (once) hoare_drop_imps ctes_of_cteCaps_of_lift)+
-          apply (wp hoare_convert_imp hoare_vcg_all_lift
-                    threadSet_ctes_of threadSet_cteCaps_of
-               | clarsimp)+
-    apply (wp cteDeleteOne_cteCaps_of getCTE_wp' | wpcw | simp
-       | wp (once) hoare_drop_imps ctes_of_cteCaps_of_lift)+
-  apply (clarsimp simp: cte_wp_at_ctes_of cteCaps_of_def)
-  apply (drule_tac x="mdbNext (cteMDBNode x)" in spec)
-  apply clarsimp
-  apply (auto simp: o_def map_option_case fun_upd_def[symmetric])
-  done
-
-lemma cancelIPC_cte_wp_at':
-  assumes x: "\<And>cap final. P cap \<Longrightarrow> finaliseCap cap final True = fail"
-  shows "\<lbrace>\<lambda>s. cte_wp_at' (\<lambda>cte. P (cteCap cte)) p s\<rbrace>
-           cancelIPC t
-         \<lbrace>\<lambda>rv s. cte_wp_at' (\<lambda>cte. P (cteCap cte)) p s\<rbrace>"
-  apply (simp add: tree_cte_cteCap_eq[unfolded o_def])
-  apply (rule hoare_pre, wp cancelIPC_cteCaps_of)
-  apply (clarsimp simp: cteCaps_of_def cte_wp_at_ctes_of x)
-  done
-
-crunch tcbSchedDequeue
-  for cte_wp_at'[wp]: "cte_wp_at' P p"
-  (wp: crunch_wps)
-
-lemma suspend_cte_wp_at':
-  assumes x: "\<And>cap final. P cap \<Longrightarrow> finaliseCap cap final True = fail"
-  shows "\<lbrace>cte_wp_at' (\<lambda>cte. P (cteCap cte)) p\<rbrace>
-           suspend t
-         \<lbrace>\<lambda>rv. cte_wp_at' (\<lambda>cte. P (cteCap cte)) p\<rbrace>"
-  apply (simp add: suspend_def)
-  unfolding updateRestartPC_def
-  apply (rule hoare_pre)
-   apply (wp threadSet_cte_wp_at' cancelIPC_cte_wp_at'
-            | simp add: x)+
-  done
-
-context begin interpretation Arch . (*FIXME: arch-split*)
-
-crunch deleteASIDPool
-  for cte_wp_at'[wp]: "cte_wp_at' P p"
-  (simp: crunch_simps assertE_def
-   wp: crunch_wps getObject_inv loadObject_default_inv)
-
-lemma deleteASID_cte_wp_at'[wp]:
-  "\<lbrace>cte_wp_at' P p\<rbrace> deleteASID param_a param_b \<lbrace>\<lambda>_. cte_wp_at' P p\<rbrace>"
-  apply (simp add: deleteASID_def invalidateHWASIDEntry_def invalidateASID_def
-              cong: option.case_cong)
-  apply (wp setObject_cte_wp_at'[where Q="\<top>"] getObject_inv
-            loadObject_default_inv setVMRoot_cte_wp_at'
-          | clarsimp simp: updateObject_default_def in_monad
-                           projectKOs
-          | rule equals0I
-          | wpc)+
-  done
-
-crunch unmapPageTable, unmapPage, unbindNotification, finaliseCapTrue_standin
-  for cte_wp_at'[wp]: "cte_wp_at' P p"
-  (simp: crunch_simps wp: crunch_wps getObject_inv loadObject_default_inv)
-
-lemma arch_finaliseCap_cte_wp_at[wp]:
-  "\<lbrace>cte_wp_at' P p\<rbrace> Arch.finaliseCap cap fin \<lbrace>\<lambda>rv. cte_wp_at' P p\<rbrace>"
-  apply (simp add: ARM_H.finaliseCap_def)
-  apply (safe ; wpsimp wp: unmapPage_cte_wp_at')
-  done
-
-lemma deletingIRQHandler_cte_preserved:
-  assumes x: "\<And>cap final. P cap \<Longrightarrow> finaliseCap cap final True = fail"
-  shows "\<lbrace>cte_wp_at' (\<lambda>cte. P (cteCap cte)) p\<rbrace>
-           deletingIRQHandler irq
-         \<lbrace>\<lambda>rv. cte_wp_at' (\<lambda>cte. P (cteCap cte)) p\<rbrace>"
-  apply (simp add: deletingIRQHandler_def getSlotCap_def
-                   getIRQSlot_def locateSlot_conv getInterruptState_def)
-  apply (wp cteDeleteOne_cte_wp_at_preserved getCTE_wp'
-              | simp add: x)+
-  done
-
-lemma finaliseCap_equal_cap[wp]:
-  "\<lbrace>cte_wp_at' (\<lambda>cte. cteCap cte = cap) sl\<rbrace>
-     finaliseCap cap fin flag
-   \<lbrace>\<lambda>rv. cte_wp_at' (\<lambda>cte. cteCap cte = cap) sl\<rbrace>"
-  apply (simp add: finaliseCap_def Let_def
-             cong: if_cong split del: if_split)
-  apply (rule hoare_pre)
-   apply (wp suspend_cte_wp_at' deletingIRQHandler_cte_preserved
-        | clarsimp simp: finaliseCap_def | wpc)+
-  apply (case_tac cap)
-  apply auto
-  done
-
-lemma setThreadState_st_tcb_at_simplish':
-  "simple' st \<Longrightarrow>
-   \<lbrace>st_tcb_at' (P or simple') t\<rbrace>
-     setThreadState st t'
-   \<lbrace>\<lambda>rv. st_tcb_at' (P or simple') t\<rbrace>"
-  apply (wp sts_st_tcb_at'_cases)
-  apply clarsimp
-  done
-
-lemmas setThreadState_st_tcb_at_simplish
-    = setThreadState_st_tcb_at_simplish'[unfolded pred_disj_def]
-
-crunch cteDeleteOne
-  for st_tcb_at_simplish: "st_tcb_at' (\<lambda>st. P st \<or> simple' st) t"
-  (wp: crunch_wps getObject_inv loadObject_default_inv threadSet_pred_tcb_no_state
-   simp: crunch_simps unless_def)
-
-lemma cteDeleteOne_st_tcb_at[wp]:
-  assumes x[simp]: "\<And>st. simple' st \<longrightarrow> P st" shows
-  "\<lbrace>st_tcb_at' P t\<rbrace> cteDeleteOne slot \<lbrace>\<lambda>rv. st_tcb_at' P t\<rbrace>"
-  apply (subgoal_tac "\<exists>Q. P = (Q or simple')")
-   apply (clarsimp simp: pred_disj_def)
-   apply (rule cteDeleteOne_st_tcb_at_simplish)
-  apply (rule_tac x=P in exI)
-  apply (auto intro!: ext)
-  done
-
-lemma cteDeleteOne_reply_pred_tcb_at:
-  "\<lbrace>\<lambda>s. pred_tcb_at' proj P t s \<and> (\<exists>t' r. cte_wp_at' (\<lambda>cte. cteCap cte = ReplyCap t' False r) slot s)\<rbrace>
-    cteDeleteOne slot
-   \<lbrace>\<lambda>rv. pred_tcb_at' proj P t\<rbrace>"
-  apply (simp add: cteDeleteOne_def unless_def isFinalCapability_def)
-  apply (rule bind_wp [OF _ getCTE_sp])
-  apply (rule hoare_assume_pre)
-  apply (clarsimp simp: cte_wp_at_ctes_of when_def isCap_simps
-                        Let_def finaliseCapTrue_standin_def)
-  apply (intro impI conjI, (wp | simp)+)
-  done
-
-context
-notes option.case_cong_weak[cong]
-begin
-crunch cteDeleteOne, unbindNotification
-  for sch_act_simple[wp]: sch_act_simple
-  (wp: crunch_wps ssa_sch_act_simple sts_sch_act_simple getObject_inv
-       loadObject_default_inv
-   simp: crunch_simps unless_def
-   rule: sch_act_simple_lift)
-end
-
-lemma rescheduleRequired_sch_act_not[wp]:
-  "\<lbrace>\<top>\<rbrace> rescheduleRequired \<lbrace>\<lambda>rv. sch_act_not t\<rbrace>"
-  apply (simp add: rescheduleRequired_def setSchedulerAction_def)
-  apply (wp hoare_TrueI | simp)+
-  done
-
-crunch cteDeleteOne
-  for sch_act_not[wp]: "sch_act_not t"
-  (simp: crunch_simps case_Null_If unless_def
-   wp: crunch_wps getObject_inv loadObject_default_inv)
-
-lemma cancelAllIPC_mapM_x_weak_sch_act:
-  "\<lbrace>\<lambda>s. weak_sch_act_wf (ksSchedulerAction s) s\<rbrace>
-   mapM_x (\<lambda>t. do
-                 y \<leftarrow> setThreadState Structures_H.thread_state.Restart t;
-                 tcbSchedEnqueue t
-               od) q
-   \<lbrace>\<lambda>rv s. weak_sch_act_wf (ksSchedulerAction s) s\<rbrace>"
-  apply (rule mapM_x_wp_inv)
-  apply (wp)
-  apply (clarsimp)
-  done
-
-lemma cancelAllIPC_mapM_x_valid_objs':
-  "\<lbrace>valid_objs' and pspace_aligned' and pspace_distinct'\<rbrace>
-   mapM_x (\<lambda>t. do
-                 y \<leftarrow> setThreadState Structures_H.thread_state.Restart t;
-                 tcbSchedEnqueue t
-               od) q
-   \<lbrace>\<lambda>_. valid_objs'\<rbrace>"
-  apply (rule hoare_strengthen_post)
-   apply (rule mapM_x_wp')
-  apply (wpsimp wp: sts_valid_objs')
-   apply (clarsimp simp: valid_tcb_state'_def)+
-  done
-
-lemma cancelAllIPC_mapM_x_tcbDomain_obj_at':
-  "\<lbrace>obj_at' (\<lambda>tcb. P (tcbDomain tcb)) t'\<rbrace>
-   mapM_x (\<lambda>t. do
-                 y \<leftarrow> setThreadState Structures_H.thread_state.Restart t;
-                 tcbSchedEnqueue t
-               od) q
-  \<lbrace>\<lambda>_. obj_at' (\<lambda>tcb. P (tcbDomain tcb)) t'\<rbrace>"
-  by (wpsimp wp: mapM_x_wp')
-
-lemma rescheduleRequired_oa_queued':
-  "rescheduleRequired \<lbrace>obj_at' (\<lambda>tcb. Q (tcbDomain tcb) (tcbPriority tcb)) t\<rbrace>"
-  unfolding rescheduleRequired_def tcbSchedEnqueue_def tcbQueuePrepend_def
-  by wpsimp
-
-lemma cancelAllIPC_tcbDomain_obj_at':
-  "\<lbrace>obj_at' (\<lambda>tcb. P (tcbDomain tcb)) t'\<rbrace>
-     cancelAllIPC epptr
-   \<lbrace>\<lambda>_. obj_at' (\<lambda>tcb. P (tcbDomain tcb)) t'\<rbrace>"
-apply (simp add: cancelAllIPC_def)
-apply (wp hoare_vcg_conj_lift hoare_vcg_const_Ball_lift
-          rescheduleRequired_oa_queued' cancelAllIPC_mapM_x_tcbDomain_obj_at'
-          getEndpoint_wp
-     | wpc
-     | simp)+
-done
-
-lemma cancelAllSignals_tcbDomain_obj_at':
-  "\<lbrace>obj_at' (\<lambda>tcb. P (tcbDomain tcb)) t'\<rbrace>
-     cancelAllSignals epptr
-   \<lbrace>\<lambda>_. obj_at' (\<lambda>tcb. P (tcbDomain tcb)) t'\<rbrace>"
-apply (simp add: cancelAllSignals_def)
-apply (wp hoare_vcg_conj_lift hoare_vcg_const_Ball_lift
-          rescheduleRequired_oa_queued' cancelAllIPC_mapM_x_tcbDomain_obj_at'
-          getNotification_wp
-     | wpc
-     | simp)+
-done
-
-lemma unbindMaybeNotification_tcbDomain_obj_at':
-  "\<lbrace>obj_at' (\<lambda>tcb. P (tcbDomain tcb)) t'\<rbrace>
-     unbindMaybeNotification r
-   \<lbrace>\<lambda>_. obj_at' (\<lambda>tcb. P (tcbDomain tcb)) t'\<rbrace>"
-  unfolding unbindMaybeNotification_def
-  by (wpsimp wp: getNotification_wp gbn_wp' simp: setBoundNotification_def)+
-
-crunch isFinalCapability
-  for sch_act[wp]: "\<lambda>s. sch_act_wf (ksSchedulerAction s) s"
-  (simp: crunch_simps)
-
-crunch
-  isFinalCapability
-  for weak_sch_act[wp]: "\<lambda>s. weak_sch_act_wf (ksSchedulerAction s) s"
-  (simp: crunch_simps)
-
-crunch cteDeleteOne
-  for ksCurDomain[wp]: "\<lambda>s. P (ksCurDomain s)"
-  (wp: crunch_wps simp: crunch_simps unless_def)
-
-lemma cteDeleteOne_tcbDomain_obj_at':
-  "\<lbrace>obj_at' (\<lambda>tcb. P (tcbDomain tcb)) t'\<rbrace> cteDeleteOne slot \<lbrace>\<lambda>_. obj_at' (\<lambda>tcb. P (tcbDomain tcb)) t'\<rbrace>"
-  apply (simp add: cteDeleteOne_def unless_def split_def)
-  apply (wp emptySlot_tcbDomain cancelAllIPC_tcbDomain_obj_at' cancelAllSignals_tcbDomain_obj_at'
-          isFinalCapability_inv getCTE_wp
-          unbindMaybeNotification_tcbDomain_obj_at'
-     | rule hoare_drop_imp
-     | simp add: finaliseCapTrue_standin_def Let_def
-            split del: if_split
-     | wpc)+
-  apply (clarsimp simp: cte_wp_at'_def)
-  done
-
-end
-
-global_interpretation delete_one_conc_pre
-  by (unfold_locales, wp) (wp cteDeleteOne_tcbDomain_obj_at' cteDeleteOne_typ_at' cteDeleteOne_reply_pred_tcb_at | simp)+
-
-context begin interpretation Arch . (*FIXME: arch-split*)
-
-lemma cteDeleteOne_invs[wp]:
-  "\<lbrace>invs'\<rbrace> cteDeleteOne ptr \<lbrace>\<lambda>rv. invs'\<rbrace>"
-  apply (simp add: cteDeleteOne_def unless_def
-                   split_def finaliseCapTrue_standin_simple_def)
-  apply wp
-    apply (rule hoare_strengthen_post)
-     apply (rule hoare_vcg_conj_lift)
-      apply (rule finaliseCap_True_invs)
-     apply (rule hoare_vcg_conj_lift)
-      apply (rule finaliseCap_replaceable[where slot=ptr])
-     apply (rule hoare_vcg_conj_lift)
-      apply (rule finaliseCap_cte_refs)
-     apply (rule finaliseCap_equal_cap[where sl=ptr])
-    apply (clarsimp simp: cte_wp_at_ctes_of)
-    apply (erule disjE)
-     apply simp
-    apply (clarsimp dest!: isCapDs simp: capRemovable_def)
-    apply (clarsimp simp: removeable'_def fun_eq_iff[where f="cte_refs' cap" for cap]
-                     del: disjCI)
-    apply (rule disjI2)
-    apply (rule conjI)
-     subgoal by auto
-    subgoal by (auto dest!: isCapDs simp: pred_tcb_at'_def obj_at'_def projectKOs
-                                          live'_def hyp_live'_def ko_wp_at'_def)
-   apply (wp isFinalCapability_inv getCTE_wp' hoare_weak_lift_imp
-        | wp (once) isFinal[where x=ptr])+
-  apply (fastforce simp: cte_wp_at_ctes_of)
-  done
-
-end
-
-global_interpretation delete_one_conc_fr: delete_one_conc
-  by unfold_locales wp
-
-declare cteDeleteOne_invs[wp]
-
-lemma deletingIRQHandler_invs' [wp]:
-  "\<lbrace>invs'\<rbrace> deletingIRQHandler i \<lbrace>\<lambda>_. invs'\<rbrace>"
-  apply (simp add: deletingIRQHandler_def getSlotCap_def
-                   getIRQSlot_def locateSlot_conv getInterruptState_def)
-  apply (wp getCTE_wp')
-  apply simp
-  done
-
-crunch unbindNotification, unbindMaybeNotification
-  for tcb_at'[wp]: "tcb_at' t"
-
-lemma finaliseCap_invs:
-  "\<lbrace>invs' and sch_act_simple and valid_cap' cap
-         and cte_wp_at' (\<lambda>cte. cteCap cte = cap) sl\<rbrace>
-     finaliseCap cap fin flag
-   \<lbrace>\<lambda>rv. invs'\<rbrace>"
-  apply (simp add: finaliseCap_def Let_def
-             cong: if_cong split del: if_split)
-  apply (rule hoare_pre)
-   apply (wp hoare_drop_imps hoare_vcg_all_lift | simp only: o_def | wpc)+
-
-  apply clarsimp
-  apply (intro conjI impI)
-    apply (clarsimp dest!: isCapDs simp: valid_cap'_def)
-   apply (drule invs_valid_global', drule(1) valid_globals_cte_wpD')
-   apply (drule valid_capAligned, drule capAligned_capUntypedPtr)
-    apply (clarsimp dest!: isCapDs)
-   apply (clarsimp dest!: isCapDs)
-  apply (clarsimp dest!: isCapDs)
-  done
-
-lemma finaliseCap_zombie_cap[wp]:
-  "\<lbrace>cte_wp_at' (\<lambda>cte. (P and isZombie) (cteCap cte)) sl\<rbrace>
-     finaliseCap cap fin flag
-   \<lbrace>\<lambda>rv. cte_wp_at' (\<lambda>cte. (P and isZombie) (cteCap cte)) sl\<rbrace>"
-  apply (simp add: finaliseCap_def Let_def
-             cong: if_cong split del: if_split)
-  apply (rule hoare_pre)
-   apply (wp suspend_cte_wp_at' deletingIRQHandler_cte_preserved
-          | clarsimp simp: finaliseCap_def gen_isCap_simps | wpc)+
-  done
-
-lemma finaliseCap_zombie_cap':
-  "\<lbrace>cte_wp_at' (\<lambda>cte. (P and isZombie) (cteCap cte)) sl\<rbrace>
-     finaliseCap cap fin flag
-   \<lbrace>\<lambda>rv. cte_wp_at' (\<lambda>cte. P (cteCap cte)) sl\<rbrace>"
-  apply (rule hoare_strengthen_post)
-   apply (rule finaliseCap_zombie_cap)
-  apply (clarsimp simp: cte_wp_at_ctes_of)
-  done
-
-lemma finaliseCap_cte_cap_wp_to[wp]:
-  "\<lbrace>ex_cte_cap_wp_to' P sl\<rbrace> finaliseCap cap fin flag \<lbrace>\<lambda>rv. ex_cte_cap_wp_to' P sl\<rbrace>"
-  apply (simp add: ex_cte_cap_to'_def)
-  apply (rule hoare_pre, rule hoare_use_eq_irq_node' [OF finaliseCap_irq_node'])
-   apply (simp add: finaliseCap_def Let_def
-              cong: if_cong split del: if_split)
-   apply (wp suspend_cte_wp_at'
-             deletingIRQHandler_cte_preserved
-             hoare_vcg_ex_lift
-                 | clarsimp simp: finaliseCap_def gen_isCap_simps
-                 | rule conjI
-                 | wpc)+
-  apply fastforce
-  done
-
-context
-notes option.case_cong_weak[cong]
-begin
-crunch unbindNotification
-  for valid_cap'[wp]: "valid_cap' cap"
-end
-
-lemma finaliseCap_valid_cap[wp]:
-  "\<lbrace>valid_cap' cap\<rbrace> finaliseCap cap final flag \<lbrace>\<lambda>rv. valid_cap' (fst rv)\<rbrace>"
-  apply (simp add: finaliseCap_def Let_def
-                   getThreadCSpaceRoot
-                   ARM_H.finaliseCap_def
-             cong: if_cong split del: if_split)
-  apply (rule hoare_pre)
-   apply (wp | simp only: valid_NullCap o_def fst_conv | wpc)+
-  apply simp
-  apply (intro conjI impI)
-   apply (clarsimp simp: valid_cap'_def gen_isCap_simps capAligned_def
-                         ARM.objBits_simps shiftL_nat)+
-  done
-
-
-context begin interpretation Arch . (*FIXME: arch-split*)
-
-crunch "Arch.finaliseCap"
+lemma arch_recycleCap_improve_cases:
+  "\<lbrakk>\<not> isPageCap cap; \<not> isPageTableCap cap; \<not> isPageDirectoryCap cap;\<not> isVCPUCap cap;
+    \<not> isASIDControlCap cap; \<not>isSGISignalCap cap \<rbrakk> \<Longrightarrow>
+   (if isASIDPoolCap cap then v else undefined) = v"
+  by (cases cap, simp_all add: isCap_simps)
+
+crunch invalidateTLBByASID
   for nosch[wp]: "\<lambda>s. P (ksSchedulerAction s)"
-  (wp: crunch_wps getObject_inv simp: loadObject_default_def updateObject_default_def)
 
-crunch finaliseCap
+crunch unmapPageTable
+  for nosch[wp]: "\<lambda>s. P (ksSchedulerAction s)"
+  (wp: crunch_wps getObject_inv hoare_vcg_all_lift hoare_vcg_if_lift3
+   simp: loadObject_default_def updateObject_default_def)
+
+context notes if_cong[cong] begin
+
+crunch Arch_finaliseCap
+  for nosch[wp]: "\<lambda>s. P (ksSchedulerAction s)"
+  (wp: crunch_wps getObject_inv simp: loadObject_default_def updateObject_default_def
+   rule: ARM_H.finaliseCap_def)
+
+end
+
+crunch deletingIRQHandler, finaliseCap
   for sch_act_simple[wp]: sch_act_simple
   (simp: crunch_simps
    rule: sch_act_simple_lift
    wp: getObject_inv loadObject_default_inv crunch_wps)
 
-end
-
-
-lemma interrupt_cap_null_or_ntfn:
-  "invs s
-    \<Longrightarrow> cte_wp_at (\<lambda>cp. is_ntfn_cap cp \<or> cp = cap.NullCap) (interrupt_irq_node s irq, []) s"
-  apply (frule invs_valid_irq_node)
-  apply (clarsimp simp: valid_irq_node_def)
-  apply (drule_tac x=irq in spec)
-  apply (drule cte_at_0)
-  apply (clarsimp simp: cte_wp_at_caps_of_state)
-  apply (drule caps_of_state_cteD)
-  apply (frule if_unsafe_then_capD, clarsimp+)
-  apply (clarsimp simp: ex_cte_cap_wp_to_def cte_wp_at_caps_of_state)
-  apply (frule cte_refs_obj_refs_elem, erule disjE)
-   apply (clarsimp | drule caps_of_state_cteD valid_global_refsD[rotated]
-     | rule irq_node_global_refs[where irq=irq])+
-   apply (simp add: cap_range_def)
-  apply (clarsimp simp: appropriate_cte_cap_def
-                 split: cap.split_asm)
-  done
-
-lemma (in delete_one) deletingIRQHandler_corres:
-  "corres dc (einvs) (invs')
-          (deleting_irq_handler irq) (deletingIRQHandler irq)"
-  apply (simp add: deleting_irq_handler_def deletingIRQHandler_def)
-  apply (rule corres_guard_imp)
-    apply (rule corres_split[OF getIRQSlot_corres])
-      apply simp
-      apply (rule_tac P'="cte_at' (cte_map slot)" in corres_symb_exec_r_conj)
-         apply (rule_tac F="isNotificationCap rv \<or> rv = capability.NullCap"
-             and P="cte_wp_at (\<lambda>cp. is_ntfn_cap cp \<or> cp = cap.NullCap) slot
-                 and einvs"
-             and P'="invs' and cte_wp_at' (\<lambda>cte. cteCap cte = rv)
-                 (cte_map slot)" in corres_req)
-          apply (clarsimp simp: cte_wp_at_caps_of_state state_relation_def)
-          apply (drule caps_of_state_cteD)
-          apply (drule(1) pspace_relation_cte_wp_at, clarsimp+)
-          apply (auto simp: cte_wp_at_ctes_of is_cap_simps gen_isCap_simps)[1]
-         apply simp
-         apply (rule corres_guard_imp, rule delete_one_corres[unfolded dc_def])
-          apply (auto simp: cte_wp_at_caps_of_state is_cap_simps can_fast_finalise_def)[1]
-         apply (clarsimp simp: cte_wp_at_ctes_of)
-        apply (wp getCTE_wp' | simp add: getSlotCap_def)+
-     apply (wp | simp add: get_irq_slot_def getIRQSlot_def
-                           locateSlot_conv getInterruptState_def)+
-   apply (clarsimp simp: ex_cte_cap_wp_to_def interrupt_cap_null_or_ntfn)
-  apply (clarsimp simp: cte_wp_at_ctes_of)
-  done
-
-context begin interpretation Arch . (*FIXME: arch-split*)
-
-lemma arch_finaliseCap_corres:
+lemma arch_finaliseCap_corres[Finalise_R_3_assms]:
   "\<lbrakk> final_matters' (ArchObjectCap cap') \<Longrightarrow> final = final'; acap_relation cap cap' \<rbrakk>
      \<Longrightarrow> corres (\<lambda>r r'. cap_relation (fst r) (fst r') \<and> cap_relation (snd r) (snd r'))
            (\<lambda>s. invs s \<and> s \<turnstile> cap.ArchObjectCap cap
@@ -3405,13 +1246,11 @@ lemma arch_finaliseCap_corres:
                  (final_matters' (ArchObjectCap cap') \<longrightarrow>
                       final' = isFinal (ArchObjectCap cap') (cte_map sl) (cteCaps_of s)))
            (arch_finalise_cap cap final) (Arch.finaliseCap cap' final')"
-  apply (cases cap;
-        clarsimp simp: arch_finalise_cap_def ARM_H.finaliseCap_def
-                       final_matters'_def case_bool_If liftM_def[symmetric]
-                       isASIDPoolCap_def isPageCap_def isPageDirectoryCap_def
-                       isPageTableCap_def
+  apply (cases cap,
+         simp_all add: arch_finalise_cap_def ARM_H.finaliseCap_def isCap_simps
+                       final_matters'_def arch_final_matters'_def case_bool_If liftM_def[symmetric]
                        o_def dc_def[symmetric]
-                split: option.split)
+                split: option.split, safe)
      apply (rule corres_guard_imp, rule deleteASIDPool_corres)
       apply (clarsimp simp: valid_cap_def mask_def)
      apply (clarsimp simp: valid_cap'_def)
@@ -3420,336 +1259,22 @@ lemma arch_finaliseCap_corres:
       apply simp
      apply (clarsimp simp: valid_cap_def valid_unmap_def)
      apply (auto simp: vmsz_aligned_def pbfs_atleast_pageBits mask_def
-                 elim: is_aligned_weaken invs_valid_asid_map)[2]
+                 elim: is_aligned_weaken)[2]
    apply (rule corres_guard_imp, rule unmapPageTable_corres)
     apply (auto simp: valid_cap_def valid_cap'_def mask_def
-               elim!: is_aligned_weaken invs_valid_asid_map)[2]
+               elim!: is_aligned_weaken)[2]
   apply (rule corres_guard_imp, rule deleteASID_corres)
-   apply (auto elim!: invs_valid_asid_map simp: mask_def valid_cap_def)[2]
+   apply (auto simp: mask_def valid_cap_def)[2]
   done
 
-lemma unbindNotification_corres:
-  "corres dc
-      (invs and tcb_at t)
-      invs'
-      (unbind_notification t)
-      (unbindNotification t)"
-  apply (simp add: unbind_notification_def unbindNotification_def)
-  apply (rule corres_guard_imp)
-    apply (rule corres_split[OF getBoundNotification_corres])
-      apply (rule corres_option_split)
-        apply simp
-       apply (rule corres_return_trivial)
-      apply (rule corres_split[OF getNotification_corres])
-        apply clarsimp
-        apply (rule corres_split[OF setNotification_corres])
-           apply (clarsimp simp: ntfn_relation_def split:Structures_A.ntfn.splits)
-          apply (rule setBoundNotification_corres)
-         apply (wp gbn_wp' gbn_wp)+
-   apply (clarsimp elim!: obj_at_valid_objsE
-                   dest!: bound_tcb_at_state_refs_ofD invs_valid_objs
-                    simp: valid_obj_def is_tcb tcb_ntfn_is_bound_def obj_at_def
-                          valid_tcb_def valid_bound_ntfn_def invs_psp_aligned invs_distinct
-                   split: option.splits)
-  apply (clarsimp dest!: obj_at_valid_objs' bound_tcb_at_state_refs_ofD' invs_valid_objs'
-                   simp: valid_obj'_def valid_tcb'_def valid_bound_ntfn'_def tcb_ntfn_is_bound'_def
-                         projectKOs
-                  split: option.splits)
-  done
+lemmas deleteCallerCap_typ_ats[wp] = typ_at_lifts[OF deleteCallerCap_typ_at']
 
-lemma unbindMaybeNotification_corres:
-  "corres dc
-      (invs and ntfn_at ntfnptr) (invs' and ntfn_at' ntfnptr)
-      (unbind_maybe_notification ntfnptr)
-      (unbindMaybeNotification ntfnptr)"
-  apply (simp add: unbind_maybe_notification_def unbindMaybeNotification_def
-              cong: option.case_cong)
-  apply (rule corres_guard_imp)
-    apply (rule corres_split[OF getNotification_corres])
-      apply (rule corres_option_split)
-        apply (clarsimp simp: ntfn_relation_def split: Structures_A.ntfn.splits)
-       apply (rule corres_return_trivial)
-      apply (rule corres_split[OF setNotification_corres])
-         apply (clarsimp simp: ntfn_relation_def split: Structures_A.ntfn.splits)
-        apply (rule setBoundNotification_corres)
-       apply (wp get_simple_ko_wp getNotification_wp)+
-   apply (clarsimp elim!: obj_at_valid_objsE
-                   dest!: bound_tcb_at_state_refs_ofD invs_valid_objs
-                    simp: valid_obj_def is_tcb tcb_ntfn_is_bound_def invs_psp_aligned invs_distinct
-                          valid_tcb_def valid_bound_ntfn_def valid_ntfn_def
-                   split: option.splits)
-  apply (clarsimp dest!: obj_at_valid_objs' bound_tcb_at_state_refs_ofD' invs_valid_objs'
-                   simp: valid_obj'_def valid_tcb'_def valid_bound_ntfn'_def
-                         tcb_ntfn_is_bound'_def valid_ntfn'_def
-                  split: option.splits)
-  done
+end (* Arch *)
 
-lemma fast_finaliseCap_corres:
-  "\<lbrakk> final_matters' cap' \<longrightarrow> final = final'; cap_relation cap cap';
-     can_fast_finalise cap \<rbrakk>
-   \<Longrightarrow> corres dc
-           (\<lambda>s. invs s \<and> valid_sched s \<and> s \<turnstile> cap
-                       \<and> cte_wp_at ((=) cap) sl s)
-           (\<lambda>s. invs' s \<and> s \<turnstile>' cap')
-           (fast_finalise cap final)
-           (do
-               p \<leftarrow> finaliseCap cap' final' True;
-               assert (capRemovable (fst p) (cte_map ptr) \<and> snd p = NullCap)
-            od)"
-  apply (cases cap, simp_all add: finaliseCap_def isCap_simps
-                                  corres_liftM2_simp[unfolded liftM_def]
-                                  o_def dc_def[symmetric] when_def
-                                  can_fast_finalise_def capRemovable_def
-                       split del: if_split cong: if_cong)
-   apply (clarsimp simp: final_matters'_def)
-   apply (rule corres_guard_imp)
-     apply (rule corres_rel_imp)
-      apply (rule ep_cancel_corres)
-     apply simp
-    apply (simp add: valid_cap_def)
-   apply (simp add: valid_cap'_def)
-  apply (clarsimp simp: final_matters'_def)
-  apply (rule corres_guard_imp)
-    apply (rule corres_split[OF unbindMaybeNotification_corres])
-         apply (rule cancelAllSignals_corres)
-       apply (wp abs_typ_at_lifts unbind_maybe_notification_invs typ_at_lifts hoare_drop_imps getNotification_wp
-            | wpc)+
-   apply (clarsimp simp: valid_cap_def)
-  apply (clarsimp simp: valid_cap'_def projectKOs valid_obj'_def
-                 dest!: invs_valid_objs' obj_at_valid_objs' )
-  done
-
-lemma cap_delete_one_corres:
-  "corres dc (einvs and cte_wp_at can_fast_finalise ptr)
-        (invs' and cte_at' (cte_map ptr))
-        (cap_delete_one ptr) (cteDeleteOne (cte_map ptr))"
-  apply (simp add: cap_delete_one_def cteDeleteOne_def'
-                   unless_def when_def)
-  apply (rule corres_guard_imp)
-    apply (rule corres_split[OF get_cap_corres])
-      apply (rule_tac F="can_fast_finalise cap" in corres_gen_asm)
-      apply (rule corres_if)
-        apply fastforce
-       apply (rule corres_split[OF isFinalCapability_corres[where ptr=ptr]])
-         apply (simp add: split_def bind_assoc [THEN sym])
-         apply (rule corres_split[OF fast_finaliseCap_corres[where sl=ptr]])
-              apply simp+
-           apply (rule emptySlot_corres, simp)
-          apply (wp hoare_drop_imps)+
-       apply (wp isFinalCapability_inv | wp (once) isFinal[where x="cte_map ptr"])+
-      apply (rule corres_trivial, simp)
-     apply (wp get_cap_wp getCTE_wp)+
-   apply (clarsimp simp: cte_wp_at_caps_of_state can_fast_finalise_Null
-                  elim!: caps_of_state_valid_cap)
-  apply (clarsimp simp: cte_wp_at_ctes_of)
-  apply fastforce
-  done
-end
-(* FIXME: strengthen locale instead *)
-
-global_interpretation delete_one
-  apply unfold_locales
-  apply (rule corres_guard_imp)
-    apply (rule cap_delete_one_corres)
-   apply auto
-  done
-
-lemma no_idle_thread_cap:
-  "\<lbrakk> cte_wp_at ((=) (cap.ThreadCap (idle_thread s))) sl s; valid_global_refs s \<rbrakk> \<Longrightarrow> False"
-  apply (cases sl)
-  apply (clarsimp simp: valid_global_refs_def valid_refs_def cte_wp_at_caps_of_state)
-  apply ((erule allE)+, erule (1) impE)
-  apply (clarsimp simp: cap_range_def)
-  done
-
-lemmas getCTE_no_0_obj'_helper
-  = getCTE_inv
-    hoare_strengthen_post[where Q'="\<lambda>_. no_0_obj'" and P=no_0_obj' and f="getCTE slot" for slot]
-
-context begin interpretation Arch . (*FIXME: arch-split*)
-context
-notes option.case_cong_weak[cong]
-begin
-crunch ThreadDecls_H.suspend, unbindNotification
-  for no_0_obj'[wp]: no_0_obj'
-  (simp: crunch_simps wp: crunch_wps getCTE_no_0_obj'_helper)
-end
-end
-
-lemma finaliseCap_corres:
-  "\<lbrakk> final_matters' cap' \<Longrightarrow> final = final'; cap_relation cap cap';
-          flag \<longrightarrow> can_fast_finalise cap \<rbrakk>
-     \<Longrightarrow> corres (\<lambda>x y. cap_relation (fst x) (fst y) \<and> cap_relation (snd x) (snd y))
-           (\<lambda>s. einvs s \<and> s \<turnstile> cap \<and> (final_matters cap \<longrightarrow> final = is_final_cap' cap s)
-                       \<and> cte_wp_at ((=) cap) sl s)
-           (\<lambda>s. invs' s \<and> s \<turnstile>' cap' \<and>
-                 (final_matters' cap' \<longrightarrow>
-                      final' = isFinal cap' (cte_map sl) (cteCaps_of s)))
-           (finalise_cap cap final) (finaliseCap cap' final' flag)"
-  supply invs_no_0_obj'[simp]
-  apply (cases cap, simp_all add: finaliseCap_def gen_isCap_simps
-                                  corres_liftM2_simp[unfolded liftM_def]
-                                  o_def dc_def[symmetric] when_def
-                                  can_fast_finalise_def
-                       split del: if_split cong: if_cong)
-        apply (clarsimp simp: final_matters'_def)
-        apply (rule corres_guard_imp)
-          apply (rule ep_cancel_corres)
-         apply (simp add: valid_cap_def)
-        apply (simp add: valid_cap'_def)
-       apply (clarsimp simp add: final_matters'_def)
-       apply (rule corres_guard_imp)
-         apply (rule corres_split[OF unbindMaybeNotification_corres])
-           apply (rule cancelAllSignals_corres)
-          apply (wp abs_typ_at_lifts unbind_maybe_notification_invs gen_typ_at_lifts hoare_drop_imps hoare_vcg_all_lift | wpc)+
-        apply (clarsimp simp: valid_cap_def)
-       apply (clarsimp simp: valid_cap'_def)
-      apply (fastforce simp: final_matters'_def shiftL_nat zbits_map_def)
-     apply (clarsimp simp add: final_matters'_def getThreadCSpaceRoot
-                               liftM_def[symmetric] o_def zbits_map_def
-                               dc_def[symmetric])
-     apply (rename_tac t)
-     apply (rule_tac P="\<lambda>s. t \<noteq> idle_thread s" and P'="\<lambda>s. t \<noteq> ksIdleThread s" in corres_add_guard)
-      apply clarsimp
-      apply (rule context_conjI)
-       apply (clarsimp dest!: no_idle_thread_cap)
-      apply (clarsimp simp: state_relation_def)
-     apply (rule corres_guard_imp)
-       apply (rule corres_split[OF unbindNotification_corres])
-         apply (rule corres_split[OF suspend_corres])
-            apply (clarsimp simp: liftM_def[symmetric] o_def dc_def[symmetric] zbits_map_def)
-          apply (rule ARM.prepareThreadDelete_corres, rule refl) (* FIXME arch-split: interface *)
-        apply (wp unbind_notification_invs unbind_notification_simple_sched_action)+
-      apply (simp add: valid_cap_def)
-     apply (simp add: valid_cap'_def)
-    apply (simp add: final_matters'_def liftM_def[symmetric]
-                     o_def dc_def[symmetric])
-    apply (intro impI, rule corres_guard_imp)
-      apply (rule deletingIRQHandler_corres)
-     apply simp
-    apply simp
-   apply (clarsimp simp: final_matters'_def)
-   apply (rule_tac F="False" in corres_req)
-    apply clarsimp
-    apply (frule zombies_finalD, (clarsimp simp: is_cap_simps)+)
-    apply (clarsimp simp: cte_wp_at_caps_of_state)
-   apply simp
-  apply (clarsimp split del: if_split simp: o_def)
-  apply (rule corres_guard_imp [OF arch_finaliseCap_corres], (fastforce simp: valid_sched_def)+)
-  done
-
-context begin interpretation Arch . (*FIXME: arch-split*)
-
-crunch copyGlobalMappings
-  for ifunsafe'[wp]: "if_unsafe_then_cap'"
-  (wp: crunch_wps ignore: storePDE)
-
-crunch copyGlobalMappings
-  for pred_tcb_at'[wp]: "pred_tcb_at' proj P t"
-  (wp: crunch_wps ignore: storePDE)
-
-crunch copyGlobalMappings
-  for vms'[wp]: "valid_machine_state'"
-  (wp: crunch_wps ignore: storePDE)
-
-crunch copyGlobalMappings
-  for ct_not_inQ[wp]: "ct_not_inQ"
-  (wp: crunch_wps ignore: storePDE)
-
-crunch copyGlobalMappings
-  for tcb_in_cur_domain'[wp]: "tcb_in_cur_domain' t"
-  (wp: crunch_wps)
-
-crunch copyGlobalMappings
-  for ct__in_cur_domain'[wp]: ct_idle_or_in_cur_domain'
-  (wp: crunch_wps)
-
-crunch copyGlobalMappings
-  for gsUntypedZeroRanges[wp]: "\<lambda>s. P (gsUntypedZeroRanges s)"
-  (wp: crunch_wps)
-
-lemma threadSet_ct_idle_or_in_cur_domain':
-  "\<lbrace>ct_idle_or_in_cur_domain' and (\<lambda>s. \<forall>tcb. tcbDomain tcb = ksCurDomain s \<longrightarrow> tcbDomain (F tcb) = ksCurDomain s)\<rbrace>
-    threadSet F t
-   \<lbrace>\<lambda>_. ct_idle_or_in_cur_domain'\<rbrace>"
-apply (simp add: ct_idle_or_in_cur_domain'_def tcb_in_cur_domain'_def)
-apply (wp hoare_vcg_disj_lift hoare_vcg_imp_lift)
-  apply wps
-  apply wp
- apply wps
- apply wp
-apply (auto simp: obj_at'_def)
-done
-
-crunch invalidateTLBByASID
-  for typ_at'[wp]: "\<lambda>s. P (typ_at' T p s)"
-crunch invalidateTLBByASID
-  for valid_arch_state'[wp]: "valid_arch_state'"
-lemmas invalidateTLBByASID_typ_ats[wp] = typ_at_lifts [OF invalidateTLBByASID_typ_at']
-
-crunch invalidateTLBByASID
-  for cteCaps_of: "\<lambda>s. P (cteCaps_of s)"
-
-lemma cteCaps_of_ctes_of_lift:
-  "(\<And>P. \<lbrace>\<lambda>s. P (ctes_of s)\<rbrace> f \<lbrace>\<lambda>_ s. P (ctes_of s)\<rbrace>) \<Longrightarrow> \<lbrace>\<lambda>s. P (cteCaps_of s) \<rbrace> f \<lbrace>\<lambda>_ s. P (cteCaps_of s)\<rbrace>"
-  unfolding cteCaps_of_def .
-
-lemmas final_matters'_simps = final_matters'_def [split_simps capability.split arch_capability.split]
-
-crunch deleteCallerCap
-  for idle_thread[wp]: "\<lambda>s. P (ksIdleThread s)"
-  (wp: crunch_wps)
-crunch deleteCallerCap
-  for sch_act_simple: sch_act_simple
-  (wp: crunch_wps)
-crunch deleteCallerCap
-  for sch_act_not[wp]: "sch_act_not t"
-  (wp: crunch_wps)
-crunch deleteCallerCap
-  for typ_at'[wp]: "\<lambda>s. P (typ_at' T p s)"
-  (wp: crunch_wps)
-lemmas deleteCallerCap_typ_ats[wp] = typ_at_lifts [OF deleteCallerCap_typ_at']
-
-crunch emptySlot
-  for ksQ[wp]: "\<lambda>s. P (ksReadyQueues s p)"
-
-lemma setEndpoint_sch_act_not_ct[wp]:
-  "\<lbrace>\<lambda>s. sch_act_not (ksCurThread s) s\<rbrace>
-   setEndpoint ptr val \<lbrace>\<lambda>_ s. sch_act_not (ksCurThread s) s\<rbrace>"
-  by (rule hoare_weaken_pre, wps, wp, simp)
-
-lemma sbn_ct_in_state'[wp]:
-  "\<lbrace>ct_in_state' P\<rbrace> setBoundNotification ntfn t \<lbrace>\<lambda>_. ct_in_state' P\<rbrace>"
-  apply (simp add: ct_in_state'_def)
-  apply (rule hoare_pre)
-   apply (wps setBoundNotification_ct')
-  apply (wp sbn_st_tcb', clarsimp)
-  done
-
-lemma set_ntfn_ct_in_state'[wp]:
-  "\<lbrace>ct_in_state' P\<rbrace> setNotification a ntfn \<lbrace>\<lambda>_. ct_in_state' P\<rbrace>"
-  apply (simp add: ct_in_state'_def)
-  apply (rule hoare_pre)
-   apply (wps setNotification_ksCurThread, wp, clarsimp)
-  done
-
-lemma unbindMaybeNotification_ct_in_state'[wp]:
-  "\<lbrace>ct_in_state' P\<rbrace> unbindMaybeNotification t \<lbrace>\<lambda>_. ct_in_state' P\<rbrace>"
-  apply (simp add: unbindMaybeNotification_def)
-  apply (wp | wpc | simp)+
-  done
-
-lemma setNotification_sch_act_sane:
-  "\<lbrace>sch_act_sane\<rbrace> setNotification a ntfn \<lbrace>\<lambda>_. sch_act_sane\<rbrace>"
-  by (wp sch_act_sane_lift)
-
-context
-notes option.case_cong_weak[cong]
-begin
-crunch unbindNotification, unbindMaybeNotification
-  for sch_act_sane[wp]: "sch_act_sane"
-end
-
-end
+interpretation Finalise_R_3?: Finalise_R_3 arch_final_matters' arch_cap_has_cleanup'
+proof goal_cases
+  interpret Arch  .
+  case 1 show ?case by (intro_locales; (unfold_locales; (fact Finalise_R_3_assms)?)?)
+qed
 
 end
